**证明Part1**    
设从基 $f$ 到基 $e$ 的过渡矩阵为 $P$     
    
 $\Rightarrow(e_1,e_2,\cdots,e_n)    
=(f_1,f_2,\cdots,f_n)\cdot P$  (1)    
    
 $(f_1,f_2,\cdots,f_n)=(e_1,e_2,\cdots,e_n)\cdot A$  (2)    
    
    
    
 $\overset{将(2)带入(1)式右边}\Longrightarrow    
(e_1,e_2,\cdots,e_n)    
=(e_1,e_2,\cdots,e_n)\cdot A\cdot P$     
    
    
 $\Rightarrow(e_1,e_2,\cdots,e_n)\cdot E_n    
=(e_1,e_2,\cdots,e_n)\cdot A\cdot P$     
    
 $\Rightarrow E_n=A\cdot P$  (形式行向量乘法消去律)    
    
    
    
 $\overset{将(1)带入(2)式右边}\Longrightarrow     
(f_1,f_2,\cdots,f_n)    
=(f_1,f_2,\cdots,f_n)\cdot P\cdot A$     
    
    
 $\Rightarrow (f_1,f_2,\cdots,f_n)\cdot E_n    
=(f_1,f_2,\cdots,f_n)\cdot P\cdot A$     
    
 $\Rightarrow E_n=P\cdot A$   (形式行向量乘法消去律)    
    
    
    
 $\Rightarrow E_n=A\cdot P=P\cdot A$      
    
 $\Rightarrow $ 过渡矩阵都是非异阵    
