**例1**  
 $\begin{vmatrix}  
1&-1&2\\\  
2&0&3\\\  
-1&-3&2  
\end{vmatrix}$  
  
 $=1\cdot\begin{vmatrix}  
0&3\\\  
-3&2  
\end{vmatrix}  
-2\cdot\begin{vmatrix}  
-1&2\\\  
-3&2  
\end{vmatrix}  
-1\cdot\begin{vmatrix}  
-1&2\\\  
0&3  
\end{vmatrix}$  
  
 $=9-8+3=4$  
  
**例2**  
 $\begin{vmatrix}  
a&a^2+a+1&1\\\  
0&-a&a-1\\\  
1&0&0  
\end{vmatrix}$  
  
 $=a\cdot\begin{vmatrix}  
-a&a-1\\\  
0&0  
\end{vmatrix}  
+0\cdot\begin{vmatrix}  
a^2+a+1&1\\\  
-a&a-1  
\end{vmatrix}$  
  
 $+1\cdot\begin{vmatrix}  
a^2+a+1&1\\\  
-a&a-1  
\end{vmatrix}$  
  
 $=(a^2+a+1)(a-1)+a=a^3+a-1$  
