**子命题-交换：**    
 $E(i,j)$ 的逆阵就是 $E(i,j)$ 本身，    
即 $E^{-1}(i,j)=E(i,j)\Leftrightarrow E(i,j)\cdot E(i,j)=E$     
    
**证法一**    
 $E(i,j)\cdot E(i,j)$ (看成右乘，按列变换处理)    
    
 $=$ 对 $E(i,j)$ 的第 $i$ 列与第 $j$ 列交换    
    
 $\Rightarrow E(i,j)\cdot E(i,j)= E$     
    
 $\Rightarrow E^{-1}(i,j)=E(i,j)$     
    
**证法二**    
 $E(i,j)\cdot E(i,j)$ (看成左乘，按行变换处理)    
    
 $=$ 对 $E(i,j)$ 的第 $i$ 行与第 $j$ 行交换    
    
 $\Rightarrow E(i,j)\cdot E(i,j)= E$     
    
 $\Rightarrow E^{-1}(i,j)=E(i,j)$     
    
**举例**    
 $\begin{bmatrix}    
0&0&1\\\     
0&1&0\\\     
1&0&0    
\end{bmatrix}    
\cdot\begin{bmatrix}    
0&0&1\\\     
0&1&0\\\     
1&0&0    
\end{bmatrix}$     
