**子命题-乘非零常数**    
 $E^{-1}(i(k))=E(i(\frac1k))    
\Leftrightarrow E(i(\frac1k))\cdot E(i(k))=E$     
    
**证法一**    
 $E(i(k))\cdot E(i(\frac1k))$ (看成右乘，按列变换处理)    
    
 $=对E(i(k))$ 的第 $i$ 列乘以常数 $\frac1k$     
    
 $\Rightarrow E(i(k))\cdot E(i(\frac1k))=E$     
    
 $\Rightarrow E^{-1}(i(k))=E(i(\frac1k))$     
    
**证法二**    
 $E(i(\frac1k))\cdot E(i(k))$ (看成左乘，按行变换处理)    
    
 $=对E(i(k))$ 的第 $i$ 行乘以常数 $\frac1k$     
    
 $\Rightarrow E(i(\frac1k))\cdot E(i(k))=E$     
    
 $\Rightarrow E^{-1}(i(k))=E(i(\frac1k))$     
    
**举例**    
 $\begin{bmatrix}    
1&0&0\\\     
0&2&0\\\     
0&0&1    
\end{bmatrix}    
\cdot\begin{bmatrix}    
1&0&0\\\     
0&\frac12&0\\\     
0&0&1    
\end{bmatrix}$     
