**证明**  
设 $\mu_0\gamma+\mu_1(\gamma+\eta_1)  
+\mu_2(\gamma+\eta_2)+\cdots+  
\mu_{n-r}(\gamma+\eta_{n-r})=\mathbf0$  
  
$\Rightarrow\sum\limits_{i=0}^{n-r}\mu_i  
\cdot\gamma+(\mu_1\cdot\eta_1+\cdots  
+\mu_{n-r}\cdot\eta_{n-r})=\mathbf0\ (\star)$  
  
$\Rightarrow  
A\left(\sum\limits_{i=0}^{n-r}\mu_i  
\cdot\gamma+\mu_1\cdot\eta_1+\cdots  
+\mu_{n-r}\cdot\eta_{n-r}\right)  
=A\cdot\mathbf0$  
  
$\Rightarrow  
\sum\limits_{i=0}^{n-r}\mu_i\cdot A\gamma  
+\underset{齐次线性方程组的基础解系}{\underline{  
A\left(\mu_1\cdot\eta_1+\cdots  
+\mu_{n-r}\cdot\eta_{n-r}\right)}}  
=A\cdot\mathbf0$  
  
$\Rightarrow  
\sum\limits_{i=0}^{n-r}\mu_i  
\cdot A\gamma+\mathbf0  
=\mathbf0$  
  
$\Rightarrow\left(  
\sum\limits_{i=0}^{n-r}\mu_i\right)  
\cdot\beta=\mathbf0$  (数 $\cdot$ 向量，满足整性性质)  
  
$\Rightarrow\sum\limits_{i=0}^{n-r}\mu_i=0$  
  
$\Rightarrow(\star)中的\ \mu_1\cdot\eta_1+\cdots  
+\mu_{n-r}\cdot\eta_{n-r}=\mathbf0$  
  
又因为 $(\eta_1,\eta_2,\cdots,\eta_{n-r})$ 是基础解系  
$\Rightarrow\mu_1=\mu_2=\cdots=\mu_{n-r}=0$  
  
又因为 $\sum\limits_{i=0}^{n-r}\mu_i=0$  
$\Rightarrow\mu_0=0$  
  
综上所述 $\Rightarrow\mu_0=  
\mu_1=\mu_2=\cdots=\mu_{n-r}=0$  
