**子命题-倍加**  
 $E^{-1}(i,j(k))=E(i,j(-k))$  
  
 $\Leftrightarrow E(i,j(k))\cdot E(i,j(-k))=E$  
  
**证法一**  
 $E(i,j(k))\cdot E(i,j(-k))$ (看成右乘，按列变换处理)  
  
 $=对E(i,j(k))$ 的第 $j$ 列乘以 $-k$ 加到第 $i$ 列  
  
 $\Rightarrow E(i,j(k))\cdot E(i,j(-k))=E$  
  
 $\Rightarrow E^{-1}(i,j(k))=E(i,j(-k))$  
  
**证法二**  
 $E(i,j(-k))\cdot E(i,j(k))$ (看成左乘，按行变换处理)  
  
 $=对E(i,j(k))$ 的第 $j$ 行乘以 $-k$ 加到第 $i$ 行  
  
 $\Rightarrow E(i,j(-k))\cdot E(i,j(k))=E$  
  
 $\Rightarrow E^{-1}(i,j(k))=E(i,j(-k))$  
  
**举例**  
 $\begin{bmatrix}  
1&2&0\\\  
0&1&0\\\  
0&0&1  
\end{bmatrix}  
\cdot\begin{bmatrix}  
1&-2&0\\\  
0&1&0\\\  
0&0&1  
\end{bmatrix}$  
  
 $\begin{bmatrix}  
1&0&3\\\  
0&1&0\\\  
0&0&1  
\end{bmatrix}  
\cdot\begin{bmatrix}  
1&0&-3\\\  
0&1&0\\\  
0&0&1  
\end{bmatrix}$  
