**内容**  
$\lim\limits_{n\to+\infty}a_n=a$  
  
$\iff\lim\limits_{k\to+\infty}a_{n_{2k}}=\lim\limits_{k\to+\infty}a_{n_{2k-1}}=a$  
  
**证明: 充分性**  
$\quad\lim\limits_{k\to+\infty}a_{2k}=a$  
  
$\Rightarrow\forall\;\epsilon>0,\;\exists\;N_1>0,\;2k>N_1,\;\forall\;a_{2k},\;|a_{2k}-a|<\epsilon$  
  
$\quad\lim\limits_{k\to+\infty}a_{2k+1}=a$  
  
$\Rightarrow\forall\;\epsilon>0,\;\exists\;N_2>0,\;2k+1>N_2,\;\forall\;a_{2k+1},\;|a_{2k+1}-a|<\epsilon$  
  
$N=\max\{N_1,N_2\}$  
  
$\Rightarrow \forall\;\epsilon>0,\;\exists\;N>0,\;n>N,\;\forall\;a_n,\;|a_n-a|<\epsilon$  
  
**证明: 必要性**  
$\quad\lim\limits_{n\to+\infty}a_n=a$  
  
$\Rightarrow\forall\;\epsilon>0,\;\exists\;N>0,\;n>N,\;\forall\;a_n,(\rm{after}\;a_N)\;|a_n-a|<\epsilon$  
  
$\rm{let}\;k>N\Rightarrow n_k\geq k >N,\;a_k\;\rm{before\;or\;equal}\;a_{n_k}$  
  
$\Rightarrow\forall\;\epsilon>0,\;\exists\;N>0,\;n_k>N,\;\forall\;a_{n_k},\;|a_{n_k}-a|<\epsilon$  
