**定义**  
$a_1=1,\; a_2=1,\; a_{n+1}=a_{n}+a_{n-1}$  
  
$b_n=\dfrac{a_{n+1}}{a_n}=1+\dfrac{a_{n-1}}{a_n}$  
  
$b_{n-1}=\dfrac{a_n}{a_{n-1}}$  
  
$\Rightarrow b_n=1+\dfrac1{b_{n-1}}$  
  
$\Rightarrow b_{n+1}=1+\dfrac1{b_n}$  
  
$\Rightarrow b_1=1,\; b_2=2,\; b_3=\dfrac32,\;b_4=\dfrac53,\;b_5=\dfrac85,\;b_6=\dfrac{13}8,\;\cdots$  
  
**证明: Step1 假设极限存在**  
$\lim\limits_{n\to\infty}b_n=b$  
  
$\Rightarrow \lim\limits_{n\to\infty}b_n=\lim\limits_{n\to\infty}\left[1+\dfrac1{b_{n-1}}\right]$  
  
$\Rightarrow\lim\limits_{n\to\infty}b_n=1+\lim\limits_{n\to\infty}\left[\dfrac1{b_{n-1}}\right]$  
  
$\Rightarrow b=1+\dfrac1b$  
  
$\Rightarrow b=\dfrac{1\pm\sqrt5}{2}$  
  
**证明: Step2 非单调**  
$b_n=1+\dfrac1{b_{n-1}}$  
  
$\rm{if}\;b_n>\dfrac{\sqrt5+1}{2}\Rightarrow1+\dfrac1{b_{n-1}}>\dfrac{\sqrt5+1}{2}\Rightarrow b_{n-1}<\dfrac{\sqrt5+1}{2}$  
  
$\rm{if}\;b_n<\dfrac{\sqrt5+1}{2}\Rightarrow1+\dfrac1{b_{n-1}}<\dfrac{\sqrt5+1}{2}\Rightarrow b_{n-1}>\dfrac{\sqrt5+1}{2}$  
  
**证明: Step3 递推公式**  
$b_n=1+\dfrac{1}{b_{n-1}}$  
  
$\Rightarrow b_{n-1}=1+\dfrac1{b_{n-2}}$  
  
$\Rightarrow b_n=1+\dfrac1{1+\dfrac1{b_{n-2}}}$  
  
$\Rightarrow b_n=1+\dfrac{b_{n-2}}{b_{n-2}+1}$  
  
$b_n=1+\dfrac{1}{b_{n-1}}$  
  
$\Rightarrow b_{n+2}=1+\dfrac1{b_{n+1}}$  
  
$\Rightarrow b_{n+2}=1+\dfrac1{1+\dfrac1{b_n}}$  
  
$\Rightarrow b_{n+2}=1+\dfrac{b_n}{b_n+1}$  
  
**证明: Step4 奇数列**  
<font color=blue>有界</font>  
$1\leq b_1<\dfrac{\sqrt5+1}2,\;b_{n+2}=1+\dfrac{b_n}{b_n+1}=1+\dfrac{1}{1+\dfrac1{b_n}}$  
  
$\rm{suppose}\;1\leq b_{2k-1}<\dfrac{\sqrt5+1}2$  
  
$\Rightarrow\dfrac{\sqrt5-1}2<\dfrac1{b_{2k-1}}\leq1$  
  
$\Rightarrow\dfrac{\sqrt5+1}2<1+\dfrac1{b_{2k-1}}\leq2$  
  
$\Rightarrow\dfrac12\leq\dfrac1{1+\dfrac1{b_{2k-1}}}<\dfrac{\sqrt5-1}2$  
  
$\Rightarrow\dfrac32\leq1+\dfrac1{1+\dfrac1{b_{2k-1}}}<\dfrac{\sqrt5+1}2$  
  
$\Rightarrow1<1+\dfrac1{1+\dfrac1{b_{2k-1}}}<\dfrac{\sqrt5+1}2$  
  
$\Rightarrow1<1+\dfrac{b_{2k-1}}{b_{2k+1}+1}<\dfrac{\sqrt5+1}2$  
  
$\Rightarrow1<b_{2k+1}<\dfrac{\sqrt5+1}2$  
  
<font color=blue>单调递增</font>  
$b_{n+2}-b_n$  
  
$=\left(1+\dfrac{b_n}{b_n+1}\right)-\left(1+\dfrac{b_{n-2}}{b_{n-2}+1}\right)$  
  
$=\dfrac{b_n-b_{n-2}}{(b_n+1)(b_{n-2}+1)}$  
  
$n=2k-1$  
  
$b_{2k+1}-b_{2k-1},\;\cdots,\;b_3-b_1$  
  
$\Rightarrow b_{2k+1}-b_{2k-1}>0$  
  
$\Rightarrow b_{2k+1}>b_{2k-1}$  
  
<font color=blue>求极限</font>  
$b_{n+2}=1+\dfrac{b_n}{b_n+1}$  
  
$n=2k-1$  
  
$\Rightarrow b_{2k+1}=1+\dfrac{b_{2k-1}}{b_{2k-1}+1}$  
  
$\Rightarrow\lim\limits_{n\to\infty}b_{2k+1}=\lim\limits_{n\to\infty}\left(1+\dfrac{b_{2k-1}}{b_{2k-1}+1}\right)=1+\lim\limits_{n\to\infty}(b_{2k-1})\div\left(\lim\limits_{n\to\infty}b_{2k-1}+1\right)$  
  
$\Rightarrow b=1+\dfrac{b}{b+1}\;(b^2+b=b+1+b)$  
  
$\Rightarrow b^2-b-1=0$  
  
$\Rightarrow b=\dfrac{1\pm\sqrt5}2$  
  
**证明: Step5 偶数列**  
<font color=blue>有界</font>  
$\dfrac{\sqrt5+1}2<b_2\leq2,\;b_{n+2}=1+\dfrac{b_n}{b_n+1}=1+\dfrac{1}{1+\dfrac1{b_n}}$  
  
$\rm{suppose}\;\dfrac{\sqrt5+1}2<b_{2k}\leq2$  
  
$\Rightarrow \dfrac12\leq\dfrac1{b_{2k}}<\dfrac{\sqrt5-1}2$  
  
$\Rightarrow\dfrac32\leq1+\dfrac1{b_{2k}}<\dfrac{\sqrt5+1}2$  
  
$\Rightarrow\dfrac{\sqrt5-1}2<\dfrac1{1+\dfrac1{b_{2k}}}\leq\dfrac23$  
  
$\Rightarrow\dfrac{\sqrt5+1}2<1+\dfrac1{1+\dfrac1{b_{2k}}}\leq\dfrac53$  
  
$\Rightarrow\dfrac{\sqrt5+1}2<1+\dfrac{b_{2k}}{b_{2k}+1}\leq\dfrac53<2$  
  
$\Rightarrow\dfrac{\sqrt5+1}2<b_{2k+2}<2$  
  
<font color=blue>单调递减</font>  
$b_{n+2}-b_n$  
  
$=\left(1+\dfrac{b_n}{b_n+1}\right)-\left(1+\dfrac{b_{n-2}}{b_{n-2}+1}\right)$  
  
$=\dfrac{b_n-b_{n-2}}{(b_n+1)(b_{n-2}+1)}$  
  
$n=2k$  
  
$b_{2k+2}-b_{2k},\;\cdots,\;b_4-b_2$  
  
$\Rightarrow b_{2k+2}-b_{2k}<0$  
  
$\Rightarrow b_{2k+2}<b_{2k}$  
  
<font color=blue>求极限</font>  
$b_{n+2}=1+\dfrac{b_n}{b_n+1}$  
  
$n=2k$  
  
$\Rightarrow b_{2k+2}=1+\dfrac{b_{2k}}{b_{2k}+1}$  
  
$\Rightarrow\lim\limits_{n\to\infty}b_{2k+2}=\lim\limits_{n\to\infty}\left(1+\dfrac{b_{2k}}{b_{2k}+1}\right)=1+\lim\limits_{n\to\infty}(b_{2k})\div\left(\lim\limits_{n\to\infty}b_{2k}+1\right)$  
  
$\Rightarrow b=1+\dfrac{b}{b+1}\;(b^2+b=b+1+b)$  
  
$\Rightarrow b^2-b-1=0$  
  
$\Rightarrow b=\dfrac{1\pm\sqrt5}2$  
  
**证明: Step6 奇数列极限＝偶数列极限**  
$\lim\limits_{n\to\infty}b_{2k}=\lim\limits_{n\to\infty}b_{2k-1}=\dfrac{1+\sqrt5}2$  
