**内容**  
三角形 $\triangle ABC$ 中，  
$\cos\angle C=\dfrac{a^2+b^2-c^2}{2\cdot a\cdot b}$  
  
**证法一**  
三角形 $\triangle ABC$ 中  
  
$\Rightarrow\overrightarrow{AB}=\overrightarrow{CB}-\overrightarrow{CA}$  
  
$\Rightarrow|\overrightarrow{AB}|=|\overrightarrow{CB}-\overrightarrow{CA}|$  
  
$\Rightarrow|\overrightarrow{AB}|^2=|\overrightarrow{CB}-\overrightarrow{CA}|^2$  
  
$\Rightarrow c^2=|\overrightarrow{CB}|^2-2\overrightarrow{CB}\cdot\overrightarrow{CA}+|\overrightarrow{CA}|^2$  
  
$\Rightarrow c^2=a^2-2\cdot a\cdot b\cdot\cos\angle C+b^2$  
  
$\Rightarrow\cos\angle C=\dfrac{a^2+b^2-c^2}{2\cdot a\cdot b}$  
  
**证法二**  
以 $C$ 点为坐标原点， $CB$ 为 $x$ 轴正半轴  
  
$\Rightarrow A$ 点坐标为 $(b\cos\angle C,b\sin\angle C)$  
  
$\Rightarrow B$ 点坐标为 $(a,0)$  
  
$\Rightarrow\overrightarrow{AB}=(b-b\cos\angle C,-a\sin\angle C)$  
  
$\Rightarrow|\overrightarrow{AB}|=\sqrt{(a-b\cos\angle C)^2+(-b\sin\angle C)^2}$  
  
$=\sqrt{a^2-2ab\cos\angle C+b^2}$  
  
$\Rightarrow c=\sqrt{a^2-2ab\cos\angle C+b^2}$  
  
$\Rightarrow\cos\angle C=\dfrac{a^2+b^2-c^2}{2\cdot a\cdot b}$  
  
**说明**  
1 同理可得  
$\cos\angle A=\dfrac{c^2+b^2-a^2}{2\cdot c\cdot b}$  
  
$\cos\angle B=\dfrac{a^2+c^2-b^2}{2\cdot a\cdot c}$  
  
2 当 $\angle C=90^\circ$ ，退化成了勾股定理  
  
**推论**  
$\angle A$ 是锐角 $\Leftrightarrow\cos\angle A>0\Leftrightarrow b^2+c^2>a^2$  
  
$\angle A$ 是直角 $\Leftrightarrow\cos\angle A=0\Leftrightarrow b^2+c^2=a^2$ (勾股定理)  
  
$\angle A$ 是钝角 $\Leftrightarrow\cos\angle A<0\Leftrightarrow b^2+c^2<a^2$  
  
**应用场景**  
1 已知两边以及夹角，求第三边  
2 已知三边，求三个角  
