**内容**
$\forall\;n\in N,\;\exists\;k\in(0,1),\;|x_{n+1}-x_n|\leq k\,|x_n-x_{n-1}|$

$\Rightarrow \lim\limits_{n\to\infty}x_n=a$

**证明: 柯西审敛原理**
$|x_{n+1}-x_n|\leq k\,|x_n-x_{n-1}|$

$\Rightarrow $

$|x_{3}-x_2|\leq k\,|x_2-x_{1}|$

$|x_4-x_3|\leq k\,|x_3-x_2|\leq k^2\,|x_2-x_1|$

$|x_5-x_4|\leq k\,|x_4-x_3|\leq k^3\,|x_2-x_1|$

$\cdots$

$|x_{n+1}-x_n|\leq k\,|x_n-x_{n-1}|\leq k^{n-1}\,|x_2-x_1|$

$\cdots$

$|x_{m}-x_{m-1}|\leq k\,|x_{m-1}-x_{m-2}|\leq k^{m-2}\,|x_2-x_1|$

---

$|x_m-x_n|=|(x_m-x_{m-1})+(x_{m-1}-x_{m-2})+(x_{m-2}-x_{m-3})+\cdots+(x_{n+2}-x_{n+1})+(x_{n+1}-x_n)|$

$\leq|x_m-x_{m-1}|+|x_{m-1}-x_{m-2}|+|x_{m-2}-x_{m-3}|+\cdots+|x_{n+2}-x_{n+1}|+|x_{n+1}-x_n|$

$\leq k^{m-2}\,|x_2-x_1|+k^{m-3}\,|x_2-x_1|+k^{m-4}\,|x_2-x_1|+\cdots+k^{n-1}\,|x_2-x_1|$

$=k^{n-1}\,|x_2-x_1|\cdot(1+k+k^2+\cdots+k^{m-n-3}+k^{m-n-2}+k^{m-n-1})$

$=k^{n-1}\,|x_2-x_1|\cdot\dfrac{1\cdot(1-k^{m-n})}{1-k}$

$<k^{n-1}\,|x_2-x_1|\cdot\dfrac{1}{1-k}$

---

$\forall\;\epsilon>0,\;\exists\;N,\;n>N,\;k^{n-1}\,|x_2-x_1|\cdot\dfrac{1}{1-k}<\epsilon$

$\Rightarrow\forall\;\epsilon>0,\;\exists\;N,\;n>N,\;|x_m-x_n|<\epsilon$
