**定理**  
$y=a^x\,(a>0,a\neq1)$  
  
$\Rightarrow\lim\limits_{x\to x_0}a^x=a^{x_0}$  
  
**证明-分析**  
$\lim\limits_{x\to x_0}a^x=a^{x_0}$  
  
$\iff \lim\limits_{x\to x_0}(a^x-a^{x_0})=0$  
  
$\iff \lim\limits_{x\to x_0}[a^{x_0}(a^{x-x_0}-1)]=0$  
  
$\iff a^{x_0}\lim\limits_{x\to x_0}(a^{x-x_0}-1)=0$  
  
$\Leftarrow\lim\limits_{x\to x_0}(a^{x-x_0}-1)=0$  
  
$\iff \lim\limits_{x\to x_0}a^{x-x_0}=1$  
  
$\Leftarrow \lim\limits_{x\to0}a^x=1\,(x-x_0=\Delta x)a>1$  
  
**证法一(夹逼定理)**  
$\lim\limits_{n\to\infty}\sqrt[n]a=\lim\limits_{n\to\infty}a^{\dfrac1n}=1$  
  
$a>1,\;0<x<\dfrac1n\;\left(\dfrac1n=\dfrac1{[x]},0<x<1\right)$  
  
$\Rightarrow 1<a^x<a^{\dfrac1n}$  
  
$\lim\limits_{n\to\infty}1=1,\;\lim\limits_{n\to\infty}a^{\dfrac1n}=1$  
  
$\Rightarrow \lim\limits_{x\to0^+}a^x=1$  
  
$x<0,\;y=-x$  
  
$\Rightarrow a^x=a^{-y}=\dfrac1{a^y}$  
  
$\Rightarrow\lim\limits_{x\to0^-}a^x=\lim\limits_{y\to0^+}a^{-y}=\lim\limits_{y\to0^+}\dfrac1{a^y}=1\div\lim\limits_{y\to0^+}a^y=1$  
  
**证法二(ε-δ语言)**  
$\lim\limits_{x\to0}a^x=1$  
  
$\iff\forall\;\epsilon>0,\;\exists\;\delta>0,\;|x-0|<\delta,\;|a^x-1|<\epsilon$  
  
$\iff\forall\;\epsilon>0,\;\exists\;\delta>0,\;|x|<\delta,\;1-\epsilon<a^x<1+\epsilon$  
  
$\iff\forall\;\epsilon>0,\;\exists\;\delta>0,\;|x|<\delta,\;\log_a^{1-\epsilon}<x<\log_a^{1+\epsilon}$  
  
$\Leftarrow-\log_a^{1+\epsilon}<x<\log_a^{1+\epsilon}$  
  
$\Leftarrow\rm{let}\;\delta=\max\left\{\log_a^{1-\epsilon},\log_a^{1+\epsilon}\right\}=\log_a^{1+\epsilon}                               0<\epsilon<1$  
  
$\Rightarrow 1<1+\epsilon<2$  
  
$\Rightarrow \log_a^{1}<\log_a^{1+\epsilon}<\log_a^2$  
  
$\Rightarrow-\log_a^{2}<-\log_a^{1+\epsilon}<-\log_a^1=0$  
  
$\Rightarrow-\log_a^{2}<-\log_a^{1+\epsilon}<0$  
  
$\Rightarrow -1<-\epsilon<0$  
  
$\Rightarrow 0<1-\epsilon<1$  
  
$\Rightarrow-\infty<\log_a^{1-\epsilon}<0$  
  
$-\log_a^{1+\epsilon}<x\Rightarrow\log_a^{1-\epsilon}<x$  
  
$0<a<1$  
  
$\rm{let}\;a=\dfrac1b\Rightarrow b>1$  
  
$\Rightarrow\lim\limits_{x\to0}a^x=\lim\limits_{x\to0}\dfrac1{b^x}=1$  
