**内容**
$\sin\left(\dfrac{3\pi}{2}-\alpha\right)=-\cos\alpha$

$\sin\left(\dfrac{3\pi}{2}+\alpha\right)=-\cos\alpha$

$\cos\left(\dfrac{3\pi}{2}-\alpha\right)=-\sin\alpha$

$\cos\left(\dfrac{3\pi}{2}+\alpha\right)=\sin\alpha$

**证明**
$\sin\left(\dfrac{3\pi}{2}-\alpha\right)$

$=\sin\left[\pi+\left(\dfrac{\pi}{2}-\alpha\right)\right]$

$=-\sin\left(\dfrac{\pi}{2}-\alpha\right)$

$=-\cos\alpha$

---

$\sin\left(\dfrac{3\pi}{2}+\alpha\right)$

$=\sin\left[\pi+\left(\dfrac{\pi}{2}+\alpha\right)\right]$

$=-\sin\left(\dfrac{\pi}{2}+\alpha\right)$

$=-\cos\alpha$

---

$\cos\left(\dfrac{3\pi}{2}-\alpha\right)$

$=\cos\left[\pi+\left(\dfrac{\pi}{2}-\alpha\right)\right]$

$=-\cos\left(\dfrac{\pi}{2}-\alpha\right)$

$=-\sin\alpha$

---

$\cos\left(\dfrac{3\pi}{2}+\alpha\right)$

$=\cos\left[\pi+\left(\dfrac{\pi}{2}+\alpha\right)\right]$

$=-\cos\left(\dfrac{\pi}{2}+\alpha\right)$

$=-(-\sin\alpha)$

$=\sin\alpha$
