**内容**  
$\sin(\alpha-\beta)=\sin\alpha\cdot\cos\beta-\cos\alpha\cdot\sin\beta$  
  
简记为 $S_{(\alpha-\beta)}$  
  
**证法一**  
$\sin(\alpha-\beta)$  
  
$=\sin(\alpha+(-\beta))$  
  
$=\sin\alpha\cdot\cos(-\beta)+\cos\alpha\cdot\sin(-\beta)$  
  
$=\sin\alpha\cdot\cos\beta-\cos\alpha\cdot\sin\beta$  
  
**证法二**  
$\sin(\alpha-\beta)$  
  
$=\cos\left[\dfrac{\pi}{2}-(\alpha-\beta)\right]$  
  
$=\cos\left[\dfrac{\pi}{2}-\alpha+\beta\right]$  
  
$=\cos\left(\dfrac{\pi}{2}-\alpha\right)\cdot\cos\beta-\sin\left(\dfrac{\pi}{2}-\alpha\right)\cdot\sin\beta$  
  
$=\sin\alpha\cdot\cos\beta-\cos\alpha\cdot\sin\beta$  
