**内容1**  
$\cos\alpha\cdot\cos\beta=\dfrac12[\cos(\alpha-\beta)+\cos(\alpha+\beta)]$  
  
**证明1**  
$\cos(\alpha-\beta)=\cos\alpha\cdot\cos\beta+\sin\alpha\cdot\sin\beta$  
  
$\cos(\alpha+\beta)=\cos\alpha\cdot\cos\beta-\sin\alpha\cdot\sin\beta$  
  
$\Rightarrow\cos(\alpha-\beta)+\cos(\alpha+\beta)=(\cos\alpha\cdot\cos\beta+\sin\alpha\cdot\sin\beta)+(\cos\alpha\cdot\cos\beta-\sin\alpha\cdot\sin\beta)$  
  
$=2\cos\alpha\cdot\cos\beta$  
  
$\Rightarrow \cos\alpha\cdot\cos\beta=\dfrac12[\cos(\alpha-\beta)+\cos(\alpha+\beta)]$  
  
---  
  
**内容2**  
$\sin\alpha\cdot\sin\beta=\dfrac12[\cos(\alpha-\beta)-\cos(\alpha+\beta)]$  
  
**证明2**  
$\cos(\alpha-\beta)=\cos\alpha\cdot\cos\beta+\sin\alpha\cdot\sin\beta$  
  
$\cos(\alpha+\beta)=\cos\alpha\cdot\cos\beta-\sin\alpha\cdot\sin\beta$  
  
$\Rightarrow\cos(\alpha-\beta)-\cos(\alpha+\beta)=(\cos\alpha\cdot\cos\beta+\sin\alpha\cdot\sin\beta)-(\cos\alpha\cdot\cos\beta-\sin\alpha\cdot\sin\beta)$  
  
$=2\sin\alpha\cdot\sin\beta$  
  
$\Rightarrow\sin\alpha\cdot\sin\beta=\dfrac12[\cos(\alpha-\beta)-\cos(\alpha+\beta)]$  
  
---  
  
**内容3**  
$\sin\alpha\cdot\cos\beta=\dfrac12[\sin(\alpha+\beta)+\sin(\alpha-\beta)]$  
  
**证明3**  
$\sin(\alpha+\beta)=\sin\alpha\cdot\cos\beta+\cos\alpha\cdot\sin\beta$  
  
$\sin(\alpha-\beta)=\sin\alpha\cdot\cos\beta-\cos\alpha\cdot\sin\beta$  
  
$\Rightarrow\sin(\alpha+\beta)+\sin(\alpha-\beta)=[\sin\alpha\cdot\cos\beta+\cos\alpha\cdot\sin\beta]+[\sin\alpha\cdot\cos\beta-\cos\alpha\cdot\sin\beta]$  
  
$=2\sin\alpha\cdot\cos\beta$  
  
$\Rightarrow\sin\alpha\cdot\cos\beta=\dfrac12[\sin(\alpha+\beta)+\sin(\alpha-\beta)]$  
  
---  
  
**内容4**  
$\cos\alpha\cdot\sin\beta=\dfrac12[\sin(\alpha+\beta)-\sin(\alpha-\beta)]$  
  
**证明4**  
$\sin(\alpha+\beta)=\sin\alpha\cdot\cos\beta+\cos\alpha\cdot\sin\beta$  
  
$\sin(\alpha-\beta)=\sin\alpha\cdot\cos\beta-\cos\alpha\cdot\sin\beta$  
  
$\Rightarrow\sin(\alpha+\beta)-\sin(\alpha-\beta)=[\sin\alpha\cdot\cos\beta+\cos\alpha\cdot\sin\beta]-[\sin\alpha\cdot\cos\beta-\cos\alpha\cdot\sin\beta]$  
  
$=2\cos\alpha\cdot\sin\beta$  
  
$\Rightarrow\cos\alpha\cdot\sin\beta=\dfrac12[\sin(\alpha+\beta)-\sin(\alpha-\beta)]$  
  
---  
  
**说明**  
两个三角函数相乘，数分里面用到了一次  
