**内容**  
$\sin3\alpha=3\sin\alpha-4\sin^3\alpha$  
  
**证明**  
$\sin3\alpha$  
  
$=\sin(\alpha+2\alpha)$  
  
$=\sin\alpha\cdot\cos2\alpha+\cos\alpha\cdot\sin2\alpha$  
  
$=\sin\alpha\cdot(1-2\sin^2\alpha)+2\cos\alpha\cdot\cos\alpha\cdot\sin\alpha$  
  
$=\sin\alpha-2\sin^3\alpha+2(1-\sin^2\alpha)\cdot\sin\alpha$  
  
$=\sin\alpha-2\sin^3\alpha+2\sin\alpha-2\sin^3\alpha$  
  
$=3\sin\alpha-4\sin^3\alpha$  
  
**推论**  
$\sin3\alpha=4\sin\alpha\cdot\sin(\alpha+\dfrac\pi3)\cdot\sin(\dfrac\pi3-\alpha)$  
  
$\sin3\alpha=3\sin\alpha-4\sin^3\alpha$  
  
$=4\sin\alpha\cdot\left(\dfrac34-\sin^2\alpha\right)=4\sin\alpha\cdot\left[\dfrac34(\sin^2\alpha+\cos^2\alpha)-\sin^2\alpha\right]$  
  
$=4\sin\alpha\cdot\left[\dfrac34\cos^2\alpha-\dfrac14\sin^2\alpha\right]$  
  
$=4\sin\alpha\cdot\left(\dfrac{\sqrt3}2\cos\alpha-\dfrac12\sin\alpha\right)\cdot\left(\dfrac{\sqrt3}2\cos\alpha+\dfrac12\sin\alpha\right)$  
  
$=4\sin\alpha\cdot\left(\sin\dfrac\pi3\cos\alpha+\cos\dfrac\pi3\sin\alpha\right)\cdot\left(\sin\dfrac\pi3\cos\alpha-\cos\dfrac\pi3\sin\alpha\right)$  
  
$=4\sin\alpha\cdot\sin(\alpha+\dfrac\pi3)\cdot\sin(\dfrac\pi3-\alpha)$  
