**内容1**  
$\cos\alpha+\cos\beta=2\cos\dfrac{\alpha+\beta}2\cdot\cos\dfrac{\alpha-\beta}2$  
  
**证明1**  
$\rm{let}\;\alpha=\dfrac{\alpha+\beta}2+\dfrac{\alpha-\beta}2,\;\beta=\dfrac{\alpha+\beta}2-\dfrac{\alpha-\beta}2$  
  
$\Rightarrow\cos\alpha+\cos\beta$  
  
$=\cos\left(\dfrac{\alpha+\beta}2+\dfrac{\alpha-\beta}2\right)+\cos\left(\dfrac{\alpha+\beta}2-\dfrac{\alpha-\beta}2\right)$  
  
$=\left[\cos\left(\dfrac{\alpha+\beta}2\right)\cdot\cos\left(\dfrac{\alpha-\beta}2\right)-\sin\left(\dfrac{\alpha+\beta}2\right)\cdot\sin\left(\dfrac{\alpha-\beta}2\right)\right]+\left[\cos\left(\dfrac{\alpha+\beta}2\right)\cdot\cos\left(\dfrac{\alpha-\beta}2\right)+\sin\left(\dfrac{\alpha+\beta}2\right)\cdot\sin\left(\dfrac{\alpha-\beta}2\right)\right]$  
  
$=2\cos\left(\dfrac{\alpha+\beta}2\right)\cdot\cos\left(\dfrac{\alpha-\beta}2\right)$  
  
---  
  
**内容2**  
$\cos\alpha-\cos\beta=-2\sin\dfrac{\alpha+\beta}2\cdot\sin\dfrac{\alpha-\beta}2$  
  
**证明2**  
$\rm{let}\;\alpha=\dfrac{\alpha+\beta}2+\dfrac{\alpha-\beta}2,\;\beta=\dfrac{\alpha+\beta}2-\dfrac{\alpha-\beta}2$  
  
$\Rightarrow\cos\alpha-\cos\beta$  
  
$=\cos\left(\dfrac{\alpha+\beta}2+\dfrac{\alpha-\beta}2\right)-\cos\left(\dfrac{\alpha+\beta}2-\dfrac{\alpha-\beta}2\right)$  
  
$=\left[\cos\left(\dfrac{\alpha+\beta}2\right)\cdot\cos\left(\dfrac{\alpha-\beta}2\right)-\sin\left(\dfrac{\alpha+\beta}2\right)\cdot\sin\left(\dfrac{\alpha-\beta}2\right)\right]-\left[\cos\left(\dfrac{\alpha+\beta}2\right)\cdot\cos\left(\dfrac{\alpha-\beta}2\right)+\sin\left(\dfrac{\alpha+\beta}2\right)\cdot\sin\left(\dfrac{\alpha-\beta}2\right)\right]$  
  
$=-2\sin\left(\dfrac{\alpha+\beta}2\right)\cdot\sin\left(\dfrac{\alpha-\beta}2\right)$  
  
---  
  
**内容3**  
$\sin\alpha+\sin\beta=2\sin\dfrac{\alpha+\beta}2\cdot\cos\dfrac{\alpha-\beta}2$  
  
**证明3**  
$\rm{let}\;\alpha=\dfrac{\alpha+\beta}2+\dfrac{\alpha-\beta}2,\;\beta=\dfrac{\alpha+\beta}2-\dfrac{\alpha-\beta}2$  
  
$\sin\alpha+\sin\beta$  
  
$=\sin\left(\dfrac{\alpha+\beta}2+\dfrac{\alpha-\beta}2\right)+\sin\left(\dfrac{\alpha+\beta}2-\dfrac{\alpha-\beta}2\right)$  
  
$=\left[\sin\left(\dfrac{\alpha+\beta}2\right)\cdot\cos\left(\dfrac{\alpha-\beta}2\right)+\cos\left(\dfrac{\alpha+\beta}2\right)\cdot\sin\left(\dfrac{\alpha-\beta}2\right)\right]+\left[\sin\left(\dfrac{\alpha+\beta}2\right)\cdot\cos\left(\dfrac{\alpha-\beta}2\right)-\cos\left(\dfrac{\alpha+\beta}2\right)\cdot\sin\left(\dfrac{\alpha-\beta}2\right)\right]$  
  
$=2\sin\dfrac{\alpha+\beta}2\cdot\cos\dfrac{\alpha-\beta}2$  
  
---  
  
**内容4**  
$\sin\alpha-\sin\beta=2\cos\dfrac{\alpha+\beta}2\cdot\sin\dfrac{\alpha-\beta}2$  
  
**证明4**  
$\rm{let}\;\alpha=\dfrac{\alpha+\beta}2+\dfrac{\alpha-\beta}2,\;\beta=\dfrac{\alpha+\beta}2-\dfrac{\alpha-\beta}2$  
  
$\sin\alpha-\sin\beta$  
  
$=\sin\left(\dfrac{\alpha+\beta}2+\dfrac{\alpha-\beta}2\right)-\sin\left(\dfrac{\alpha+\beta}2-\dfrac{\alpha-\beta}2\right)$  
  
$=\left[\sin\left(\dfrac{\alpha+\beta}2\right)\cdot\cos\left(\dfrac{\alpha-\beta}2\right)+\cos\left(\dfrac{\alpha+\beta}2\right)\cdot\sin\left(\dfrac{\alpha-\beta}2\right)\right]-\left[\sin\left(\dfrac{\alpha+\beta}2\right)\cdot\cos\left(\dfrac{\alpha-\beta}2\right)-\cos\left(\dfrac{\alpha+\beta}2\right)\cdot\sin\left(\dfrac{\alpha-\beta}2\right)\right]$  
  
$=2\cos\dfrac{\alpha+\beta}2\cdot\sin\dfrac{\alpha-\beta}2$  
  
---  
  
**内容5**  
$\tan\alpha+\tan\beta=\dfrac{\sin(\alpha+\beta)}{\cos\alpha\cdot\cos\beta}$  
  
**证明5**  
$\tan\alpha+\tan\beta$  
  
$=\dfrac{\sin\alpha}{\cos\alpha}+\dfrac{\sin\beta}{\cos\beta}$  
  
$= \dfrac{\sin\alpha\cdot\cos\beta+\sin\beta\cdot\cos\alpha}{\cos\alpha\cdot\cos\beta}$  
  
$=\dfrac{\sin(\alpha+\beta)}{\cos\alpha\cdot\cos\beta}$  
  
---  
  
**内容6**  
$\tan\alpha-\tan\beta=\dfrac{\sin(\alpha-\beta)}{\cos\alpha\cdot\cos\beta}$  
  
**证明6**  
$\tan\alpha-\tan\beta$  
  
$=\dfrac{\sin\alpha}{\cos\alpha}-\dfrac{\sin\beta}{\cos\beta}$  
  
$= \dfrac{\sin\alpha\cdot\cos\beta-\sin\beta\cdot\cos\alpha}{\cos\alpha\cdot\cos\beta}$  
  
$=\dfrac{\sin(\alpha-\beta)}{\cos\alpha\cdot\cos\beta}$  
  
**说明**  
两个三角函数相加(减)  
  
余加余，余并肩  
余减余，负正弦  
正加正，正在前  
正减正，余在前  
  
还有tan和cot的  
