**内容**
$\quad\lim f(x)=A,\;\lim g(x)=B\Rightarrow$

$\quad\alpha\lim f(x)+\beta\lim g(x)$

$\quad=\lim\alpha f(x)+\lim\beta g(x)$

$\quad=\lim[\alpha f(x)+\beta g(x)]$

$\quad=\alpha A+\beta B$

**具体形式: $x\to x_0$**
$\quad\lim\limits_{x\to x_0}f(x)=A,\;\lim\limits_{x\to x_0}g(x)=B\Rightarrow$

$\quad\alpha\lim\limits_{x\to x_0}f(x)+\beta\lim\limits_{x\to x_0}g(x)$

$\quad=\lim\limits_{x\to x_0}\alpha f(x)+\lim\limits_{x\to x_0}\beta g(x)$

$\quad=\lim\limits_{x\to x_0}[\alpha f(x)+\beta g(x)]$

$\quad=\alpha A+\beta B$

**具体形式: $x\to x_0^+$**
$\quad\lim\limits_{x\to x_0^+}f(x)=A,\;\lim\limits_{x\to x_0^+}g(x)=B\Rightarrow$

$\quad\alpha\lim\limits_{x\to x_0^+}f(x)+\beta\lim\limits_{x\to x_0^+}g(x)$

$\quad=\lim\limits_{x\to x_0^+}\alpha f(x)+\lim\limits_{x\to x_0^+}\beta g(x)$

$\quad=\lim\limits_{x\to x_0^+}[\alpha f(x)+\beta g(x)]$

$\quad=\alpha A+\beta B$

**具体形式: $x\to x_0^-$**
$\quad\lim\limits_{x\to x_0^-}f(x)=A,\;\lim\limits_{x\to x_0^-}g(x)=B\Rightarrow$

$\quad\alpha\lim\limits_{x\to x_0^-}f(x)+\beta\lim\limits_{x\to x_0^-}g(x)$

$\quad=\lim\limits_{x\to x_0^-}\alpha f(x)+\lim\limits_{x\to x_0^-}\beta g(x)$

$\quad=\lim\limits_{x\to x_0^-}[\alpha f(x)+\beta g(x)]$

$\quad=\alpha A+\beta B$

**具体形式: $x\to+\infty$**
$\quad\lim\limits_{x\to+\infty}f(x)=A,\;\lim\limits_{x\to+\infty}g(x)=B\Rightarrow$

$\quad\alpha\lim\limits_{x\to+\infty}f(x)+\beta\lim\limits_{x\to+\infty}g(x)$

$\quad=\lim\limits_{x\to+\infty}\alpha f(x)+\lim\limits_{x\to+\infty}\beta g(x)$

$\quad=\lim\limits_{x\to+\infty}[\alpha f(x)+\beta g(x)]$

$\quad=\alpha A+\beta B$

**具体形式: $x\to-\infty$**
$\quad\lim\limits_{x\to-\infty}f(x)=A,\;\lim\limits_{x\to-\infty}g(x)=B\Rightarrow$

$\quad\alpha\lim\limits_{x\to-\infty}f(x)+\beta\lim\limits_{x\to-\infty}g(x)$

$\quad=\lim\limits_{x\to-\infty}\alpha f(x)+\lim\limits_{x\to-\infty}\beta g(x)$

$\quad=\lim\limits_{x\to-\infty}[\alpha f(x)+\beta g(x)]$

$\quad=\alpha A+\beta B$

**具体形式: $x\to\infty$**
$\quad\lim\limits_{x\to\infty}f(x)=A,\;\lim\limits_{x\to\infty}g(x)=B\Rightarrow$

$\quad\alpha\lim\limits_{x\to\infty}f(x)+\beta\lim\limits_{x\to\infty}g(x)$

$\quad=\lim\limits_{x\to\infty}\alpha f(x)+\lim\limits_{x\to\infty}\beta g(x)$

$\quad=\lim\limits_{x\to\infty}[\alpha f(x)+\beta g(x)]$

$\quad=\alpha A+\beta B$
