**内容**  
若 $e^w=z$ ，则 $w=\rm{Ln}(z)$  
  
公式推导  
设 $z=re^{i\theta}$ ， $w=a+bi$  
  
$\Rightarrow e^{a+bi}=re^{i\theta}$  
  
$\Rightarrow e^a e^{ib}=re^{i\theta}$  
  
$\Rightarrow\begin{cases}e^a=r\\\ b=\theta+2k\pi,&k\in\mathbb Z\end{cases}$  
  
$\Rightarrow\begin{cases}a=\ln r,&r\in\mathbb R\\\ b=\theta+2k\pi,&k\in\mathbb Z\end{cases}$  
  
$\Rightarrow w=\rm{Ln}(z)=\ln r+(\theta+2k\pi)i$  
  
定义: 对数的主值  
$\ln z=\ln r+\theta_0i$  
$\Rightarrow\rm{Ln}(z)=\ln z+2k\pi i$  
取定一个 $k$ ， $w$ 变成单值函数，称为 $w$ 的一个分支  
  
举例1: $\rm{Ln}(-1)=\ln1+(\pi+2k\pi)i=(1+2k)\pi i$  
  
举例2: $\rm{Ln}(1+i)=\ln(\sqrt2)+\left(\dfrac\pi4+2k\pi\right)i$  
