**待证明**
$1^\circ\ V_0=V_1\oplus V_2\oplus\cdots \oplus V_m$ ($V_0$是直和空间)

$2^\circ\ \forall\ 2\le i\le m，V_i\cap
(V_1+V_2+\cdots+V_{i-1})=\{\mathbf0\}$
$V_2\cap V_1=\{\mathbf0\}$
$V_3\cap(V_1+V_2)=\{\mathbf0\}$
$V_4\cap(V_1+V_2+V_3)=\{\mathbf0\}$
$\cdots$
$V_i\cap(V_1+V_2+\cdots+V_{i-1})=\{\mathbf0\}$

**证明**
$(1)\Rightarrow(2)$
$V_i\cap(V_1+V_2+\cdots+V_{i-1})\subseteq$
$V_i\cap(V_1+\cdots+V_{i-1}+V_{i+1}+\cdots+V_m)$

$V_i\cap(V_1+V_2+\cdots+
V_{i-1}+V_{i+1}+\cdots+V_m)=\{\mathbf0\}$

$\Rightarrow
V_i\cap(V_1+V_2+\cdots+V_{i-1})=\{\mathbf0\}$

---

$(V_1+\cdots+V_{i-1}+V_{i+1}+\cdots+V_m)$中元素的形式为：

$\lambda_1\alpha_1+\cdots+\lambda_{i-1}\alpha_{i-1}+\lambda_{i+1}\alpha_{i+1}+\cdots+\lambda_m\alpha_m\ (\bigstar)$

当$\lambda_{i+1}=\cdots=\lambda_m=0$时，$(\bigstar)$就变成了$V_1+V_2+\cdots+V_{i-1}$中的形式

$\Rightarrow(V_1+V_2+\cdots+V_{i-1})$是$(V_1+\cdots+V_{i-1}+V_{i+1}+\cdots+V_m)$的子集
