**内容**  
设 $\Phi,\ \Psi\in\rm{Hom}(V,U)$ ，  
 $(e_1,\cdots,e_n)$ 是 $V_K^n$ 的一个基，  
 $(f_1,\cdots,f_m)$ 是 $U_K^m$ 的一个基，  
 $\Phi$ 在该基下的表示矩阵为 $A$ ，  
 $\Psi$ 在该基下的表示矩阵为 $B$ ，  
则 $(k\cdot\Phi)$ 在该基下的表示矩阵为 $k\cdot A$  
  
**证明**  
 $(k\cdot\Phi)(e_i),\ 1\le i\le n$  
  
 $=k\cdot\Phi(e_i)$  
  
 $=k\cdot(a_{1i}f_1+a_{2i}f_2+\cdots+a_{mi}f_m)$  
  
 $=(k\cdot a_{1i})f_1+(k\cdot a_{2i})f_2+\cdots+(k\cdot a_{mi})f_m$  
  
 $\Rightarrow(k\cdot\Phi)(e_i)=(k\cdot a_{1i})f_1+(k\cdot a_{2i})f_2+\cdots+(k\cdot a_{mi})f_m$  
  
 $\Rightarrow(k\cdot\Phi)$ 在该基下的表示矩阵为 $k\cdot A$  
  
---  
  
 $((k\cdot\Phi)(e_1),(k\cdot\Phi)(e_2),\cdots,(k\cdot\Phi)(e_n))$  
  
 $=k\cdot(\Phi(e_1),\Phi(e_2),\cdots,\Phi(e_n))$  
  
 $=k\cdot((e_1,e_2,\cdots,e_n)\cdot A)$  
  
 $=(e_1,e_2,\cdots,e_n)(k\cdot A)$  
