**内容**  
设 $\Phi$ 是 $V$ 到 $U$ 的线性映射， $\Psi$ 是 $U$ 到 $W$ 的线性映射  
 $(e_1,\cdots,e_n)$ 是 $V_K^n$ 的一个基，  
 $(f_1,\cdots,f_m)$ 是 $U_K^m$ 的一个基，  
 $(g_1,\cdots,g_p)$ 是 $W_K^p$ 的一个基，  
 $\Phi$ 在上述基下的表示矩阵为 $A_{m\times n}$ ，  
 $\Psi$ 在上述基下的表示矩阵为 $B_{p\times m}$ ，  
则 $(\Psi\circ\Phi)$ 在上述基下的表示矩阵为 $B\cdot A$  
  
**证明**  
 $(\Psi\circ\Phi)(e_i),\ 1\le i\le n$  
  
 $=\Psi(\Phi(e_i))$  
  
 $=\Psi((a_{1i}f_1+a_{2i}f_2+\cdots+a_{mi}f_m))$  
  
 $=a_{1i}\cdot\Psi(f_1)+a_{2i}\cdot\Psi(f_2)+\cdots+a_{mi}\cdot\Psi(f_m)$  
  
 $=a_{1i}\cdot\sum\limits_{j=1}^pb_{j1}\cdot g_j+a_{2i}\cdot\sum\limits_{j=1}^pb_{j2}\cdot g_j+\cdots+a_{mi}\cdot\sum\limits_{j=1}^pb_{jm}\cdot g_j$  
  
 $=\sum\limits_{j=1}^pa_{1i}\cdot b_{j1}\cdot g_j+\sum\limits_{j=1}^pa_{2i}\cdot b_{j2}\cdot g_j+\cdots+\sum\limits_{j=1}^pa_{mi}\cdot b_{jm}\cdot g_j$  
  
 $=\sum\limits_{j=1}^p(a_{1i}\cdot b_{j1}+a_{2i}\cdot b_{j2}+a_{mi}\cdot b_{jm})\cdot g_j$  
  
 $=(a_{1i}\cdot b_{11}+a_{2i}\cdot b_{12}+a_{mi}\cdot b_{1m})\cdot g_1+(a_{1i}\cdot b_{21}+a_{2i}\cdot b_{22}+a_{mi}\cdot b_{2m})\cdot g_2+\cdots+(a_{1i}\cdot b_{p1}+a_{2i}\cdot b_{p2}+a_{mi}\cdot b_{pm})\cdot g_p$  
  
 $=(g_1,g_2,\cdots,g_p)\cdot [B\cdot (a_{1i},a_{2i},\cdots,a_{mi})^T]$  
  
 $\Rightarrow(\Psi\circ\Phi)(e_i)=(g_1,g_2,\cdots,g_p)\cdot [B\cdot (a_{1i},a_{2i},\cdots,a_{mi})^T]$  
  
---  
  
丘版给的条件是 $\Phi,\Psi\in\rm{Hom}(V)$  
  
 $(\ (\Psi\circ\Phi)(e_1),(\Psi\circ\Phi)(e_2),\cdots,(\Psi\circ\Phi)(e_n)\ )$  
  
 $=(\ \Psi(\Phi(e_1)),\Psi(\Phi(e_2)),\cdots,\Psi(\Phi(e_n))\ )$  
  
 $=\Psi(\ \Phi(e_1),\Phi(e_2),\cdots,\Phi(e_n)\ )$  
  
 $=\Psi(\ (e_1,e_2,\cdots,e_n)\cdot A\ )$  
  
 $=\Psi\left(\ \sum\limits_{i=1}^na_{i1}\cdot e_i,\ \sum\limits_{i=1}^na_{i2}\cdot e_i,\ \cdots,\ \sum\limits_{i=1}^na_{in}\cdot e_i\ \right)$  
  
 $=\left(\ \Psi\left(\sum\limits_{i=1}^na_{i1}\cdot e_i\right),\ \Psi\left(\sum\limits_{i=1}^na_{i2}\cdot e_i\right),\ \cdots,\ \Psi\left(\sum\limits_{i=1}^na_{in}\cdot e_i\right)\ \right)$  
  
 $=\left(\ \sum\limits_{i=1}^na_{i1}\cdot\Psi(e_i),\ \sum\limits_{i=1}^na_{i2}\cdot\Psi(e_i),\ \cdots,\ \sum\limits_{i=1}^na_{in}\cdot\Psi(e_i)\ \right)$  
  
 $=\left(\ \sum\limits_{i=1}^na_{i1}\cdot\sum\limits_{j=1}^nb_{j1}e_j,\ \sum\limits_{i=1}^na_{i2}\cdot\sum\limits_{j=1}^nb_{j2}e_j,\ \cdots,\ \sum\limits_{i=1}^na_{in}\cdot\sum\limits_{j=1}^nb_{jn}e_j\ \right)$  
  
(推不下去了)  
