**内容**  
$x_n>0$  
  
$\lim\limits_{n\to\infty}{x_n}=l\iff\lim\limits_{n\to\infty}\sqrt[n]{\prod\limits_{k=1}^nx_k}=l$  
  
**证法1: stolz定理**  
$\lim\limits_{n\to\infty}\sqrt[n]{\prod\limits_{k=1}^nx_k}$  
  
$=\lim\limits_{n\to\infty}e^{\dfrac{\ln{\prod\limits_{k=1}^nx_k}}n}$  
  
$=\lim\limits_{n\to\infty}e^{\dfrac{\ln{x_1}+\ln{x_2}+\ln{x_3}+\cdots+\ln{x_n}}{n}}$  
  
$=e^{\lim\limits_{n\to\infty}{\dfrac{\ln{x_1}+\ln{x_2}+\ln{x_3}+\cdots+\ln{x_n}}{n}}}$  
  
---  
  
$\lim\limits_{n\to\infty}{\dfrac{\ln{x_1}+\ln{x_2}+\ln{x_3}+\cdots+\ln{x_n}}{n}}$  
  
$u_n=\ln{x_1}+\ln{x_2}+\ln{x_3}+\cdots+\ln{x_n},\;v_n=n$  
  
$\Rightarrow\lim\limits_{n\to\infty}\dfrac{u_n}{v_n}=\lim\limits_{n\to\infty}\dfrac{u_n-u_{n-1}}{v_n-v_{n-1}}=\lim\limits_{n\to\infty}\dfrac{\ln x_n}1$  
  
---  
  
$e^{\lim\limits_{n\to\infty}\dfrac{\ln x_n}1}$  
  
$=\lim\limits_{n\to\infty}e^{\ln x_n}$  
  
$=\lim\limits_{n\to\infty}x_n$  
  
**证法2: 夹逼定理**  
$a>0$  
  
$\lim\limits_{n\to\infty}a_n=a>0$  
  
$\Rightarrow \lim\limits_{n\to\infty}\dfrac{a_1+a_2+a_3+\cdots+a_n}n=a$  
  
$\Rightarrow \lim\limits_{n\to\infty}\dfrac1{a_n}=a$  
  
$\Rightarrow \lim\limits_{n\to\infty}\dfrac{n}{\dfrac1{a_1}+\dfrac1{a_2}+\dfrac1{a_3}+\cdots+\dfrac1{a_n}}=\lim\limits_{n\to\infty}\dfrac1{\dfrac{\dfrac1{a_1}+\dfrac1{a_2}+\dfrac1{a_3}+\cdots+\dfrac1{a_n}}{n}}=\dfrac1{\dfrac1a}=a$  
  
$\dfrac{a_1+a_2+a_3+\cdots+a_n}n\geq\sqrt[n]{a_1\cdot a_2\cdot a_3\cdots a_n}\geq\dfrac{n}{\dfrac1{a_1}+\dfrac1{a_2}+\dfrac1{a_3}+\cdots+\dfrac1{a_n}}$  
  
$\Rightarrow\lim\limits_{n\to\infty}\sqrt[n]{a_1\cdot a_2\cdot a_3\cdots a_n}=a$  
  
---  
  
$a=0$  
  
$\dfrac{a_1+a_2+a_3+\cdots+a_n}n\geq\sqrt[n]{a_1\cdot a_2\cdot a_3\cdots a_n}>0$  
