**内容**  
$A\cdot x+B\cdot  y+C=0$  
  
该方程表示的几何图形是直线，任意直线都可以由形如上式的方程表出，(<font color=red>但是并不是只能由上述形式的方程表出</font>)  
  
**证明**  
$\dfrac{y-y_0}{x-x_0}=\dfrac{y_1-y_0}{x_1-x_0}$  
  
$\Rightarrow y-y_0=\dfrac{y_1-y_0}{x_1-x_0}\cdot(x-x_0)$  
  
$\Rightarrow (y-y_0)\cdot(x_1-x_0)=(y_1-y_0)\cdot(x-x_0)$  
  
$\Rightarrow(x_1-x_0)\cdot y-y_0\cdot(x_1-x_0)=(y_1-y_0)\cdot x-(y_1-y_0)\cdot x_0$  
  
$\Rightarrow(y_1-y_0)\cdot x-(x_1-x_0)\cdot y+x_1\cdot y_0-x_0\cdot y_1=0$  
  
$\rm{let}\;A=y_1-y_0,\;B=-(x_1-x_0),\;C=x_1\cdot y_0-x_0\cdot y_1$  
  
$\Rightarrow A\cdot x+B\cdot  y+C=0$  
  
$\Rightarrow k=-\dfrac AB$  
