**内容**  
$a\sin\alpha+b\cos\alpha=\sqrt{a^2+b^2}\cdot\sin(\alpha+\varphi),\ \tan\varphi=\dfrac ba$  
  
$a\sin\alpha+b\cos\alpha=\sqrt{a^2+b^2}\cdot\cos(\alpha-\varphi),\ \tan\varphi=\dfrac ab$  
  
**证明**  
$a\sin\alpha+b\cos\alpha$  
  
$=\sqrt{a^2+b^2}\cdot\left(\dfrac{a}{\sqrt{a^2+b^2}}\cdot\sin\alpha+\dfrac{b}{\sqrt{a^2+b^2}}\cdot\cos\alpha\right)$  
  
令 $\cos\varphi=\dfrac{a}{\sqrt{a^2+b^2}}$  
  
$\Rightarrow\sin\varphi=\dfrac{b}{\sqrt{a^2+b^2}}$  
  
$=\sqrt{a^2+b^2}\cdot\left(\cos\varphi\cdot\sin\alpha+\sin\varphi\cdot\cos\alpha\right)$  
  
$=\sqrt{a^2+b^2}\cdot\left(\sin\alpha\cdot\cos\varphi+\cos\alpha\cdot\sin\varphi\right)$  
  
$=\sqrt{a^2+b^2}\cdot\sin(\alpha+\varphi)$  
  
---  
  
令 $\sin\varphi=\dfrac{a}{\sqrt{a^2+b^2}}$  
  
$\Rightarrow\cos\varphi=\dfrac{b}{\sqrt{a^2+b^2}}$  
  
$=\sqrt{a^2+b^2}\cdot\left(\sin\varphi\cdot\sin\alpha+\cos\varphi\cdot\cos\alpha\right)$  
  
$=\sqrt{a^2+b^2}\cdot\left(\cos\varphi\cdot\cos\alpha+\sin\varphi\cdot\sin\alpha\right)$  
  
$=\sqrt{a^2+b^2}\cdot\left(\cos\alpha\cdot\cos\varphi+\sin\alpha\cdot\sin\varphi\right)$  
  
$=\sqrt{a^2+b^2}\cdot\cos(\alpha-\varphi)$  
