**内容**  
证明 $x_n=1+\dfrac1{2^2}+\dfrac1{3^2}+\cdots+\dfrac1{n^2}$ 收敛  
  
**解**  
$x_n=1+\dfrac1{2^2}+\dfrac1{3^2}+\cdots+\dfrac1{n^2}$  
  
$\Rightarrow|x_m-x_n|=x_m-x_n$  
  
$=\dfrac1{(n+1)^2}+\dfrac1{(n+2)^2}+\dfrac1{(n+3)^2}+\cdots+\dfrac1{(m-1)^2}+\dfrac1{m^2}$  
  
$<\dfrac1{n(n+1)}+\dfrac1{(n+1)(n+2)}+\dfrac1{(n+2)(n+3)}+\cdots+\dfrac1{(m-2)(m-1)}+\dfrac1{(m-1)m}$  
  
$=\left(\dfrac1n-\dfrac1{n+1}\right)+\left(\dfrac1{n+1}-\dfrac1{n+2}\right)+\left(\dfrac1{n+2}-\dfrac1{n+3}\right)+\cdots\left(\dfrac1{m-2}-\dfrac1{m-1}\right)+\left(\dfrac1{m-1}-\dfrac1{m}\right)$  
  
$=\dfrac1n-\dfrac1m<\dfrac1n$  
  
$\Rightarrow|x_m-x_n|<\epsilon$  
