**内容：**    
 $-1$ 乘以 $\alpha$ 等于 $\alpha$ 的逆元， $\forall\alpha,(-1)\cdot\alpha=-\alpha$     
    
证明：    
 $(-1)\alpha+\alpha$     
    
 $=(-1)\alpha+(1)\alpha$     
    
 $=[(-1)+(1)]\alpha$  (逆用左分配律)    
    
 $=0\cdot\alpha$     
    
 $=\mathbf{0}$     
    
 $(-1)\cdot\alpha+\alpha+(-\alpha)    
=-\alpha$  (两边同时加上 $-\alpha$ )    
    
 $(-1)\cdot\alpha+[\alpha+(-\alpha)]=-\alpha$  (加法结合律)    
    
 $(-1)\cdot\alpha+\mathbf{0}=-\alpha$     
    
 $(-1)\cdot\alpha=-\alpha$  (零元的性质)    
    
**证法二**    
 $\alpha+(-1)\cdot\alpha$     
 $=1\cdot\alpha+(-1)\cdot\alpha$     
 $=(1-1)\cdot\alpha=\mathbf0$     
    
 $\Rightarrow\alpha+(-1)\cdot\alpha=\mathbf0$     
    
 $\Rightarrow(-1)\cdot\alpha=-\alpha$  (移项)    
