**内容**  
设 $f_1(x)|g(x)$ ， $f_2(x)|g(x)$ ， $(f_1(x),f_2(x))=1$  
则 $f_1(x)f_2(x)|g(x)$  
互素一定有，不互素未必没有  
  
**证明**  
由互素的充要条件( $1=f(x)u(x)+g(x)v(x)$ )得  
 $\exists\ u(x),v(x)$ 使得， $f_1(x)u(x)+f_2(x)v(x)  
=1$  
两边同时乘 $g(x)$ 得  
 $f_1(x)u(x)g(x)+f_2(x)v(x)g(x)=g(x)$  
两边同时除以 $f_1(x)f_2(x)$  
  
 $\Rightarrow\dfrac{f_1(x)u(x)g(x)+f_2(x)v(x)g(x)}{f_1(x)f_2(x)}=\dfrac{g(x)}{f_1(x)f_2(x)}$  
  
 $\Rightarrow\dfrac{f_1(x)u(x)g(x)}{f_1(x)f_2(x)}+\dfrac{f_2(x)v(x)g(x)}{f_1(x)f_2(x)}=\dfrac{g(x)}{f_1(x)f_2(x)}$  
  
 $\Rightarrow\dfrac{u(x)g(x)}{f_2(x)}+\dfrac{v(x)g(x)}{f_1(x)}=\dfrac{g(x)}{f_1(x)f_2(x)}$  
  
又因为 $f_1(x)|g(x)$ ， $f_2(x)|g(x)$  
 $\Rightarrow u(x)p(x)+v(x)q(x)=\dfrac{g(x)}{f_1(x)f_2(x)}$  
 $\Rightarrow g(x)$ 能被 $f_1(x)f_2(x)$ 整除  
