**内容**  
设 $(f_1(x),g(x))=1,\ (f_2(x),g(x))=1$ ，则 $(f_1(x)f_2(x),g(x))=1$  
  
**证明**  
 $(f_1(x),g(x))=1$  
 $\Rightarrow f_1(x)u_1(x)+g(x)v_1(x)=1\ (1)$  
(多项式互素的充要条件)  
  
 $(f_2(x),g(x))=1$  
 $\Rightarrow f_2(x)u_2(x)+g(x)v_2(x)=1\ (2)$  
(多项式互素的充要条件)  
  
 $(1)$ 式乘以 $(2)$ 式  
 $\Rightarrow f_1(x)f_2(x)u_1(x)u_2(x)$  
 $+g(x)[f_2(x)v_1(x)u_2(x)+f_1(x)u_1(x)v_2(x)$  
 $+g(x)u_1(x)v_2(x)]=1$  
令 $[f_2(x)v_1(x)u_2(x)+f_1(x)u_1(x)v_2(x)$  
 $+g(x)u_1(x)v_2(x)]=l(x)$  
 $\Rightarrow [f_1(x)f_2(x)]\cdot[u_1(x)u_2(x)]+g(x)l(x)=1$  
(多项式互素的充要条件)  
 $\Rightarrow(f_1(x)f_2(x),g(x))=1$  
