**例**  
  
$|A|=\begin{vmatrix}  
x&a_1&a_2&\cdots&a_{n-1}&a_n\\\  
a_1&x&a_2&\cdots&a_{n-1}&a_n\\\  
\vdots&\vdots&\vdots&\ddots&\vdots&\vdots\\\  
a_1&a_2&a_3&\cdots&x&a_n\\\  
a_1&a_2&a_3&\cdots&a_n&x  
\end{vmatrix}$  
  
解：  
  
$|A|=\underset{每列元素都加到第1列}{\underline{\begin{vmatrix}  
x+\sum\limits_{i=1}^na_i  
&a_1&a_2&\cdots&a_{n-1}&a_n\\\  
x+\sum\limits_{i=1}^na_i  
&x&a_2&\cdots&a_{n-1}&a_n\\\  
\vdots&\vdots&\vdots&\ddots&\vdots&\vdots\\\  
x+\sum\limits_{i=1}^na_i  
&a_2&a_3&\cdots&x&a_n\\\  
x+\sum\limits_{i=1}^na_i  
&a_2&a_3&\cdots&a_n&x  
\end{vmatrix}}}$  
  
$=\left(x+\sum\limits_{i=1}^na_i\right)  
\cdot\begin{vmatrix}  
1&a_1&a_2&\cdots&a_{n-1}&a_n\\\  
1&x&a_2&\cdots&a_{n-1}&a_n\\\  
\vdots&\vdots&\vdots&\ddots&\vdots&\vdots\\\  
1&a_2&a_3&\cdots&x&a_n\\\  
1&a_2&a_3&\cdots&a_n&x  
\end{vmatrix}$  
  
第1列乘 $-a_1$ ，加到第2列  
第1列乘 $-a_2$ ，加到第3列  
$\cdots$  
第1列乘 $-a_n$ ，加到第 $n$ 列  
  
  
$=\left(x+\sum\limits_{i=1}^na_i\right)  
\cdot\begin{vmatrix}  
1&0&0&\cdots&0\\\  
1&x-a_1&0&\cdots&0\\\  
1&a_2-a_1&x-a_2&\cdots&0\\\  
\vdots&\vdots&\vdots&\ddots&\vdots\\\  
1&a_2-a_1&a_3-a_2&\cdots&x-a_n  
\end{vmatrix}$  
  
$=\left(x+\sum\limits_{i=1}^na_i\right)  
\cdot\prod\limits_{i=1}^n(x-a_i)$  
