**内容**  
$\limsup\limits_{n\to\infty}(x_n+y_n)\leq\limsup\limits_{n\to\infty}x_n+\limsup\limits_{n\to\infty}y_n$  
  
$\liminf\limits\limits_{n\to\infty}(x_n+y_n)\geq\liminf\limits\limits_{n\to\infty}x_n+\liminf\limits\limits_{n\to\infty}y_n$  
  
**证明: 上极限**  
$\limsup\limits_{n\to\infty}x_n=H_1,\;\limsup\limits_{n\to\infty}y_n=H_2$  
  
$\Rightarrow\forall\;\epsilon>0,\;\exists\;N_1,\;n>N_1,\;x_n<H_1+\epsilon$  
  
$\Rightarrow\forall\;\epsilon>0,\;\exists\;N_2,\;n>N_2,\;y_n<H_2+\epsilon$  
  
$N=\max\{N_1,N_2\}$  
  
$\Rightarrow\forall\;\epsilon>0,\;\exists\;N,\;n>N,\;x_n<H_1+\epsilon,\;y_n<H_2+\epsilon$  
  
$\Rightarrow\forall\;\epsilon>0,\;\exists\;N,\;n>N,\;x_n+y_n<H_1+H_2+2\epsilon$  
  
$\Rightarrow\forall\;\lim\limits_{n\to\infty}(x_{n_k}+y_{n_k})\leq H_1+H_2+2\epsilon$  
  
$\Rightarrow\limsup\limits_{n\to\infty}(x_n+y_n)\leq H_1+H_2+2\epsilon$  
  
$\Rightarrow\limsup\limits_{n\to\infty}(x_n+y_n)\leq\limsup\limits_{n\to\infty}x_n+\limsup\limits_{n\to\infty}y_n\;(\epsilon\to0)$  
  
**证明: 下极限**  
$\liminf\limits\limits_{n\to\infty}x_n=h_1,\;\liminf\limits\limits_{n\to\infty}y_n=h_2$  
  
$\Rightarrow\forall\;\epsilon>0,\;\exists\;N_1,\;n>N_1,\;x_n>h_1-\epsilon$  
  
$\Rightarrow\forall\;\epsilon>0,\;\exists\;N_2,\;n>N_2,\;y_n>h_2-\epsilon$  
  
$N=\max\{N_1,N_2\}$  
  
$\Rightarrow\forall\;\epsilon>0,\;\exists\;N,\;n>N,\;x_n>h_1-\epsilon,\;y_n>h_2-\epsilon$  
  
$\Rightarrow\forall\;\epsilon>0,\;\exists\;N,\;n>N,\;x_n+y_n>h_1+h_2-2\epsilon$  
  
$\Rightarrow\forall\;\lim\limits_{n\to\infty}(x_{n_k}+y_{n_k})\geq h_1+h_2-2\epsilon$  
  
$\Rightarrow\liminf\limits\limits_{n\to\infty}(x_n+y_n)\geq h_1+h_2-2\epsilon$  
  
$\Rightarrow\liminf\limits\limits_{n\to\infty}(x_n+y_n)\geq\liminf\limits\limits_{n\to\infty}x_n+\liminf\limits\limits_{n\to\infty}y_n\;(\epsilon\to0)$  
  
**反例(不可加)**  
$x_n=(-1)^n,\;y_n=(-1)^{n+1}$  
  
$\Rightarrow\limsup\limits_{n\to\infty}x_n=1,\;\limsup\limits_{n\to\infty}y_n=1$  
  
$\Rightarrow\limsup\limits_{n\to\infty}(x_n-y_n)=0$  
