**内容1**  
$\lim\limits_{n\to\infty}x_n=a$  
  
$\Rightarrow\limsup\limits_{n\to\infty}(x_n+y_n)=\lim\limits_{n\to\infty}x_n+\limsup\limits_{n\to\infty}y_n$  
  
**内容2**  
$\lim\limits_{n\to\infty}x_n=a$  
  
$\Rightarrow\liminf\limits_{n\to\infty}(x_n+y_n)=\lim\limits_{n\to\infty}x_n+\liminf\limits_{n\to\infty}y_n$  
  
**证明: 上极限**  
$\limsup\limits_{n\to\infty}y_n$  
  
$=\limsup\limits_{n\to\infty}(x_n+y_n-x_n)$  
  
$=\limsup\limits_{n\to\infty}[(x_n+y_n)-x_n]$  
  
$\leq\limsup\limits_{n\to\infty}(x_n+y_n)-\limsup\limits_{n\to\infty}x_n$  
  
$=\limsup\limits_{n\to\infty}(x_n+y_n)-\lim\limits_{n\to\infty}x_n$  
  
$\Rightarrow\limsup\limits_{n\to\infty}y_n+\lim\limits_{n\to\infty}x_n\leq\limsup\limits_{n\to\infty}(x_n+y_n)$  
  
$\limsup\limits_{n\to\infty}(x_n+y_n)\leq\limsup\limits_{n\to\infty}x_n+\limsup\limits_{n\to\infty}y_n$  
  
$\Rightarrow\limsup\limits_{n\to\infty}(x_n+y_n)\leq\lim\limits_{n\to\infty}x_n+\limsup\limits_{n\to\infty}y_n$  
  
$\limsup\limits_{n\to\infty}y_n+\lim\limits_{n\to\infty}x_n\leq\limsup\limits_{n\to\infty}(x_n+y_n)$  
  
$\limsup\limits_{n\to\infty}(x_n+y_n)\leq\lim\limits_{n\to\infty}x_n+\limsup\limits_{n\to\infty}y_n$  
  
$\Rightarrow\limsup\limits_{n\to\infty}(x_n+y_n)=\lim\limits_{n\to\infty}x_n+\limsup\limits_{n\to\infty}y_n$  
  
**证明: 下极限**  
$\liminf\limits_{n\to\infty}y_n$  
  
$=\liminf\limits_{n\to\infty}(x_n+y_n-x_n)$  
  
$=\liminf\limits_{n\to\infty}[(x_n+y_n)-x_n]$  
  
$\geq\liminf\limits_{n\to\infty}(x_n+y_n)-\liminf\limits_{n\to\infty}x_n$  
  
$=\liminf\limits_{n\to\infty}(x_n+y_n)-\lim\limits_{n\to\infty}x_n$  
  
$\Rightarrow\liminf\limits_{n\to\infty}y_n+\lim\limits_{n\to\infty}x_n\geq\liminf\limits_{n\to\infty}(x_n+y_n)$  
  
$\liminf\limits_{n\to\infty}(x_n+y_n)\geq\liminf\limits_{n\to\infty}x_n+\liminf\limits_{n\to\infty}y_n$  
  
$\Rightarrow\liminf\limits_{n\to\infty}(x_n+y_n)\geq\lim\limits_{n\to\infty}x_n+\liminf\limits_{n\to\infty}y_n$  
  
$\liminf\limits_{n\to\infty}y_n+\lim\limits_{n\to\infty}x_n\leq\liminf\limits_{n\to\infty}(x_n+y_n)$  
  
$\liminf\limits_{n\to\infty}(x_n+y_n)\leq\lim\limits_{n\to\infty}x_n+\liminf\limits_{n\to\infty}y_n$  
  
$\Rightarrow\liminf\limits_{n\to\infty}(x_n+y_n)=\lim\limits_{n\to\infty}x_n+\liminf\limits_{n\to\infty}y_n$  
