**内容1**
$x_n\geq0,\;y_n\geq0$

$\Rightarrow\limsup\limits_{n\to\infty}(x_n\cdot y_n)\leq\limsup\limits_{n\to\infty}x_n\cdot\limsup\limits_{n\to\infty}y_n$

**内容2**
$x_n\geq0,\;y_n\geq0$

$\Rightarrow\liminf\limits_{n\to\infty}(x_n\cdot y_n)\geq\liminf\limits_{n\to\infty}x_n\cdot\liminf\limits_{n\to\infty}y_n$

**证明: 上极限**
$\limsup\limits_{n\to\infty}x_n=H_1$

$\Rightarrow\forall\;\epsilon>0,\;\exists\;N_1>0,\;n>N_1,\;0<x_n<H_1+\epsilon$

$\limsup\limits_{n\to\infty}y_n=H_2$

$\Rightarrow\forall\;\epsilon>0,\;\exists\;N_2>0,\;n>N_2,\;0<y_n<H_2+\epsilon$

$N=\max\{N_1,N_2\}$

$\Rightarrow\forall\;\epsilon>0,\;\exists\;N>0,\;n>N,\;0<x_n<H_1+\epsilon,\;0<y_n<H_2+\epsilon$

$\Rightarrow\forall\;\lim\limits_{n\to\infty}(x_{n_k}\cdot y_{n_k})<(H_1+\epsilon)(H_2+\epsilon)$

$\Rightarrow\limsup\limits_{n\to\infty}(x_n\cdot y_n)<(H_1+\epsilon)(H_2+\epsilon)$

$\epsilon\to0$

$\Rightarrow\limsup\limits_{n\to\infty}(x_n\cdot y_n)\leq\limsup\limits_{n\to\infty}x_n\cdot\limsup\limits_{n\to\infty}y_n$

**证明: 下极限**
$\liminf\limits_{n\to\infty}x_n=h_1$

$\Rightarrow\forall\;\epsilon>0,\;\exists\;N_1>0,\;n>N_1,\;x_n>h_1-\epsilon$

$\liminf\limits_{n\to\infty}y_n=h_2$

$\Rightarrow\forall\;\epsilon>0,\;\exists\;N_2>0,\;n>N_2,\;y_n>h_2-\epsilon$

$N=\max\{N_1,N_2\}$

$\Rightarrow\forall\;\epsilon>0,\;\exists\;N>0,\;n>N,\;x_n>h_1-\epsilon,\;0<y_n>h_2-\epsilon$

$\Rightarrow\forall\;\lim\limits_{n\to\infty}(x_{n_k}\cdot y_{n_k})>(h_1-\epsilon)(h_2-\epsilon)$

$\Rightarrow\liminf\limits_{n\to\infty}(x_n\cdot y_n)>(h_1-\epsilon)(h_2-\epsilon)$

$\epsilon\to0$

$\Rightarrow\liminf\limits_{n\to\infty}(x_n\cdot y_n)\geq\liminf\limits_{n\to\infty}x_n\cdot\liminf\limits_{n\to\infty}y_n$

**推论**
$x_n\geq0,\;y_n\geq0$

$\liminf\limits_{n\to\infty}x_n\cdot\liminf\limits_{n\to\infty}y_n\leq\liminf\limits_{n\to\infty}(x_n\cdot y_n)\leq\limsup\limits_{n\to\infty}(x_n\cdot y_n)\leq\limsup\limits_{n\to\infty}x_n\cdot\limsup\limits_{n\to\infty}y_n$
