**内容1-1**
$\lim\limits_{n\to\infty}x_n=\xi>0$

$\limsup\limits_{n\to\infty}(x_n\cdot y_n)=\lim\limits_{n\to\infty}x_n\cdot\limsup\limits_{n\to\infty}y_n$

**内容1-2**
$\lim\limits_{n\to\infty}x_n=\xi>0$

$\liminf\limits_{n\to\infty}(x_n\cdot y_n)=\lim\limits_{n\to\infty}x_n\cdot\liminf\limits_{n\to\infty}y_n$

**内容2-1**
$\lim\limits_{n\to\infty}x_n=\xi<0$

$\limsup\limits_{n\to\infty}(x_n\cdot y_n)=\lim\limits_{n\to\infty}x_n\cdot\liminf\limits_{n\to\infty}y_n$

**内容2-2**
$\lim\limits_{n\to\infty}x_n=\xi<0$

$\liminf\limits_{n\to\infty}(x_n\cdot y_n)=\lim\limits_{n\to\infty}x_n\cdot\limsup\limits_{n\to\infty}y_n$
