**预备1**    
    
此处对映射加法和数乘的定义源自定理： $\mathbb{L}(V,U)$ 是线性空间    
    
**预备2**    
 $T(\Phi)=\begin{cases}    
\Phi(e_1)=a_{11}\cdot f_1+a_{21}\cdot f_2    
+\cdots+a_{m1}\cdot f_m\\\     
\Phi(e_2)=a_{12}\cdot f_1+a_{22}\cdot f_2    
+\cdots+a_{m2}\cdot f_m\\\     
\Phi(e_3)=a_{13}\cdot f_1+a_{23}\cdot f_2    
+\cdots+a_{m3}\cdot f_m\\\     
\cdots\\\     
\Phi(e_n)=a_{1n}\cdot f_1+a_{2n}\cdot f_2    
+\cdots+a_{mn}\cdot f_m    
\end{cases}=A$     
    
 $T(\Psi)=\begin{cases}    
\Psi(e_1)=b_{11}\cdot f_1+b_{21}\cdot f_2    
+\cdots+b_{m1}\cdot f_m\\\     
\Psi(e_2)=b_{12}\cdot f_1+b_{22}\cdot f_2    
+\cdots+b_{m2}\cdot f_m\\\     
\Phi(e_3)=b_{13}\cdot f_1+b_{23}\cdot f_2    
+\cdots+b_{m3}\cdot f_m\\\     
\cdots\\\     
\Psi(e_n)=b_{1n}\cdot f_1+b_{2n}\cdot f_2    
+\cdots+b_{mn}\cdot f_m    
\end{cases}=B$     
    
**证明保持加法**    
设  $T(\Phi)=A，T(\Psi)=B$     
    
 $(\Phi+\Psi)(e_j)$     
    
 $=\Phi(e_j)+\Psi(e_j)$     
    
 $=\sum\limits_{i=1}^ma_{ij}f_i    
+\sum\limits_{i=1}^mb_{ij}f_i$     
    
 $=\sum\limits_{i=1}^m(a_{ij}+b_{ij})f_i$     
    
 $\Rightarrow T(\ (\Phi+\Psi)\ )=$     
 $\begin{cases}    
(\Phi+\Psi)(e_1)=(a_{11}+b_{11})\cdot f_1+(a_{21}+b_{21})\cdot f_2    
+\cdots+(a_{m1}+b_{m1})\cdot f_m\\\     
(\Phi+\Psi)(e_2)=(a_{12}+b_{12})\cdot f_1+(a_{22}+b_{22})\cdot f_2    
+\cdots+(a_{m2}+b_{m2})\cdot f_m\\\     
(\Phi+\Psi)(e_3)=(a_{13}+b_{13})\cdot f_1+(a_{23}+b_{23})\cdot f_2    
+\cdots+(a_{m3}+b_{m3})\cdot f_m\\\     
\cdots\\\     
(\Phi+\Psi)(e_n)=(a_{1n}+b_{1n})\cdot f_1+(a_{2n}+b_{2n})\cdot f_2    
+\cdots+(a_{mn}+b_{mn})\cdot f_m    
\end{cases}$     
 $=C$     
    
 $\Rightarrow T(\ (\Phi+\Psi)(e_j)\ )    
=\lgroup a_{ij}+b_{ij}\rgroup_{m\times n}    
=A+B$     
    
 $\Rightarrow T(\Phi+\Psi)=T(\Phi)+T(\Psi)$     
    
**证明保持数乘**    
 $\forall\ k\in K，(k\cdot\Phi)(e_j)$     
    
 $=k\cdot \Phi(e_j)$     
    
 $=k\cdot\left(\sum\limits_{i=1}^ma_{ij}f_i\right)$     
    
 $=\sum\limits_{i=1}^m(k\cdot a_{ij})f_i$     
    
 $\Rightarrow T(\ (k\cdot\Phi)(e_j)\ )    
=\lgroup k\cdot a_{ij}\rgroup_{m\times n}    
=k\cdot A$     
    
 $\Rightarrow T(\ (k\cdot\Phi)(e_j)\ )    
=k\cdot T(\ (\Phi)(e_j)\ )$     
    
 $\Rightarrow T(\ k\cdot\Phi\ )    
=k\cdot T(\ \Phi\ )$     
    
    
    
