**内容**  
设 $A(\lambda)$ 的非零行列式因子为 $D_1(\lambda),D_2(\lambda),\cdots,D_r(\lambda)$ ，  
则 $\forall\ 1\le i\le r-1,\ D_i(\lambda)\mid D_{i+1}(\lambda)$  
  
**证明**  
任取 $A(\lambda)$ 的第 $i+1$ 阶子式 $M_{i+1}$  
按第1行展开得  
 $\Rightarrow M_{i+1}=a_{11}(\lambda)M_{11}-a_{12}(\lambda)M_{12}+\cdots+(-1)^{i+2}a_{1,i+1}(\lambda)M_{1,i+1}$  
其中的 $M_{11},M_{12},\cdots,M_{1,i+1}$ 都是 $A(\lambda)$ 的第 $i$ 阶子式，是 $M_{i+1}$ 的1阶子式  
  
由 $D_i(\lambda)$ 的定义得  
 $\Rightarrow D_i(\lambda)\mid M_{11},\quad D_i(\lambda)\mid M_{12},\quad \cdots,\quad D_i(\lambda)\mid M_{1,i+1}$  
  
 $\Rightarrow D_i(\lambda)\mid M_{i+1}$ ，即 $D_i(\lambda)$ 是 $A(\lambda)$ 的任意第 $i+1$ 阶子式的因式  
  
 $\Rightarrow D_i(\lambda)$ 是 $A(\lambda)$ 的所有 $i+1$ 阶子式的因式  
  
 $\Rightarrow D_i(\lambda)\mid D_{i+1}(\lambda)$  
