**预备：表示矩阵**
$(\Phi(e_1)，\Phi(e_2),\cdots,\Phi(e_n))=(f_1,f_2,\cdots,f_m)\cdot T(\Phi)$
$(\Phi(f_1)，\Phi(f_2),\cdots,\Phi(f_m))=(g_1,g_2,\cdots,g_p)\cdot T(\Psi)$
$(\Phi\circ\Psi(e_1)，\Phi\circ\Psi(e_2),\cdots,\Phi\circ\Psi(e_n))$
$=(g_1,g_2,\cdots,g_p)\cdot T(\Psi\circ\Phi)$

**证明**
设 $T(\Phi)=A=\lgroup a_{ij}\rgroup_{m\times n}，
T(\Psi)=B=\lgroup b_{ij}\rgroup_{p\times m}$，

要证$\underset{p\times n}{T(\Psi\circ\Phi)}
=\underset{p\times m}{T(\Psi)}
\cdot\underset{m\times n}{T(\Phi)}$，
只要证 $\underset{p\times n}{T(\Psi\circ\Phi)}=B\cdot A$即可

---

$[(\Phi(e_1)，\Phi(e_2)，\cdots，\Phi(e_n)]
=[f_1，f_2，\cdots，f_m]\cdot A\ (1)$

$\Leftrightarrow\Phi(e_j)=[f_1，f_2，\cdots，f_m]\cdot
\begin{bmatrix}
a_{1j}\\\ a_{2j}\\\ \vdots\\\ a_{mj}
\end{bmatrix}
=\sum\limits_{i=1}^ma_{ij}\cdot f_i$

$\Rightarrow\Psi(\Phi(e_j))=
\Psi\left(\sum\limits_{i=1}^ma_{ij}\cdot f_i\right)
=\sum\limits_{i=1}^ma_{ij}\cdot\Psi(f_i)$

$\Rightarrow[\Psi(\Phi(e_1))，\Psi(\Phi(e_2))，
\cdots，\Psi(\Phi(e_n))]$

$=[\Psi(f_1)，\Psi(f_2)，\cdots，\Psi(f_m)]\cdot A\ (2)$
观察$(1)$与$(2)$，发现$A$没有变，因为线性映射保持线性组合

---

又因为$[\Psi(f_1)，\Psi(f_2)，\cdots，\Psi(f_m)]$
$=(g_1,g_2,\cdots,g_p)\cdot B$

$\Rightarrow[\Psi(\Phi(e_1))，\Psi(\Phi(e_2))，
\cdots，\Psi(\Phi(e_n))]$

$=(g_1,g_2,\cdots,g_p)\cdot B\cdot A$

$\Rightarrow
\underset{p\times n}{T(\Psi\circ\Phi)}
=B\cdot A
=\underset{p\times m}{T(\Psi)}
\cdot\underset{m\times n}{T(\Phi)}$

