$D_n=\begin{vmatrix}
5&3&0&\cdots&0&0\\\ 
2&5&3&\cdots&0&0\\\ 
0&2&5&\cdots&0&0\\\ 
0&0&0&\cdots&5&3\\\ 
0&0&0&\cdots&2&5
\end{vmatrix}$

按第$n$列展开
$=5\cdot(-1)^{2n}\cdot D_{n-1}$

$+3\cdot(-1)^{n-1+n}\cdot
\begin{vmatrix}
5&3&\cdots&0&0&0\\\ 
2&5&\cdots&0&0&0\\\ 
0&0&\cdots&5&3&0\\\ 
\vdots&\vdots&\ddots&\vdots&\vdots&\vdots\\\ 
0&0&\cdots&2&5&3\\\ 
0&0&\cdots&0&0&2
\end{vmatrix}$

按第$n-1$行展开
$=5\cdot(-1)^{2n}\cdot D_{n-1}$

$+3\cdot(-1)^{n-1+n}\cdot2\cdot(-1)^{2(n-1)}
\cdot\begin{vmatrix}
5&3&\cdots&0&0\\\ 
2&5&\cdots&0&0\\\ 
0&0&\cdots&5&3\\\ 
\vdots&\vdots&\ddots&\vdots&\vdots\\\ 
0&0&\cdots&2&5
\end{vmatrix}$

$=5D_{n-1}-6D_{n-2}$

$\Rightarrow D_n=5D_{n-1}-6D_{n-2}$

---
$\Rightarrow D_n-2D_{n-1}=3(D_{n-1}-2D_{n-2})$

$\Rightarrow 
D_{n-1}-2D_{n-2}=3(D_{n-2}-2D_{n-3})$

$\Rightarrow 
D_{n-2}-2D_{n-3}=3(D_{n-3}-2D_{n-4})$

$\Rightarrow 
D_{n-1}-2D_{n-2}=3(D_{n-1}-2D_{n-2})$

$\quad\quad\quad\quad\quad\quad\quad\quad
=3^2\cdot(D_{n-2}-2D_{n-3})$

$\quad\quad\quad\quad\quad\quad\quad\quad
=3^3\cdot(D_{n-3}-2D_{n-4})$

$\quad\quad\quad\quad\quad\quad\quad\quad
\cdots$

$\quad\quad\quad\quad\quad\quad\quad\quad
=3^{n-2}\cdot(D_2-2D_1)$


又因为$D_1=5，D_2=19$
$\Rightarrow D_{n}-2D_{n-1}=3^n$

---
$\Rightarrow D_n-3D_{n-1}
=2D_{n-1}-6D_{n-2}
=2(D_{n-1}-3D_{n-2})$

$=2^2\cdot(D_{n-2}-3D_{n-3})$

$=2^3\cdot(D_{n-3}-3D_{n-4})$

$\cdots$

$=2^{n-2}\cdot(D_2-3D_1)=2^n$

---
$\Rightarrow\begin{cases}
D_{n}-2D_{n-1}=3^n&\\\ 
D_{n}-3D_{n-1}=2^n
\end{cases}$

$\Rightarrow D_n=3^{n+1}-2^{n+1}$
