**求行列式**  
$M=\begin{bmatrix}  
a_1^2&a_1a_2+1&a_1a_3+1&\cdots&a_1a_n+1\\\  
a_2a_1+1&a_2^2&a_2a_3+1&\cdots&a_2a_n+1\\\  
a_3a_1+1&a_3a_2+1&a_3^2&\cdots&a_3a_n+1\\\  
\vdots&\vdots&\vdots&\ddots&\vdots\\\  
a_na_1+1&a_na_2+1&a_na_3+1&\cdots&a_n^2  
\end{bmatrix}$  
  
观察： $i\neq j,(i,j):a_ia_j+1；i=j,(i,i):a_i^2$  
  
**解**  
**1 矩阵分解：整体化成乘积形式**  
  
$M=$  
  
$\begin{bmatrix}  
a_1^2+1&a_1a_2+1&a_1a_3+1&\cdots&a_1a_n+1\\\  
a_2a_1+1&a_2^2+1&a_2a_3+1&\cdots&a_2a_n+1\\\  
a_3a_1+1&a_3a_2+1&a_3^2+1&\cdots&a_3a_n+1\\\  
\vdots&\vdots&\vdots&\ddots&\vdots\\\  
a_na_1+1&a_na_2+1&a_na_3+1&\cdots&a_n^2+1  
\end{bmatrix}$  
  
$-\begin{bmatrix}  
-1&0&0&\cdots&0\\\  
0&-1&0&\cdots&0\\\  
0&0&-1&\cdots&0\\\  
\vdots&\vdots&\vdots&\ddots&\vdots\\\  
0&0&0&\cdots&-1  
\end{bmatrix}$  
  
$=-E_n+(a_ia_j+1)_{n\times n}$  
  
$=-E_n+\underset{n\times 2}{\begin{bmatrix}  
a_1&1\\\  
a_2&1\\\  
a_3&1\\\  
\vdots&\vdots\\\  
a_n&1  
\end{bmatrix}}  
\cdot\underset{n\times 2}{\begin{bmatrix}  
a_1&a_2&a_3&\cdots&a_n\\\  
1&1&1&\cdots&1  
\end{bmatrix}}$  
  
$=-E_n-\begin{bmatrix}  
a_1&1\\\  
a_2&1\\\  
a_3&1\\\  
\vdots&\vdots\\\  
a_n&1  
\end{bmatrix}  
\cdot (-E_2)^{-1}  
\cdot\begin{bmatrix}  
a_1&a_2&a_3&\cdots&a_n\\\  
1&1&1&\cdots&1  
\end{bmatrix}$  
  
**2 构造一个 $2n\times 2n$ 的矩阵**  
  
$\begin{bmatrix}  
A=-E_2&B=\begin{bmatrix}  
a_1&a_2&a_3&\cdots&a_n\\\  
1&1&1&\cdots&1  
\end{bmatrix}\\\  
C=\begin{bmatrix}  
a_1&1\\\  
a_2&1\\\  
a_3&1\\\  
\vdots&\vdots\\\  
a_n&1  
\end{bmatrix}&D=-E_n  
\end{bmatrix}$  
  
<font color=brown>注意到其中A，D均可逆</font>  
$\Rightarrow$ 满足降阶公式的条件  
  
$\Rightarrow  
|A|\cdot|D-CA^{-1}B|=|D|\cdot|A-BD^{-1}C|$  
  
<font color=red>注意到公式中的 $D-CA^{-1}B$ 就是原矩阵 $M$ </font>，  
令 $D-CA^{-1}B=M$  
$\Rightarrow|M|=|D-CA^{-1}B|$  
$\Rightarrow  
|A|\cdot|M|=|D|\cdot|A-BD^{-1}C|$  
  
$\Rightarrow  
|-E_2|\cdot|M|=|-E_n|\cdot|-E_2-B(-E_n)^{-1}C|$  
  
$=(-1)^n\cdot \begin{bmatrix}  
\sum\limits_{i=1}^na_i^2-1  
&\sum\limits_{i=1}^na_i\\\  
\sum\limits_{i=1}^na_i&n-1\end{bmatrix}$  
  
$\Rightarrow|M|=(-1)^n\cdot \begin{bmatrix}  
\sum\limits_{i=1}^na_i^2-1  
&\sum\limits_{i=1}^na_i\\\  
\sum\limits_{i=1}^na_i&n-1\end{bmatrix}$  
  
$=(-1)^n\cdot\left[\left(\sum\limits_{i=1}^na_i^2-1\right)(n-1)-\left(\sum\limits_{i=1}^na_i\right)^2\right]$  
