**条件**    
 $\begin{array}{ccc}    
V_K^n&\xrightarrow{\Phi}&U_K^m\\\     
\eta_v\downarrow&&\downarrow\eta_u\\\     
K^n&\xrightarrow{\Phi_A}&K^m    
\end{array}$     
    
**结论**    
 $\eta_u\circ\Phi=\Phi_A\circ\eta_v$     
    
**证明**    
起点 $\to$ 右 $\to$ 下： $V_K^n\to U_K^m\to K^m$     
 $(\eta_u\circ\Phi)(\alpha)$     
    
 $=\eta_u(\ \Phi(\alpha)\ )$     
    
 $=\eta_u(\beta)=\begin{bmatrix}\mu_1\\\ \mu_2\\\ \vdots\\\ \mu_m\end{bmatrix}$     
    
---    
起点 $\to$ 下 $\to$ 右： $V_K^n\to K^n\to K^m$     
    
 $(\Phi_A\circ\eta_v)(\alpha)$     
    
 $=\Phi_A(\ \eta_v(\alpha)\ )$     
    
 $=\Phi_A(\begin{bmatrix}\lambda_1\\ \lambda_2\\\ \vdots\\\ \lambda_n\end{bmatrix})$     
    
 $=\begin{bmatrix}\lambda_1\\ \lambda_2\\\ \vdots\\\ \lambda_n\end{bmatrix}\cdot A$     
    
---    
    
又因为**坐标向量与表示矩阵**    
 $\begin{bmatrix}\mu_1\\\ \mu_2\\\ \vdots\\\ \mu_m\end{bmatrix}=A\cdot\begin{bmatrix}\lambda_1\\\ \lambda_2\\\ \vdots\\\ \lambda_n\end{bmatrix}$     
    
 $\Rightarrow    
\eta_u\circ\Phi=\Phi_A\circ\eta_v$     
    
