**证明**
$\alpha=(e_1,e_2,\cdots,e_n)\cdot
(\lambda_1,\lambda_2,\cdots,\lambda_n)^T$ (矩阵乘法)

$=(f_1,f_2,\cdots,f_n)\cdot
(\mu_1,\mu_2,\cdots,\mu_n)^T$ (矩阵乘法)

$=(e_1,e_2,\cdots,e_n)\cdot A\cdot
(\mu_1,\mu_2,\cdots,\mu_n)^T$

$\Rightarrow(e_1,e_2,\cdots,e_n)\cdot
(\lambda_1,\lambda_2,\cdots,\lambda_n)^T$
$=(e_1,e_2,\cdots,e_n)\cdot A\cdot
(\mu_1,\mu_2,\cdots,\mu_n)^T$

$\overset{由引理得}\Longrightarrow
\underset{n\times 1}
{(\lambda_1,\lambda_2,\cdots,\lambda_n)^T}
=\underset{n\times n}A\cdot
\underset{n\times 1}{
(\mu_1,\mu_2,\cdots,\mu_n)^T}$



