**证明**  
<font color=brown>Part1</font>  
令 $g(x)=\rm{lcm}(m_1(x),\cdots,m_k(x))$  
$\Rightarrow m_i(x)\mid g(x)$  
$\Rightarrow g(x)=m_i(x)q_i(x)$  
又因为 $m_i(A_i)=$ 零矩阵  
$\Rightarrow g(A_i)=$ 零矩阵  
  
又因为 $g(A)=\begin{bmatrix}  
g(A_1)&&\\\  
&g(A_2)&\\\  
&&\ddots\\\  
&&&g(A_k)  
\end{bmatrix}$  
  
$\Rightarrow g(A)=$ 零矩阵  
  
$\Rightarrow g(x)$ 是 $A$ 的极小适合多项式  
  
$\Rightarrow m(x)\mid g(x)$  
  
<font color=brown>Part2</font>  
再证明 $g(x)\mid m(x)$  
零矩阵 $=m(A)=\begin{bmatrix}  
m(A_1)&&\\\  
&m(A_2)&\\\  
&&\ddots\\\  
&&&m(A_k)  
\end{bmatrix}$  
$\Rightarrow m(A_i)=$ 零矩阵  
$\Rightarrow m_i(x)\mid m(x)$  
$\Rightarrow m(x)$ 是 $m_1(x),m_2(x),\cdots,m_k(x)$ 的公倍式  
$\Rightarrow g(x)\mid m(x)$  
  
$\Rightarrow m(x)$ 与 $g(x)$ 相差一个非零常数，即 $m(x)$ 与 $g(x)$ 相伴  
$\Rightarrow m(x)=c g(x)$  
  
由因为都是首一的  
$\Rightarrow c=1$  
$\Rightarrow m(x)=g(x)$  
