**证明V2**  
<font color=blue>Part1</font>  
令 $g(x)=\rm{lcm}(m_1(x),\cdots,m_k(x))$  
$\Rightarrow m_i(x)\mid g(x)$  
$\Rightarrow g(x)=m_i(x)q_i(x)$  
$\Rightarrow g(A_i)=m_i(A_i)q_i(A_i)$  
$\Rightarrow g(A_i)=$ 零矩阵  
  
<font color=blue>Part2</font>  
$g(A)=\begin{bmatrix}  
g(A_1)&&\\\  
&g(A_2)&\\\  
&&\ddots\\\  
&&&g(A_k)  
\end{bmatrix}$  
  
<font color=blue>Part3</font>  
Part1+Part2  
$\Rightarrow g(A)=$ 零矩阵  
$\Rightarrow g(x)=\rm{lcm}(m_1(x),\cdots,m_k(x))$ 是 $A$ 的适合多项式  
$\Rightarrow m(x)\mid g(x)$  
  
<font color=blue>Part4</font>  
$m(A)=\begin{bmatrix}  
m(A_1)&&\\\  
&m(A_2)&\\\  
&&\ddots\\\  
&&&m(A_k)  
\end{bmatrix}=$ 零矩阵  
$\Rightarrow m(x)$ 是 $A_1,A_2,\cdots,A_k$ 的适合多项式  
$\Rightarrow m_i(x)\mid m(x)$  
$\Rightarrow m(x)$ 是 $m_1(x),m_2(x),\cdots,m_k(x)$ 的公倍式  
  
<font color=blue>Part5</font>  
$m(x)$ 是 $m_1(x),m_2(x),\cdots,m_k(x)$ 的公倍式  
$g(x)=\rm{lcm}(m_1(x),\cdots,m_k(x))$  
$\Rightarrow g(x)\mid m(x)$  
  
<font color=blue>Part6</font>  
$\Rightarrow m(x)$ 与 $g(x)$ 相差一个非零常数，即 $m(x)$ 与 $g(x)$ 相伴  
$\Rightarrow m(x)=c g(x)$  
  
又因为都是首一的  
$\Rightarrow c=1$  
$\Rightarrow m(x)=g(x)$  
