**内容**  
$\lim\limits_{n\to+\infty}x_n=a,\;\lim\limits_{n\to+\infty}y_n=b$  
  
$\Rightarrow\alpha\lim\limits_{n\to+\infty}x_n+\beta\lim\limits_{n\to+\infty}y_n$  
  
$=\lim\limits_{n\to+\infty}\alpha x_n+\lim\limits_{n\to+\infty}\beta y_n$  
  
$=\lim\limits_{n\to+\infty}(\alpha x_n+\beta y_n)$  
  
$=\alpha a+\beta b$  
  
**证明思路**  
分析法，要证xxx只要证xxx  
  
**证明**  
$\lim\limits_{n\to+\infty}x_n=a$  
$\Leftrightarrow\forall\;\epsilon>0,\;\exists\;N_1>0,\;n>N_1,\;  
\forall\;x_n,\;|x_n-a|<\epsilon$  
  
$\lim\limits_{n\to+\infty}y_n=b$  
$\Leftrightarrow\forall\;\epsilon>0,\;\exists\;N_2>0,\;n>N_2,\;  
\forall\;y_n,\;|y_n-b|<\epsilon$  
  
$N=\max\{N_1,\;N_2\}$  
$\Rightarrow  
\forall\;\epsilon>0,\;\exists\;N>0,\;n>N,\;  
\forall\;x_n,y_n,\;  
|x_n-a|<\epsilon,\;|y_n-b|<\epsilon$  
  
---  
  
$\Rightarrow  
|(y_n-b)-(x_n-a)|\leq\left| |y_n-b|+|x_n-a| \right|<\epsilon$  
$\quad|(y_n-b)+(x_n-a)|\leq\left| |y_n-b|+|x_n-a| \right|<\epsilon$  
  
$\Rightarrow |(y_n-x_n)-(b-a)|<\epsilon$  
$\quad|(y_n+x_n)-(b+a)|<\epsilon$  
  
---  
  
$|(\alpha x_n+\beta y_n)-(\alpha a+\beta b)|$  
$=|\alpha(x_n-a)-\beta(y_n-b)|$  
$\leq |\alpha(x_n-a)|+|\beta(y_n-b)|$  
$=|\alpha|\,|(x_n-a)|+|\beta|\,|(y_n-b)|$  
$<|\alpha|\epsilon+|\beta|\epsilon$  
$=(|\alpha|+|\beta|)\epsilon$  
  
$\Rightarrow  
|(\alpha x_n+\beta y_n)-(\alpha a+\beta b)|<  
(|\alpha|+|\beta|)\epsilon$  
