**性质1**  
若 $B=P^{-1}\cdot A\cdot P$ ，则 $B^m=P^{-1}\cdot A^m\cdot P$  
  
*推导*  
$B^m=(P^{-1}\cdot A\cdot P)^m$  
$=(P^{-1}\cdot A\cdot P)(P^{-1}\cdot A\cdot P)\cdots(P^{-1}\cdot A\cdot P)(P^{-1}\cdot A\cdot P)$  
$=P^{-1}\cdot A\cdots A\cdot P$  
$=P^{-1}\cdot A^m\cdot P$  
  
**性质2**  
设 $B=P^{-1}\cdot A\cdot P,\ A\in M_n(K),\ f(x)=a_nx^n+a_{n-1}x+\cdots+a_1x+a_0$  
则 $f(B)=P^{-1}\cdot f(A)\cdot P$  
  
*推导*  
$f(A)=a_nA^n+a_{n-1}A+\cdots+a_1A+a_0E_n$  
  
$\Rightarrow f(B)=f(P^{-1}\cdot A\cdot P)$  
  
$=a_n(P^{-1}\cdot A\cdot P)^n+a_{n-1}(P^{-1}\cdot A\cdot P)^{n-1}+\cdots+a_1(P^{-1}\cdot A\cdot P)+a_0(P^{-1}\cdot E_n\cdot P)$  
  
$=a_n(P^{-1}\cdot A^n\cdot P)+a_{n-1}(P^{-1}\cdot A^{n-1}\cdot P)+\cdots+a_1(P^{-1}\cdot A\cdot P)+a_0(P^{-1}\cdot E_n\cdot P)$  
  
$=P^{-1}(a_nA^n+a_{n-1}A+\cdots+a_1A+a_0E_n)P$  
  
$=P^{-1}\cdot f(A)\cdot P$  
  
**性质3**  
若 $B=P^{-1}\cdot A\cdot P$ ，则 $B^{-1}=P^{-1}\cdot A^{-1}\cdot P$  
  
*推导*  
$B^{-1}=(P^{-1}\cdot A\cdot P)^{-1}$  
$=P^{-1}\cdot A^{-1}\cdot P$  
  
**性质4**  
若 $B=P^{-1}\cdot A\cdot P$ ，则 $B^{\star}=P^{\star}\cdot A^{\star}\cdot(P^{\star})^{-1}$  
  
*推导*  
$B^{\star}=(P^{-1}\cdot A\cdot P)^{\star}$  
  
$=P^{\star}\cdot A^{\star}\cdot(P^{-1})^{\star}$  
  
$=P^{\star}\cdot A^{\star}\cdot(P^{\star})^{-1}$  
