**举例**  
$k=3, n=5$  
$\Rightarrow S_3-S_2\cdot\sigma_1+S_1\cdot\sigma_2-k\cdot\sigma_3$  
$=(x_1^3+x_2^3+x_3^3+x_4^3+x_5^3)-(x_1^2+x_2^2+x_3^2+x_4^2+x_5^2)(x_1+x_2+x_3+x_4+x_5)$  
$+(x_1+x_2+x_3+x_4+x_5)\cdot(x_1x_2+x_1x_3+x_1x_4+x_1x_5+x_2x_3+x_2x_4+x_2x_5+x_3x_4+x_3x_5+x_4x_5)$  
$-3\cdot(x_1x_2x_3+x_1x_2x_4+x_1x_2x_5+x_1x_3x_4+x_1x_3x_5+x_1x_4x_5+x_2x_3x_4+x_2x_3x_5+x_2x_4x_5+x_3x_4x_5)$  
$=0$  
  
```  
clc;  
  
syms x_1 x_2 x_3 x_4 x_5;  
  
f_1=(x_1^3+x_2^3+x_3^3+x_4^3+x_5^3)-expand((x_1^2+x_2^2+x_3^2+x_4^2+x_5^2)*(x_1+x_2+x_3+x_4+x_5));  
  
disp(f_1);  
  
f_2=expand((x_1+x_2+x_3+x_4+x_5)*(x_1*x_2+x_1*x_3+x_1*x_4+x_1*x_5+x_2*x_3+x_2*x_4+x_2*x_5+x_3*x_4+x_3*x_5+x_4*x_5));  
  
disp(f_2);  
  
f_3=-3*(x_1*x_2*x_3+x_1*x_2*x_4+x_1*x_2*x_5+x_1*x_3*x_4+x_1*x_3*x_5+x_1*x_4*x_5+x_2*x_3*x_4+x_2*x_3*x_5+x_2*x_4*x_5+x_3*x_4*x_5);  
  
disp(f_3);  
  
disp(f_1+f_2+f_3);  
```  
  
$k=5, n=3$  
$S_5-S_4\sigma_1+S_3\sigma_2-S_2\sigma_3$  
$=(x_1^5+x_2^5+x_3^5)-(x_1^4+x_2^4+x_3^4)(x_1+x_2+x_3)+(x_1^4+x_2^4+x_3^4)(x_1x_2+x_1x_3+x_2x_3)$  
$-(x_1^2+x_2^2+x_3^2)(x_1+x_2+x_3)$  
$=0$  
```  
clc;  
  
syms x_1 x_2 x_3;  
  
f_1 = x_1^5+x_2^5+x_3^5;  
  
f_2=expand((x_1^4+x_2^4+x_3^4)*(x_1+x_2+x_3))+expand((x_1^4+x_2^4+x_3^4)*(x_1x_2+x_1x_3+x_2x_3));  
  
f_3=-expand((x_1^2+x_2^2+x_3^2)*(x_1+x_2+x_3));  
  
disp(f_1+f_2+f_3);  
```  
