**证明**    
<font color=brown>必要性</font>    
 $\Phi:V\rightarrow U$ 是从 $V$ 到 $U$ 的线性映射    
    
 $\Rightarrow$ 保持加法： $\Phi(k\cdot\alpha    
+l\cdot\beta)=\Phi(k\cdot\alpha)    
+\Phi(l\cdot\beta)$     
    
 $\Rightarrow$ 保持数乘： $\Phi(k\cdot\alpha)    
=k\cdot\Phi(\alpha);\ \Phi(l\cdot\beta)    
=l\cdot\Phi(\beta)$     
    
 $\Rightarrow\Phi(k\cdot\alpha+l\cdot\beta)    
=k\cdot\Phi(\alpha)+l\cdot\Phi(\beta)$     
    
<font color=brown>充分性</font>    
令 $k=l=1$     
    
 $\Rightarrow    
\Phi(\alpha+\beta)=\Phi(\alpha)+\Phi(\beta)$     
    
 $\Rightarrow$ 保持加法    
    
令 $l=0$     
    
 $\Rightarrow\Phi(k\cdot\alpha)    
=k\cdot\Phi(\alpha)$     
    
 $\Rightarrow$ 保持数乘    
