**证明**  
由条件 $V=V_1\oplus V_2$ 得  
 $\Rightarrow\rm{dim}_K(V)=\rm{dim}_K(V_1)  
+\rm{dim}_K(V_2)$   
  
不妨设 $V_1$ 的维数为 $r$ ，则 $V_2$ 的维数为 $n-r$   
则可设 $V_1$ 的一个基为 $(e_1,e_2,\cdots,e_r)$ ，  
 $V_2$ 的一个基为 $e_{r+1},\cdots,e_n$   
  
又因为 $V_1,V_2$ 都是 $\Phi$ 下的不变子空间  
 $\Rightarrow\Phi(e_i)\in V_1,\ 1\le i\le r$   
 $\Rightarrow\Phi(e_j)\in V_2,\ r+1\le j\le n$   
  
 $\Rightarrow\begin{cases}  
\Phi(e_1)=a_{11}e_1+a_{21}e_2+\cdots+a_{r1}e_r&\\\  
\Phi(e_2)=a_{12}e_1+a_{22}e_2+\cdots+a_{r2}e_r&\\\  
\cdots\\\  
\Phi(e_r)=a_{1r}e_1+a_{2r}e_2+\cdots+a_{rr}e_r  
\end{cases}$   
  
 $\begin{cases}  
\Phi(e_{r+1})=b_{{r+1},{r+1}}e_{r+1}+b_{{r+2},{r+1}}e_{r+2}+\cdots+b_{n,{r+1}}e_n&\\\  
\Phi(e_{r+2})=b_{{r+1},{r+2}}e_{r+1}+b_{{r+2},{r+2}}e_{r+2}+\cdots+b_{n,{r+2}}e_n&\\\  
\cdots\\\  
\Phi(e_n)=b_{{r+1},n}e_{r+1}+b_{{r+2},n}e_{r+2}+\cdots+b_{n,n}e_n  
\end{cases}$   
  
---  
写出 $\Phi$ 在 $V_K^n$ 上的表示矩阵的结构  
 $(\ \Phi(e_1),\Phi(e_2),\cdots,\Phi(e_r),\Phi(e_{r+1}),\Phi(e_{r+2},\cdots,\Phi(e_n)\ )$   
 $=(e_1,e_2,\cdots,e_r,e_{r+1},\cdots,e_n)\left[\begin{array}{c:c}\ast&\ast\\\  
\ast&\ast\end{array}\right]_n$   
  
根据矩阵乘法定义可以推断出  
 $(\ \underbrace{\Phi(e_1),\Phi(e_2),\cdots,\Phi(e_r)},\underbrace{\Phi(e_{r+1}),\Phi(e_{r+2},\cdots,\Phi(e_n)}\ )$   
 $=(\underbrace{e_1,e_2,\cdots,e_r},\underbrace{e_{r+1},\cdots,e_n})\left[\begin{array}{c:c}A_r&\ast\\\  
\bf{O}&B_{n-r}\end{array}\right]_n$   
