**转置部分**  
  
 $1^\circ\ (A^T)^T=A$  
  
 $2^\circ\ (A\cdot B)^T=B^T\cdot A^T$  
  
 $3^\circ\ (c\cdot A)^=c\cdot A^T$  
  
 $4^\circ\ |A^T|=|A|$  
  
**逆阵部分**  
  
 $1^\circ\ (A^{-1})^{-1}=A$  
  
 $2^\circ\ (AB)^{-1}=B^{-1}\cdot A^{-1}$  
  
 $3^\circ\ (c\cdot A)^{-1}=\frac1c\cdot A^{-1}$  
  
 $4^\circ\ |A^{-1}|=|A|^{-1}$  
  
 $5^\circ\ (A^T)^{-1}=(A^{-1})^T$  
  
 $6^\circ\ $ 可逆矩阵满足乘法消去律和整性  
  
**伴随部分**  
  
 $1^\circ\ A\cdot A^\star=A^\star\cdot A=|A|\cdot E_n$  
  
 $2^\circ\ (A^\star)^\star=  
\begin{cases}  
A&n=2\\\  
|A|^{n-2}\cdot A&n\geq3  
\end{cases}$  
  
 $3^\circ\ (AB)^\star  
=B^\star\cdot A^\star$  
  
 $4^\circ\ (c\cdot A)^\star=c^{n-1}\cdot A^\star$  
  
 $5^\circ\ |A^\star|=|A|^{n-1}$  
  
 $6^\circ\ (A^T)^\star=(A^\star)^T$  
  
 $7^\circ\ (A^{-1})^\star=(A^\star)^{-1}$  
  
