**内容**    
若 $\alpha\perp\beta$ ，则 $\Vert\alpha+\beta\Vert^2=\Vert\alpha\Vert^2+\Vert\beta\Vert^2$     
    
**证明**    
 $\Vert\alpha+\beta\Vert^2$     
    
 $=(\alpha+\beta,\alpha+\beta)$     
    
 $=(\alpha,\alpha+\beta)+(\beta,\alpha+\beta)$     
    
 $=(\alpha,\beta)+(\alpha,\alpha)+(\beta,\alpha)+(\beta,\beta)$     
    
 $=\Vert\alpha\Vert^2+\Vert\beta\Vert^2+(\alpha,\beta)+(\beta,\alpha)$     
    
 $=\Vert\alpha\Vert^2+\Vert\beta\Vert^2+0+0$     
    
 $\Rightarrow\Vert\alpha+\beta\Vert^2=\Vert\alpha\Vert^2+\Vert\beta\Vert^2$     
    
**推广**    
条件是两两正交    
    
 $\Vert\alpha+\beta+\gamma\Vert^2$     
    
 $=(\alpha+\beta+\gamma,\alpha+\beta+\gamma)$     
    
 $=(\alpha,\alpha+\beta+\gamma)+(\beta,\alpha+\beta+\gamma)+(\gamma,\alpha+\beta+\gamma)$     
    
 $=(\alpha,\alpha)+(\alpha,\beta)+(\alpha,\gamma)$     
 $\enspace+(\beta,\alpha)+(\beta,\beta)+(\beta,\gamma)$     
 $\enspace+(\gamma,\alpha)+(\gamma,\beta)+(\gamma,\gamma)$     
    
 $=(\alpha,\alpha)+(\beta,\beta)+(\gamma,\gamma)$     
    
 $=\Vert\alpha\Vert^2+\Vert\beta\Vert^2+\Vert\gamma\Vert^2$     
