**证明**
设$(e_1,e_2,\cdots,e_k)$是$\rm{Ker}(\Phi)$的一个基，将其扩展成全空间$V_K$的一个基$(e_1,e_2,\cdots,e_k,e_{k+1},e_{k+2},\cdots,e_n)$

$\Rightarrow\forall\ \alpha\in V_K,\ \alpha=\sum\limits_{i=1}^n\lambda_ie_i$

$\Rightarrow\Phi(\alpha)
=\lambda_{k+1}\Phi(e_{k+1})+\cdots+
\lambda_n\Phi(e_n)$

又因为$\Phi(\alpha)\in\rm{Im}(\Phi)$

$\Rightarrow\rm{Im}(\Phi)=\rm{L}(\Phi(e_{k+1}),\cdots,\Phi(e_n))$

---

下面证明$\Phi(e_{k+1}),\cdots,\Phi(e_n)$线性无关

设$c_{k+1}\Phi(e_{k+1})+\cdots+
c_n\Phi(e_n)=\bf{0}$

其中$c_{k+1},\cdots,c_n$是待定系数

因为$\Phi$是线性映射

$\Rightarrow\Phi(c_{k+1}e_{k+1}+\cdots+
c_ne_n)=\bf{0}$

$\Rightarrow(c_{k+1}e_{k+1}+\cdots+
c_ne_n)\in\rm{Ker}(\Phi)$

$\Rightarrow(c_{k+1}e_{k+1}+\cdots+
c_ne_n)$可由$(e_1,e_2,\cdots,e_k)$线性表出

$\Rightarrow c_{k+1}e_{k+1}+\cdots+
c_ne_n=-c_1e_1-c_2e_2-\cdots-c_ke_k$

$\Rightarrow  c_1e_1+c_2e_2+\cdots+
c_ke_k+c_{k+1}e_{k+1}+\cdots+c_ne_n=\bf{0}$

又因为$(e_1,e_2,\cdots,e_k,e_{k+1},e_{k+2},\cdots,e_n)$线性无关

$\Rightarrow c_1=c_2=\cdots=c_k=c_{k+1}=\cdots=c_n=0$

$\Rightarrow\Phi(e_{k+1}),\cdots,\Phi(e_n)$线性无关

---
已证$\rm{Im}(\Phi)=\rm{L}(\Phi(e_{k+1}),\cdots,\Phi(e_n))$

又已证$\Phi(e_{k+1}),\cdots,\Phi(e_n)$线性无关

$\Rightarrow(\Phi(e_{k+1}),\cdots,\Phi(e_n))$是$\rm{Im}(\Phi)$的一个基

$\Rightarrow\rm{dim}_K(\rm{Im}(\Phi))=n-k$

又因为$\rm{dim}_K(\rm{Ker}(\Phi))=k$

$\Rightarrow\rm{dim}_K(\rm{Ker}(\Phi))
+\rm{dim}_K(\rm{Im}(\Phi))=n$