**内容**  
$\quad\lim f(x)=A,\;\lim g(x)=B$  
  
$\Rightarrow $  
  
$\quad\lim f(x)\cdot\lim g(x)$  
  
$\quad=\lim[f(x)\cdot g(x)]$  
  
$\quad=AB$  
  
  
**具体形式: $x\to x_0$**  
$\quad\lim\limits_{x\to x_0}f(x)=A,\;\lim\limits_{x\to x_0}g(x)=B$  
  
$\Rightarrow $  
  
$\quad\lim\limits_{x\to x_0}f(x)\cdot\lim\limits_{x\to x_0}g(x)$  
  
$\quad=\lim\limits_{x\to x_0}[f(x)\cdot g(x)]$  
  
$\quad=AB$  
  
**具体形式: $x\to x_0^{-}$**  
$\quad\lim\limits_{x\to x_0^-}f(x)=A,\;\lim\limits_{x\to x_0^-}g(x)=B$  
  
$\Rightarrow $  
  
$\quad\lim\limits_{x\to x_0^-}f(x)\cdot\lim\limits_{x\to x_0^-}g(x)$  
  
$\quad=\lim\limits_{x\to x_0^-}[f(x)\cdot g(x)]$  
  
$\quad=AB$  
  
**具体形式: $x\to x_0^{+}$**  
$\quad\lim\limits_{x\to x_0^+}f(x)=A,\;\lim\limits_{x\to x_0^+}g(x)=B$  
  
$\Rightarrow $  
  
$\quad\lim\limits_{x\to x_0^+}f(x)\cdot\lim\limits_{x\to x_0^+}g(x)$  
  
$\quad=\lim\limits_{x\to x_0^+}[f(x)\cdot g(x)]$  
  
$\quad=AB$  
  
**具体形式: $x\to+\infty$**  
$\quad\lim\limits_{x\to+\infty}f(x)=A,\;\lim\limits_{x\to+\infty}g(x)=B$  
  
$\Rightarrow $  
  
$\quad\lim\limits_{x\to+\infty}f(x)\cdot\lim\limits_{x\to+\infty}g(x)$  
  
$\quad=\lim\limits_{x\to+\infty}[f(x)\cdot g(x)]$  
  
$\quad=AB$  
  
**具体形式: $x\to-\infty$**  
$\quad\lim\limits_{x\to-\infty}f(x)=A,\;\lim\limits_{x\to-\infty}g(x)=B$  
  
$\Rightarrow $  
  
$\quad\lim\limits_{x\to-\infty}f(x)\cdot\lim\limits_{x\to-\infty}g(x)$  
  
$\quad=\lim\limits_{x\to-\infty}[f(x)\cdot g(x)]$  
  
$\quad=AB$  
  
**具体形式: $x\to\infty$**  
$\quad\lim\limits_{x\to\infty}f(x)=A,\;\lim\limits_{x\to\infty}g(x)=B$  
  
$\Rightarrow $  
  
$\quad\lim\limits_{x\to\infty}f(x)\cdot\lim\limits_{x\to\infty}g(x)$  
  
$\quad=\lim\limits_{x\to\infty}[f(x)\cdot g(x)]$  
  
$\quad=AB$  
