**证明**  
$\quad |\,f(x)g(x)-AB|$  
  
$\quad=|\,f(x)g(x)-f(x)B+f(x)B-AB|$  
  
$\quad\leq|\,f(x)|\,|g(x)-B|+|B|\,|\,f(x)-A|$  
  
$\quad<M\,|g(x)-B|+|B|\,|\,f(x)-A|$  
  
$\quad<M\cdot\dfrac{\epsilon}{2M}+|B|\cdot\dfrac{\epsilon}{2|B|}=\epsilon$  
  
$\quad\rm{or}<(M+|B|)\epsilon$  
  
---  
  
$\lim\limits_{x\to x_0}g(x)=B$  
  
$\Rightarrow\exists\;\delta_0>0,\;0<|x-x_0|<\delta_0,\;|g(x)|\leq M$  
  
$\Rightarrow\exists\;\delta_1,\;0<|x-x_0|<\delta_1,\;\forall\;g(x),\;|g(x)-B|<\dfrac\epsilon{2|A|}$  
  
$\lim\limits_{x\to x_0}f(x)=A$  
  
$\Rightarrow\exists\;\delta_3,\;0<|x-x_0|<\delta_3,\;\forall\;f(x),\;|f(x)-a|<\dfrac\epsilon{2M}$  
  
$\delta=\min\{\delta_1,\;\delta_2,\;\delta_3\}$  
  
$\Rightarrow\forall\;\epsilon>0,\;\exists\;\delta>0,\;0<|x-x_0|<\delta,\;\forall\;f(x),\;g(x)$  
  
$\quad |\,f(x)g(x)-AB|$  
  
$\quad=|\,f(x)g(x)-Ag(x)+Ag(x)-AB|$  
  
$\quad\leq|g(x)|\,|\,f(x)-A|+|A|\,|g(x)-B|$  
  
$\quad<M|\,f(x)-A|+|A||g(x)-B|$  
  
$\quad<M\,\dfrac\epsilon{2M}+|A|\,\dfrac\epsilon{2|A|}=\epsilon$  
