**证明**  
<font color=brown>必要性</font>: 若 $m(x)\mid f(x)-g(x)$ ，则 $f(x)$ 与 $g(x)$ 除以 $m(x)$ 具有相同的余式  
  
做带余除法  
$f(x)=m(x)\cdot q_a(x)+r_a(x), 0\leq\rm{deg}[r_a(x)]<\rm{deg}[m(x)]$  
$g(x)=m(x)\cdot q_b(x)+r_b(x), 0\leq\rm{deg}[r_b(x)]<\rm{deg}[m(x)]$  
  
等式两边相减  
$f(x)-g(x)$  
$=[\ m(x)\cdot q_a(x)+r_a(x)\ ]-[\ m(x)\cdot q_b(x)+r_b(x)\ ]$  
$=m(x)\cdot q_a(x)-m(x)\cdot q_b(x)+r_a(x)-r_b(x)$  
$=m(x)\cdot [\ q_a(x)-q_b(x)\ ]+r_a(x)-r_b(x)$  
  
因为 $m(x)\mid[\ f(x)-g(x)\ ]$  
$\Rightarrow m(x)\mid[\ r_a(x)-r_b(x)\ ]$  
  
$\rm{deg}[\ r_a(x)-r_b(x)\ ]\leq\max[\rm{deg}[r_a(x)],\rm{deg}[r_b(x)]]$  
$\Rightarrow \rm{deg}[\ r_a(x)-r_b(x)\ ]<\rm{deg}[m(x)]$  
  
<font color=blue>又因为 $m(x)$ 可以整除一个次数比它小的多项式</font>  
<font color=blue> $\Rightarrow r_a(x)-r_b(x)$ 只能是零多项式</font>  
$\Rightarrow r_a(x)=r_b(x)$  
$\Rightarrow f(x)$ 与 $g(x)$ 除以 $m(x)$ 具有相同的余式  
  
<font color=brown>充分性</font>: 若 $f(x)$ 与 $g(x)$ 除以 $m(x)$ 具有相同的余式，则 $m(x)\mid[f(x)-g(x)]$  
$f(x)$ 与 $g(x)$ 除以 $m(x)$ 具有相同的余式  
$\Rightarrow f(x)=m(x)\cdot q_1(x)+r(x),\ g(x)=m(x)\cdot q_2(x)+r(x)$  
两式作差得  
$\Rightarrow f(x)-g(x)=m(x)\cdot [\ q_1(x)-q_2(x)\ ]$  
$\Rightarrow m(x)\mid[f(x)-g(x)]$  
