**内容**  
设 $f(x),g(x)\in K[x]$ ，若存在 $h(x),r(x)\in K[x]$ ，使得 $f(x)=h(x)g(x)+r(x)$  
则 $d(x)=\rm{gcd}[f(x),g(x)]\Leftrightarrow d(x)=\rm{gcd}[g(x),r(x)]$  
  
**证明**  
任取 $f(x)$ 与 $g(x)$ 的一个公因式 $c(x)$  
$\Rightarrow c(x)\mid f(x),\ c(x)\mid g(x)$  
$\Rightarrow c(x)\mid f(x)-h(x)g(x)$  
$\Rightarrow c(x)\mid r(x)$  
  
任取 $g(x)$ 与 $r(x)$ 的一个公因式 $p(x)$  
$\Rightarrow p(x)\mid g(x),\ p(x)\mid r(x)$  
$\Rightarrow p(x)\mid h(x)g(x)+r(x)$  
$\Rightarrow p(x)\mid f(x)$  
  
$\Rightarrow f(x),g(x)$ 与 $g(x),r(x)$ 有相同的公因式  
  
$\Rightarrow c(x)$ 是 $f(x),g(x)$ 的公因式 $\Leftrightarrow c(x)$ 是 $g(x),r(x)$ 的公因式  
  
取 $d(x)=\rm{gcd}[f(x),g(x)]$  
$\Rightarrow d(x)$ 是 $g(x),r(x)$ 的公因式  
  
任取 $g(x)$ 与 $r(x)$ 的一个公因式 $c(x)$  
$\Rightarrow c(x)$ 是 $f(x),g(x)$ 的公因式  
又因为 $d(x)=\rm{gcd}[f(x),g(x)]$  
$\Rightarrow c(x)\mid d(x)$  
$\Rightarrow d(x)=\rm{gcd}[g(x),r(x)]$  
  
反之同理可证  
