**内容**  
x_1=2,\;x_{n+1}=\frac{2x^3_n+1}{3x^2_n}  
  
**说明**  
①首项等于2是为了说明数列为正项数列  
②由递推关系式求极限，通常是解方程  
  
**证明**  
Step1: 有下界  
$x_{n+1}=\frac13\left(x_n+x_n+\dfrac1{x^2_n}\right)$  
  
$\geq\sqrt[3]{x_n\cdot x_n\cdot\dfrac1{x^2_n}}=1$  
  
  
Step2: 单减  
$x_{n+1}-x_n=\dfrac{2x^3_n+1}{3x^2_n}-x_n$  
  
$=\dfrac{1-x^3_n}{3x^2_n}\leq0$  
  
$\Rightarrow x_n\geq x_{n+1}$  
  
  
Step3: 求极限  
$\lim\limits_{n\to+\infty}x_{n}=a$  
  
$\Rightarrow  
\lim\limits_{n\to+\infty}x_{n+1}=  
\lim\limits_{n\to+\infty}x_{n}=a$  
  
$\Rightarrow  
\left[2\left(\lim\limits_{n\to+\infty}x_n\right)^3+1\right]\div3\left(\lim\limits_{n\to+\infty}x_n\right)^2=  
\lim\limits_{n\to+\infty}x_{n}$  
  
$\Rightarrow \dfrac{2a^3+1}{3a^2}=a$  
  
$\Rightarrow a=1$  
