**内容**  
$0<x_1<1,\; x_{n+1}=x_n(1-x_n)$  
  
**证明**  
Step1: 有界  
  
$0<x_1<1,\; x_{n+1}=x_n(1-x_n)$  
  
$0<x_1<1$  
  
$\rm{suppose}\;0<x_k<1$  
  
$\Rightarrow 0<(1-x_k)<1$  
  
$\Rightarrow 0<x_k(1-x_k)<1$  
  
$\Rightarrow 0<x_{k+1}<1$  
  
$\Rightarrow 0<x_{n}<1$  
  
---  
  
Step2: 单调  
  
$x_{n+1}=x_n(1-x_n)$  
  
$\Rightarrow x_{n+1}-x_n=x_n(1-x_n)-x_n=-x_n^2<0$  
  
---  
  
Step3: 求极限  
  
$\lim\limits_{n\to\infty}x_n=a$  
  
$x_{n+1}=x_n(1-x_n)$  
  
$\Rightarrow \lim\limits_{n\to\infty}x_{n+1}=\lim\limits_{n\to\infty}[x_n(1-x_n)]$  
  
$=\lim\limits_{n\to\infty}x_n\cdot\lim\limits_{n\to\infty}(1-x_n)$  
  
$=[1-\lim\limits_{n\to\infty}x_n]\cdot\lim\limits_{n\to\infty}x_n$  
  
$\Rightarrow a=(1-a)a$  
  
$\Rightarrow a=0\quad\Rightarrow\lim\limits_{n\to\infty}x_n=0$  
  
---  
  
**拓展**  
$x_{n+1}=x_n(1-x_n)$  
  
$\lim\limits_{n\to\infty}(nx_n)$  
  
$=\lim\limits_{n\to\infty}\dfrac{n}{\dfrac1{x_n}}$  
  
$=\lim\limits_{n\to\infty}\dfrac{n-(n-1)}{\dfrac1{x_n}-\dfrac1{x_{n-1}}}$  
  
$=\lim\limits_{n\to\infty}\dfrac{x_{n-1}-x_n}{x_{n-1}\cdot x_n}$  
  
$=\lim\limits_{n\to\infty}\dfrac{x_{n-1}-x_{n-1}(1-x_{n-1})}{x_{n-1}\cdot x_{n-1}(1-x_{n-1})}$  
  
$=\lim\limits_{n\to\infty}\dfrac{x_{n-1}^2}{x_{n-1}^2\cdot(1-x_{n-1})}$  
  
$=\lim\limits_{n\to\infty}\dfrac{1}{1-x_{n-1}}=1$  
  
1 巩固stolz定理  
  
2 引出等价无穷小的概念  
