**证明思路**  
  
要证 $T$ 是单射，只要证若 $T(\Phi)=T(\Psi)=A$ ，则 $\Phi=\Psi$  
  
**证明： $T$ 是单射**  
 $\forall\ \Phi，\Psi\in\mathbb L(U^n,V^m)$  
  
令 $T(\Phi)=T(\Psi)=A=\lgroup a_{ij}\rgroup_{m\times n}\in M_{m\times n}(K)$  
  
 $\begin{cases}  
\Phi(e_1)=\beta_1=a_{11}\cdot f_1+a_{21}\cdot f_2  
+\cdots+a_{m1}\cdot f_m\\\  
\Phi(e_2)=\beta_2=a_{12}\cdot f_1+a_{22}  
\cdot f_2+\cdots+a_{m2}\cdot f_m\\\  
\Phi(e_3)=\beta_3=a_{13}\cdot f_1+a_{23}  
\cdot f_2+\cdots+a_{m3}\cdot f_m\\\  
\cdots\\\  
\Phi(e_n)=\beta_n=a_{1n}\cdot f_1+a_{2n}  
\cdot f_2+\cdots+a_{mn}\cdot f_m  
\end{cases}$  
  
 $\begin{cases}  
\Psi(e_1)=\gamma_1=b_{11}\cdot f_1+b_{21}\cdot f_2  
+\cdots+b_{m1}\cdot f_m\\\  
\Psi(e_2)=\gamma_2=b_{12}\cdot f_1+b_{22}  
\cdot f_2+\cdots+b_{m2}\cdot f_m\\\  
\Psi(e_3)=\gamma_3=b_{13}\cdot f_1+b_{23}  
\cdot f_2+\cdots+b_{m3}\cdot f_m\\\  
\cdots\\\  
\Psi(e_n)=\gamma_n=b_{1n}\cdot f_1+b_{2n}  
\cdot f_2+\cdots+b_{mn}\cdot f_m  
\end{cases}$  
  
又因为 $T(\Phi)=T(\Psi)=A$  
  
 $\Rightarrow a_{ij}=b_{ij}$  
  
 $\Rightarrow\beta_i=\gamma_i,\forall\ 1\le i\le n$  
  
 $\Rightarrow\Phi(e_i)=\Psi(e_i),\forall\ 1\le i\le n$  
  
 $\Rightarrow\Phi，\Psi$ 是同一个映射 (线性扩张的唯一性)  
  
---  
综上两点，得 $T$ 是双射  
