**用逆矩阵证明克莱姆法则**  
 $A_{n\times n}\cdot X_{n\times1}=\beta_{n\times1}$   
  
 $\Rightarrow A^{-1}\cdot A_{n\times n}\cdot X_{n\times1}=A^{-1}\cdot\beta_{n\times1}，$ 等式两边同时左乘 $A$ 的逆矩阵  
  
 $\Rightarrow E\cdot X_{n\times1}=A^{-1}\cdot\beta_{n\times1}$   
  
 $\Rightarrow X_{n\times1}=A^{-1}\cdot\beta_{n\times1}$   
  
 $\Rightarrow X_{n\times1}=\frac1{|A|}A^\star\cdot\beta_{n\times1}$   
  
 $\Rightarrow X_{n\times1}=\frac1{|A|}(A^\star_{n\times n}\cdot\beta_{n\times1})$   
  
 $\begin{bmatrix}  
x_1\\\ x_2\\\ \vdots\\\ x_n  
\end{bmatrix}=\frac1{|A^\star|}\cdot\begin{bmatrix}  
A_{11}&A_{21}&A_{31}&\cdots&A_{n1}\\\   
A_{12}&A_{22}&A_{32}&\cdots&A_{n2}\\\   
\vdots&\vdots&\vdots&\ddots&\vdots\\\   
A_{1n}&A_{2n}&A_{3n}&\cdots&A_{nn}  
\end{bmatrix}\cdot\begin{bmatrix}  
b_1\\\ b_2\\\ \vdots\\\ b_m  
\end{bmatrix}$   
  
 $\Rightarrow x_j=\frac1{|A|}(b_1A_{1j}+b_2A_{2j}+\cdots+b_nA_{nj})$   
  
 $\Rightarrow x_j=\frac1{|A|}  
\sum\limits_{i=1}^nb_i\cdot A_{ij}$ ， $\beta$ 替换 $|A|$ 的第 $j$ 列  
  
 $\Rightarrow x_j=\frac{|A_j|}{|A|}$ (按列展开)  
  
注释：  
  
 $b_1A_{1j}$ ：第1行第 $j$ 列  
  
 $b_2A_{2j}$ ：第2行第 $j$ 列  
  
 $\cdots$   
  
 $b_nA_{nj}$ ：第 $n$ 行第 $j$ 列  
