**说明**  
是否暗示着可以把a-b上的定积分，转化成  
0-1上的定积分，一个普通的线性变量代换?  
  
**公式**  
$\int\limits_a^bf(x)\,dx=(b-a)\int_0^1f\,[a+(b-a)x]dx$  
  
**推导**  
$\int\limits_a^bf(x)\,dx$  
  
$=\lim\limits_{n\to\infty}\sum\limits_{i=1}^nf\left(a+\dfrac{b-a}n\cdot i\right)\cdot\dfrac{b-a}n=\lim\limits_{n\to\infty}(b-a)\sum\limits_{i=1}^nf\left[a+(b-a)\cdot\dfrac{i}n\right]\cdot\dfrac1n$  
  
$=(b-a)\int\limits_0^1f\,[a+(b-a)x]dx$  
  
$\rm{let}\;a+(b-a)x=t$  
  
$\Rightarrow x=0\to t=a,\;x=1\to t=b,\;dx=\dfrac1{b-a}dt$  
  
$=(b-a)\int\limits_a^bf(t)\cdot\dfrac1{b-a}dt$  
  
$=\int\limits_a^bf(t)dt=\int\limits_a^bf(x)dx$  
  
**例**  
$\int\limits_1^2\sqrt x dx=\int\limits_0^1 \sqrt{1+x}dx$  
  
$a=1,\;b=2,\;a+(b-a)x=1+(2-1)x=1+x$  
