**左分配律**

设矩阵$A_{m\times n}, B_{m\times n}，C_{n\times p}$

则左分配律：$(A+B)\cdot C=A\cdot C+B\cdot C$

**右分配律**

设矩阵$A_{m\times n}, B_{n\times p}，C_{n\times p}$

则右分配律：$A\cdot(B+C)=A\cdot B+A\cdot C$

**左分配律证明**

$(A+B)\cdot C=\sum\limits_{k=1}^n(a_{ik}+b_{ik})\cdot c_{kr}$

$=\sum\limits_{k=1}^na_{ik}\cdot c_{kr}+\sum\limits_{k=1}^nb_{ik}\cdot c_{kr}$

$=A\cdot C+B\cdot C$

**右分配律证明**

$A\cdot(B+C)=\sum\limits_{k=1}^na_{ik}\cdot(b_{kr}+c_{kr})$

$\sum\limits_{k=1}^na_{ik}\cdot b_{kr}+\sum\limits_{k=1}^na_{ik}\cdot c_{kr}$

$=A\cdot B+A\cdot C$