**例**  
  
$\begin{vmatrix}(a+b)^2&c^2&c^2\\\ a^2&(b+c)^2&a^2\\\ b^2&b^2&(c+a)^2\end{vmatrix}=2abc(a+b+c)^3$  
  
  
  
解：  
  
$=\underset{第2列乘-1加到第1,3列}{\underline{\begin{vmatrix}(a+b)^2-c^2&c^2&0\\\ a^2-(b+c)^2&(b+c)^2&a^2-(b+c)^2\\\ 0&b^2&(c+a)^2-b^2\end{vmatrix}}}$  
  
  
  
$=\underset{第1,3列提取公因子}{\underline{(a+b+c)^2\cdot\begin{vmatrix}a+b-c&c^2&0\\\ a-b-c&(b+c)^2&a-b-c\\\ 0&b^2&a+c-b\end{vmatrix}}}$  
  
  
  
$=\underset{第1,3行乘-1，加到第2行}{\underline{(a+b+c)^2\cdot\begin{vmatrix}a+b-c&c^2&0\\\ -2b&2bc&-2c\\\ 0&b^2&a+c-b\end{vmatrix}}}$  
  
  
  
$=\underset{第1列乘\frac c2加到第2列，第3列乘\frac b2加到第2列}{\underline{(a+b+c)^2\cdot\begin{vmatrix}a+b-c&\frac c2(a+b+c)&0\\\ -2b&0&-2c\\\ 0&\frac b2(a+b+c)&a+c-b\end{vmatrix}}}$  
  
  
  
$=\underset{第2列提取公因子}{\underline{(a+b+c)^3\cdot\begin{vmatrix}a+b-c&\frac c2&0\\\ -2b&0&-2c\\\ 0&\frac b2&a+c-b\end{vmatrix}}}$  
  
  
  
$=(a+b+c)^3\cdot\left(\right.$  
  
$\underset{按第1列展开}{\underline{(a+b-c)\begin{vmatrix}0&-2c\\\ \frac b2&a+c-b\end{vmatrix}-(-2b)\cdot\begin{vmatrix}\frac c2&0\\\ \frac b2&a+c-b\end{vmatrix}\left.\right)}}$  
  
  
  
$=(a+b+c)^3\cdot[(a+b-c)\cdot bc+bc\cdot(a+c-b)]$  
  
  
  
$=2abc(a+b+c)^3$  
