 $\begin{vmatrix}  
\lambda&-1&0&0\\\   
0&\lambda&-1&0\\\    
0&0&\lambda&-1\\\   
4&3&2&\lambda+1  
\end{vmatrix}$   
  
按第1行展开  
 $=a_{11}\cdot A_{11}+a_{12}\cdot A_{12}  
+a_{13}\cdot A_{13}+a_{14}\cdot A_{14}$   
  
 $=a_{11}\cdot A_{11}+a_{12}\cdot A_{12}+0+0$   
  
 $=\lambda\cdot(-1)^{1+1}\cdot  
\begin{vmatrix}  
\lambda&-1&0\\\    
0&\lambda&-1\\\   
3&2&\lambda+1  
\end{vmatrix}$   
  
 $+(-1)\cdot(-1)^{1+2}\cdot  
\begin{vmatrix}  
0&-1&0\\\    
0&\lambda&-1\\\   
4&2&\lambda+1  
\end{vmatrix}$   
  
按第4行展开  
 $=a_{41}\cdot A_{41}+a_{42}\cdot A_{42}  
+a_{43}\cdot A_{43}+a_{44}\cdot A_{44}$   
  
 $=4\cdot(-1)^{4+1}\cdot  
\begin{vmatrix}  
-1&0&0\\\   
\lambda&-1&0\\\    
0&\lambda&-1  
\end{vmatrix}$   
  
 $+3\cdot(-1)^{4+2}\cdot  
\begin{vmatrix}  
\lambda&0&0\\\   
0&-1&0\\\    
0&\lambda&-1  
\end{vmatrix}$   
  
 $+2\cdot(-1)^{4+3}\cdot  
\begin{vmatrix}  
\lambda&-1&0\\\   
0&\lambda&0\\\    
0&0&-1  
\end{vmatrix}$   
  
 $+(\lambda+1)\cdot(-1)^{4+4}\cdot  
\begin{vmatrix}  
\lambda&-1&0\\\   
0&\lambda&-1\\\    
0&0&\lambda  
\end{vmatrix}$   
  
 $=4+3\lambda+2\lambda^2  
+\lambda^3(\lambda+1)$   
  
 $=4+3\lambda+2\lambda^2  
+\lambda^3+\lambda^4$   
