 $\begin{vmatrix}  
3&1&-1&2\\\   
-5&1&3&-4\\\    
2&0&1&-1\\\   
1&-5&3&-3  
\end{vmatrix}$   
  
第3列乘 $-2$ ，加到第1列  
第3列乘 $1$ ，加到第4列  
 $=\begin{vmatrix}  
5&1&-1&1\\\   
-11&1&3&-1\\\    
0&0&1&0\\\   
-5&-5&3&0  
\end{vmatrix}$   
  
按第3行展开  
 $=1\cdot(-1)^{3+3}\cdot  
\begin{vmatrix}  
5&1&1\\\   
-11&1&-1\\\    
-5&-5&0  
\end{vmatrix}$   
  
第1行乘1，加到第2行  
 $=\begin{vmatrix}  
5&1&1\\\   
-6&2&0\\\    
-5&-5&0  
\end{vmatrix}$   
  
按第3列展开  
 $=1\cdot(-1)^{1+3}\cdot  
\begin{vmatrix}  
-6&2\\\    
-5&-5  
\end{vmatrix}=30+10=40$   
