**内容**
$\quad\lim f(x)=A,\;\lim g(x)=B,\;(B\neq0)$

$\Rightarrow $

$\quad\dfrac{\lim f(x)}{\lim g(x)}=\lim\dfrac{f(x)}{g(x)}=\dfrac AB$

**具体形式: $x\to x_0$**
$\quad\lim\limits_{x\to x_0}f(x)=A,\;\lim\limits_{x\to x_0}g(x)=B,\;(B\neq0)$

$\Rightarrow $

$\quad\lim\limits_{x\to x_0}f(x)\div\lim\limits_{x\to x_0}g(x)$

$\quad=\lim\limits_{x\to x_0} \dfrac{f(x)}{g(x)}=\dfrac AB$

**具体形式: $x\to x_0^{-}$**
$\quad\lim\limits_{x\to x_0^-}f(x)=A,\;\lim\limits_{x\to x_0^-}g(x)=B,\;(B\neq0)$

$\Rightarrow $

$\quad\lim\limits_{x\to x_0^-}f(x)\div\lim\limits_{x\to x_0^-}g(x)$

$\quad=\lim\limits_{x\to x_0^-}\dfrac{f(x)}{g(x)}=\dfrac AB$

**具体形式: $x\to x_0^{+}$**
$\quad\lim\limits_{x\to x_0^+}f(x)=A,\;\lim\limits_{x\to x_0^+}g(x)=B,\;(B\neq0)$

$\Rightarrow $

$\quad\lim\limits_{x\to x_0^+}f(x)\div\lim\limits_{x\to x_0^+}g(x)$

$\quad=\lim\limits_{x\to x_0^+}\dfrac{f(x)}{g(x)}=\dfrac AB$

**具体形式: $x\to+\infty$**
$\quad\lim\limits_{x\to+\infty}f(x)=A,\;\lim\limits_{x\to+\infty}g(x)=B,\;(B\neq0)$

$\Rightarrow $

$\quad\lim\limits_{x\to+\infty}f(x)\div\lim\limits_{x\to+\infty}g(x)$

$\quad=\lim\limits_{x\to+\infty}\dfrac{f(x)}{g(x)}=\dfrac AB$

**具体形式: $x\to-\infty$**
$\quad\lim\limits_{x\to-\infty}f(x)=A,\;\lim\limits_{x\to-\infty}g(x)=B,\;(B\neq0)$

$\Rightarrow $

$\quad\lim\limits_{x\to-\infty}f(x)\div\lim\limits_{x\to-\infty}g(x)$

$\quad=\lim\limits_{x\to-\infty}\dfrac{f(x)}{g(x)}=\dfrac AB$

**具体形式: $x\to\infty$**
$\quad\lim\limits_{x\to\infty}f(x)=A,\;\lim\limits_{x\to\infty}g(x)=B,\;(B\neq0)$

$\Rightarrow $

$\quad\lim\limits_{x\to\infty}f(x)\div\lim\limits_{x\to\infty}g(x)$

$\quad=\lim\limits_{x\to\infty} \dfrac{f(x)}{g(x)}=\dfrac AB$
