**定理**  
$y=x^\alpha$  
  
$\Rightarrow \lim\limits_{x\to x_0}x^\alpha=x_0^\alpha$  
  
**证明: 复合函数连续性**  
$\lim\limits_{x\to x_0}x^\alpha=x_0^\alpha$  
  
$\iff\lim\limits_{x\to x_0}(x^\alpha-x_0^\alpha)=0$  
  
$\rm{let}\;x^\alpha=e^{\alpha\ln x},\;x\in(0,+\infty)$  
  
$\iff\lim\limits_{x\to x_0}(e^{\alpha\ln x}-e^{\alpha\ln x_0})=0$  
  
$\iff e^{\alpha\ln x_0}\lim\limits_{x\to x_0}[e^{\alpha(\ln x-\ln x_0)}-1]=0$  
  
$y=e^u,\;u=\alpha(v),\;v=\ln x-\ln x_0$  
  
$\rm{or}$  
  
$x^\alpha=e^{\ln x^\alpha}=e^{\alpha\ln x},\;x\in(0,+\infty)$  
  
$\Rightarrow y=e^u,\;u=\alpha\ln x$  
