**三元牛顿公式**    
 $n=3$     
    
 $k=1,\ \sigma_0\cdot P_1-\sigma_1\cdot1=0$     
    
 $k=2,\ \sigma_0\cdot P_2-\sigma_1\cdot P_1+\sigma_2\cdot2=0$     
    
 $k=3,\ \sigma_0\cdot P_3-\sigma_1\cdot P_2+\sigma_2\cdot P_1-\sigma_3\cdot P_0=0$     
    
 $k=4,\ \sigma_0\cdot P_4-\sigma_1\cdot P_3+\sigma_2\cdot P_2-\sigma_3\cdot P_1=0$     
    
 $k=5,\ \sigma_0\cdot P_5-\sigma_1\cdot P_4+\sigma_2\cdot P_3-\sigma_3\cdot P_2=0$     
    
 $k=6,\ \sigma_0\cdot P_6-\sigma_1\cdot P_5+\sigma_2\cdot P_4-\sigma_3\cdot P_3=0$     
    
 $k=7,\ \sigma_0\cdot P_7-\sigma_1\cdot P_6+\sigma_2\cdot P_5-\sigma_3\cdot P_4=0$     
    
 $k=8,\ \sigma_0\cdot P_8-\sigma_1\cdot P_7+\sigma_2\cdot P_6-\sigma_3\cdot P_5=0$     
    
 $k=9,\ \sigma_0\cdot P_9-\sigma_1\cdot P_8+\sigma_2\cdot P_7-\sigma_3\cdot P_6=0$     
    
可以依次递推下去    
