**例1**  
 $x_1^2+x_2^2=(x_1+x_2)^2-2x_1x_2=\sigma_1^2-2\sigma_2=y_1^2-2y_2$   
  
**例2**  
 $x+y+z=1$   
 $x^2+y^2+z^2=2$   
 $x^3+y^3+z^3=3$   
求 $x^5+y^5+z^5$   
  
解:  
 $\sigma_0=1,\ \sigma_1=x+y+z=1$   
  
 $S_3=x^3+y^3+z^3=3,\ S_2=x^2+y^2+z^2=2,\ S_1=x+y+z=1,\ S_0=3$   
  
 $k=5,n=3:\ \sigma_0\cdot S_5-\sigma_1\cdot S_4+\sigma_2\cdot S_3-\sigma_3\cdot S_2=0$   
 $k=4,n=3:\ \sigma_0\cdot S_4-\sigma_1\cdot S_3+\sigma_2\cdot S_2-\sigma_3\cdot S_1=0$   
 $k=3,n=3:\ \sigma_0\cdot S_3-\sigma_1\cdot S_2+\sigma_2\cdot S_1-\sigma_3\cdot S_0=0$   
 $k=2,n=3:\ \sigma_0\cdot S_2-\sigma_1\cdot S_1+\sigma_2\cdot 2=0$   
  
 $\Rightarrow\sigma_2=\dfrac12\cdot(\sigma_1\cdot S_1-\sigma_0\cdot S_2)=\dfrac12\cdot(1-2)=-\dfrac12$   
  
 $\Rightarrow\sigma_3=\dfrac13\cdot(\sigma_0\cdot S_3-\sigma_1\cdot S_2+\sigma_2\cdot S_1)  
=\dfrac13\cdot(1*3-1*2-\dfrac12*1)=\dfrac16$   
  
 $\Rightarrow S_4=\sigma_1\cdot S_3-\sigma_2\cdot S_2+\sigma_3\cdot S_1  
=1*3+\dfrac12*2+\dfrac16=\dfrac{25}6$   
  
 $S_5=\sigma_1\cdot S_4-\sigma_2\cdot S_3+\sigma_3\cdot S_2  
=1*\dfrac{25}6+\dfrac12*3+\dfrac16*2=6$   
