**内容**  
设 $f$ 是 $A$ 到 $B$ 的映射， $g$ 是 $B$ 到 $C$ 的映射， $h$ 是 $C$ 到 $D$ 的映射，则 $(\ h\circ(g\circ f)\ )(x)  
=(\ (h\circ g)\circ f\ )(x)$   
  
**说明**  
复合映射结合律、映射乘法结合律  
  
**证明**  
 $\begin{array}{cc}  
\begin{array}{c}  
(\ h\circ g\circ f\ )(\ x\ )\\\   
=h(\ g\ (\ f(\ x\ )\ )\ )\\\   
=h(\ g\ (\ y\ )\ )\\\   
=h(\ z\ )=w\\\   
\end{array}&  
\begin{array}{c}  
(\ (\ h\circ g\ )\circ f\ )(\ x\ )\\\   
=(\ h\circ g\ )(\ f(\ x\ )\ )\\\   
=(\ h\circ g\ )(\ y\ )\\\   
=h(\ g\ (\ y\ )\ )\\\   
=h(\ z\ )=w  
\end{array}  
\end{array}$   
