**内容**  
$\lim f(x) = A, \ m \in N^+$  
  
$\Rightarrow \lim[f(x)]^m=\left[\lim f(x)\right]^m= A^m$  
  
**具体形式: $x\to x_0$**  
$\lim\limits_{x\to x_0} f(x) = A, \ m \in N^+$  
  
$\Rightarrow \lim\limits_{x\to x_0}[f(x)]^m=\left[\lim\limits_{x\to x_0}f(x)\right]^m= A^m$  
  
**具体形式: $x\to x_0^{-}$**  
$\lim\limits_{x\to x_0^-}f(x)=A,\ m\in N^+$  
  
$\Rightarrow \lim\limits_{x\to x_0^-}[f(x)]^m=\left[\lim\limits_{x\to x_0^-}f(x)\right]^m= A^m$  
  
**具体形式: $x\to x_0^{+}$**  
$\lim\limits_{x\to x_0^+} f(x) = A, \ m \in N^+$  
  
$\Rightarrow \lim\limits_{x\to x_0^+}[f(x)]^m=\left[\lim\limits_{x\to x_0^+}f(x)\right]^m= A^m$  
  
**具体形式: $x\to+\infty$**  
$\lim\limits_{x\to+\infty} f(x) = A, \ m \in N^+$  
  
$\Rightarrow \lim\limits_{x\to+\infty}[f(x)]^m=\left[\lim\limits_{x\to+\infty}f(x)\right]^m= A^m$  
  
**具体形式: $x\to-\infty$**  
$\lim\limits_{x\to-\infty} f(x) = A, \ m \in N^+$  
  
$\Rightarrow \lim\limits_{x\to-\infty}[f(x)]^m=\left[\lim\limits_{x\to-\infty}f(x)\right]^m= A^m$  
  
**具体形式: $x\to\infty$**  
$\lim\limits_{x\to\infty} f(x) = A, \ m \in N^+$  
  
$\Rightarrow \lim\limits_{x\to\infty}[f(x)]^m=\left[\lim\limits_{x\to \infty}f(x)\right]^m= A^m$  
