**公式**

$\begin{bmatrix}\mu_1\\\ \mu_2\\\ \vdots\\\ \mu_m\end{bmatrix}=A\cdot\begin{bmatrix}\lambda_1\\\ \lambda_2\\\ \vdots\\\ \lambda_n\end{bmatrix}$

**推导**
$\forall\ \alpha\in V_K,\ \alpha=\lambda_1\cdot e_1+\lambda_2\cdot e_2+\cdots+\lambda_n\cdot e_n$

$\Rightarrow\Phi(\alpha)=\mu_1\cdot f_1+\mu_2\cdot f_2+\cdots+\mu_m\cdot f_m$
$=[f_1,f_2,\cdots,f_m]\cdot\begin{bmatrix}\mu_1\\\ \mu_2\\\ \vdots\\\ \mu_m\end{bmatrix}$

---

$=\Phi(\lambda_1\cdot e_1+\lambda_2\cdot e_2+\cdots+\lambda_n\cdot e_n)$
$=\lambda_1\cdot\Phi(e_1)+\lambda_2\cdot\Phi(e_2)+\cdots+\lambda_n\cdot\Phi(e_n)$
$=[\Phi(e_1),\Phi(e_2),\cdots,\Phi(e_n)]\cdot\begin{bmatrix}\lambda_1\\\ \lambda_2\\\ \vdots\\\ \lambda_n\end{bmatrix}$
$=[f_1,f_2,\cdots,f_m]\cdot A\cdot\begin{bmatrix}\lambda_1\\\ \lambda_2\\\ \vdots\\\ \lambda_n\end{bmatrix}$

---

$\Rightarrow\begin{bmatrix}\mu_1\\\ \mu_2\\\ \vdots\\\ \mu_m\end{bmatrix}=A\cdot\begin{bmatrix}\lambda_1\\\ \lambda_2\\\ \vdots\\\ \lambda_n\end{bmatrix}$
