**例1**
$f(x_1,x_2,x_3)=x_1^2x_2+x_1^2x_3+x_2^2x_1+x_2^2x_1+x_2^2x_3+x_3^2x_1+x_3^2x_2$

解:
字典排序下，$f(x_1,x_2,x_3)$的首项为$x_1^2x_2$
$\Rightarrow g_1(x_1,x_2,x_3)=1\cdot\sigma_1^{2-1}\cdot \sigma_2^{1-0}\cdot \sigma_3^{0}$
$=(x_1+x_2+x_3)\cdot(x_1x_2+x_2x_3+x_3x_1)$
$=x_1^2x_2+x_1x_2x_3+x_3x_1^2+x_1x_2^2+x_2^2x_3+x_1x_2x_3+x_1x_2x_3+x_2x_3^2+x_3^2x_1$
$=x_1^2x_2+x_3x_1^2+x_1x_2^2+x_2^2x_3+x_2x_3^2+x_3^2x_1+3x_1x_2x_3$

$\Rightarrow f_1=f-g_1=-3x_1x_2x_3$

$\Rightarrow g_2=-3\sigma_1^{1-1} \sigma_2^{1-1}\ \sigma_3^1=-3(x_1x_2x_3)$

$\Rightarrow f_2=f_1-g_2=0$

$\Rightarrow f=g_1+f_1=g_1+g_2+f_2=\sigma_1\cdot \sigma_2-3\sigma_3+0$
