$f(x)=3x^4-4x^3+5x-1$ ， $g(x)=x^2-x+1$  
 $q(x)=3x^2-x-4$ ， $r(x)=2x+3$  
  
由证明过程知，可用用 $g(x)$ 不断的干掉 $f(x)$ 的最高次幂，直到 $\rm{deg}[f(x)]<\rm{deg}[g(x)]$ 为止  
  
 $\begin{array}{c:c}  
f(x)=3x^4-4x^3+5x-1&g(x)=x^2-x+1\\\  
\quad3x^4-3x^3+3x^2&q(x)=3x^2-x-4\\\  
\quad\quad\quad\quad\quad\quad\quad-x^3-3x^2+5x-1&\\\  
\quad\quad\quad\quad\quad-x^3+x^2-x&\\\  
\quad\quad\quad\quad\quad\quad\quad\quad\quad\quad-4x^2+6x-1&\\\  
\quad\quad\quad\quad\quad\quad\quad\quad\quad\quad-4x^2+4x-4&\\\  
\quad\quad\quad\quad\quad\quad\quad\quad\quad\quad\quad\quad q(x)=2x+3&  
\end{array}$  
