**内容**  
设 $\Phi,\ \Psi\in\rm{Hom}(V,U)$ ，  
 $(e_1,\cdots,e_n)$ 是 $V_K^n$ 的一个基，  
 $(f_1,\cdots,f_m)$ 是 $U_K^m$ 的一个基，  
 $\Phi$ 在该基下的表示矩阵为 $A$ ，  
 $\Psi$ 在该基下的表示矩阵为 $B$ ，  
则 $(\Phi+\Psi)$ 在该基下的表示矩阵为 $A+B$  
  
**证明**  
 $(\Phi+\Psi)(e_i),\ 1\le i\le n$  
  
 $=\Phi(e_i)+\Psi(e_i)$  
  
 $=(a_{1i}f_1+a_{2i}f_2+\cdots+a_{mi}f_m)+(b_{1i}f_1+b_{2i}f_2+\cdots+b_{mi}f_m)$  
  
 $=(a_{1i}+b_{1i})f_1+(a_{2i}+b_{2i})f_2+\cdots+(a_{mi}+b_{mi})f_m$  
  
 $\Rightarrow(\Phi+\Psi)(e_i)=(a_{1i}+b_{1i})f_1+(a_{2i}+b_{2i})f_2+\cdots+(a_{mi}+b_{mi})f_m$  
  
 $\Rightarrow(\Phi+\Psi)$ 在该基下的表示矩阵为 $A+B$  
  
---  
  
 $((\Phi+\Psi)(e_1),(\Phi+\Psi)(e_2),\cdots,(\Phi+\Psi)(e_n))$  
  
 $=(\Phi(e_1)+\Psi(e_1),\Phi(e_2)+\Psi(e_2),\cdots,\Phi(e_n)+\Psi(e_n))$  
  
 $=(\Phi(e_1),\Phi(e_2),\cdots,\Phi(e_n))+(\Psi(e_1),\Psi(e_2),\cdots,\Psi(e_n))$  
  
 $=(e_1,e_2,\cdots,e_n)A+(e_1,e_2,\cdots,e_n)B$  
  
 $=(e_1,e_2,\cdots,e_n)(A+B)$  
