**内容**
$\lim\limits_{x\to0}\left(\dfrac{a^x+b^x+c^x}{3}\right)^{\dfrac1x}$

**解法一**
$\lim\limits_{x\to0}\left(\dfrac{a^x+b^x+c^x}{3}\right)^{\dfrac1x}$

$=\lim\limits_{x\to0}\left[1+\left(\dfrac{a^x+b^x+c^x}{3}-1\right)\right]^{\dfrac1x}$

$=\lim\limits_{x\to0}\left[1+\left(\dfrac{a^x+b^x+c^x}{3}-1\right)\right]^{\dfrac1{x\cdot\left(\dfrac{a^x+b^x+c^x}{3}-1\right)}\cdot\left(\dfrac{a^x+b^x+c^x}{3}-1\right)}$

$\lim\limits_{x\to0}\dfrac{\left(\dfrac{a^x+b^x+c^x}{3}-1\right)}{x}$

$=\lim\limits_{x\to0}\dfrac13\cdot\left(\dfrac{a^x-1}x+\dfrac{b^x-1}x+\dfrac{c^x-1}x\right)$

$=\dfrac13\cdot\left(\ln a+\ln b+\ln c\right)$

$=\ln(abc)^{\dfrac13}$

$\Rightarrow\lim\limits_{x\to0}\left(\dfrac{a^x+b^x+c^x}{3}\right)^{\dfrac1x}=e^{\ln(abc)^{\dfrac13}}=\sqrt[3]{abc}$

**解法二**
$\lim\limits_{x\to0}\left(\dfrac{a^x+b^x+c^x}{3}\right)^{\dfrac1x}$

$=\lim\limits_{x\to0}e^{\dfrac1x\ln\left(\dfrac{a^x+b^x+c^x}{3}\right)}$

$=\lim\limits_{x\to0}e^{\dfrac1x\ln\left[1+\left(\dfrac{a^x+b^x+c^x}{3}\right)-1\right]}$

$=\lim\limits_{x\to0}e^{\dfrac1x\ln\left[1+\left(\dfrac{a^x+b^x+c^x}{3}-1\right)\right]}$

$=\lim\limits_{x\to0}e^{\dfrac1x\cdot\left(\dfrac{a^x+b^x+c^x}{3}-1\right)}$

$=\lim\limits_{x\to0}e^{\dfrac13\cdot\left(\dfrac{a^x-1}x+\dfrac{b^x-1}{x}+\dfrac{c^x-1}{x}\right)}$

$=e^{\dfrac13\cdot\left(\ln a+\ln b+\ln c\right)}=\sqrt[3]{abc}$
