**预备**    
    
自同构 $=$ 线性变换 $+$ 双射    
    
**证明**    
<font color=brown>必要性</font>    
设 $\Phi$ 是自同构    
    
 $\Rightarrow\Phi$ 存在逆映射，记作 $\Phi^{-1}$     
    
 $\Rightarrow I_V=\Phi\circ\Phi^{-1}    
=\Phi^{-1}\circ\Phi$  ( $I_V$ 也是自同构)    
    
 $\Rightarrow T(I_V)=T(\Phi\circ\Phi^{-1})$     
    
 $=T(\Phi\cdot\Phi^{-1})$     
    
 $=T(\Phi)\cdot T(\Phi^{-1})$     
    
 $=A\cdot B$     
    
又因为 $E_n=T(I_V)$     
    
 $\Rightarrow E_n=T(\Phi)\cdot T(\Phi^{-1})$     
    
 $\Rightarrow T(\Phi)$ 可逆，且 $T(\Phi^{-1})    
=T(\Phi)^{-1}$     
    
<font color=brown>充分性</font>    
设 $T(\Phi)$ 是可逆阵    
    
表示矩阵映射 $T:\mathbb L(V^n_K)\rightarrow M_n(K)$ 是双射    
    
 $\Rightarrow T(\Phi)^{-1}\in M_n(K)，\exists\ \Psi\in \mathbb L(V_K^n)，T(\Psi)=T(\Phi)^{-1}$     
    
 $\Rightarrow E_n=T(\Psi)\cdot T(\Phi)    
=T(\Phi)\cdot T(\Psi)\ $ 逆矩阵定义    
    
 $\Rightarrow\underset{T是双射+前面的引理+T保持乘法}{\underline{T(I_V)=T(\Psi\circ\Phi)    
=T(\Phi\circ\Psi)}}$     
    
 $\Rightarrow I_V=\Psi\circ\Phi=\Phi\circ\Psi\ $ (映射 $T$ 的单性)    
    
 $\Rightarrow \Psi=\Phi^{-1}\ $ (逆映射存在定理)    
    
 $\Rightarrow \Psi$  是 $\Phi$ 的逆映射    
    
 $\Rightarrow\Phi$ 是双射    
    
 $\Rightarrow\Phi$  是自同构    
    
**备注**    
线性恒等变换 $=$ 自同构 $=$ 线性变换 $+$ 双射    
