$\begin{vmatrix}
a_1+x_1&a_2&\cdots&a_n\\\ 
a_1&a_2+x_2&\cdots&a_n\\\ 
\vdots&\vdots&\ddots&\vdots\\\ 
a_1&a_2&\cdots&a_n+x_n
\end{vmatrix}$

$=\begin{vmatrix}
1&a_1&a_2&\cdots&a_n\\\ 
0&a_1+x_1&a_2&\cdots&a_n\\\ 
0&a_1&a_2+x_2&\cdots&a_n\\\ 
\vdots&\vdots&\vdots&\ddots&\vdots\\\ 
0&a_1&a_2&\cdots&a_n+x_n
\end{vmatrix}$

第1行乘以$-1$，加到剩余的每1行
$=\begin{vmatrix}
1&a_1&a_2&\cdots&a_n\\\ 
-1&x_1&0&\cdots&0\\\ 
-1&0&x_2&\cdots&0\\\ 
\vdots&\vdots&\vdots&\ddots&\vdots\\\ 
-1&0&0&\cdots&x_n
\end{vmatrix}$

第2列乘$\frac1{x_1}$，加到第1列
第3列乘$\frac1{x_2}$，加到第1列
$\cdots$
第$n$列乘$\frac1{x_n}$，加到第1列
$=\begin{vmatrix}
1+\sum\limits_{i=1}^n\frac{a_i}{x_i}
&a_1&a_2&\cdots&a_n\\\ 
0&x_1&0&\cdots&0\\\ 
0&0&x_2&\cdots&0\\\ 
\vdots&\vdots&\vdots&\ddots&\vdots\\\ 
0&0&0&\cdots&x_n
\end{vmatrix}$

$=\left(1+\sum\limits_{i=1}^n\frac{a_i}{x_i}\right)\cdot\prod\limits_{i=1}^nx_i$