**证明**  
设 $(f_1,\cdots,f_n)=(e_1,\cdots,e_n)\cdot P\ (1)$  
  
 $(\ \Phi(e_1),\cdots,\Phi(e_n)\ )  
=(e_1,\cdots,e_n)\cdot A\ (2)$  
  
 $(\ \Phi(f_1),\cdots,\Phi(f_n)\ )  
=(f_1,\cdots,f_n)\cdot B\ (3)$  
  
---  
  
 $(f_1,\cdots,f_n)=(e_1,\cdots,e_n)\cdot P$  
  
 $\Rightarrow\begin{cases}  
f_1=a_{11}e_1+\cdots+a_{n1}e_n\\\  
f_2=a_{12}e_1+\cdots+a_{n2}e_n\\\  
\cdots\\\  
f_n=a_{1n}e_1+\cdots+a_{nn}e_n  
\end{cases}$  
  
 $\Rightarrow\begin{cases}  
\Phi(f_1)=\Phi(a_{11}e_1+\cdots+a_{n1}e_n)\\\  
\Phi(f_2)=\Phi(a_{12}e_1+\cdots+a_{n2}e_n)\\\  
\cdots\\\  
\Phi(f_n)=\Phi(a_{1n}e_1+\cdots+a_{nn}e_n)  
\end{cases}$  
  
 $\Rightarrow\begin{cases}  
\Phi(f_1)=a_{11}\Phi(e_1)+\cdots+a_{n1}\Phi(e_n)  
\\\  
\Phi(f_2)=a_{12}\Phi(e_1)+\cdots+a_{n2}\Phi(e_n)  
\\\  
\cdots\\\  
\Phi(f_n)=a_{1n}\Phi(e_1)+\cdots+a_{nn}\Phi(e_n)  
\end{cases}$  
  
 $\Rightarrow  
(\ \Phi(f_1),\cdots,\Phi(f_n)\ )  
=(\ \Phi(e_1),\cdots,\Phi(e_n)\ )\cdot P\ (4)$  
  
---  
  
使用 $(2)$ 式替换 $(4)$ 式的右边  
 $\Rightarrow(\ \Phi(f_1),\cdots,\Phi(f_n)\ )=(e_1,\cdots,e_n)\cdot A\cdot P$  
  
利用 $(1)$ 式替换 $(3)$ 式的右边  
 $\Rightarrow(\ \Phi(f_1),\cdots,\Phi(f_n)\ )=(e_1,\cdots,e_n)\cdot P\cdot B$  
  
---  
继而得到  
 $(\ \Phi(f_1),\cdots,\Phi(f_n)\ )$  
  
 $=(e_1,\cdots,e_n)\cdot A\cdot P$  
  
 $=(e_1,\cdots,e_n)\cdot P\cdot B$  
  
 $\Rightarrow A\cdot P=P\cdot B$  
  
又因为过渡矩阵都是可逆的，即 $P$ 可逆  
  
 $\Rightarrow B=P^{-1}\cdot A\cdot P$  
