**内容**  
设 $f(x)=a_nx^n+a_{n-1}x^{n-1}+\cdots+a_1x+a_0\in K[x]$ ，若存在 $A_n\in K[x]$ ，使得 $f(A)=$ 零矩阵  
则 $A$ 的特征值 $\lambda_1,\lambda_2,\cdots,\lambda_n$ ，使得 $f(\lambda_i)=0,1\le i\le n$   
  
设 $A\in M_n(K),f(x)\in K[x]$ ，若 $f(A)=$ 零矩阵，则 $f(\lambda)=0$   
  
**证明**  
<font color=brown>引证</font>  
 $A\alpha=\lambda\alpha$   
 $\Rightarrow A^n\alpha=A^{n-1}(A\alpha)=A^{n-1}(\lambda\alpha)$   
 $=A^{n-1}(\lambda\alpha)=\lambda\cdot A^{n-1}\alpha=\lambda\cdot A^{n-2}(A\alpha)$   
 $=\lambda^2\cdot A^{n-2}\alpha$   
 $=\lambda^3\cdot A^{n-3}\alpha$   
 $=\cdots$   
 $=\lambda^n\cdot\alpha$   
  
 $A\alpha=\lambda\alpha$   
 $A^2\alpha=A(A\alpha)=A(\lambda\alpha)  
=\lambda(A\alpha)=\lambda(\lambda\alpha)  
=\lambda^2\alpha$   
 $A^3\alpha=A(A^2\alpha)=A(\lambda^2\alpha)  
=\lambda^2(A\alpha)=\lambda^2(\lambda\alpha)  
=\lambda^3\alpha$   
 $A^4\alpha=A(A^3\alpha)=A(\lambda^3\alpha)  
=\lambda^3(A\alpha)=\lambda^3(\lambda\alpha)  
=\lambda^4\alpha$   
 $\Rightarrow A^k\alpha=\lambda^k\alpha$   
  
<font color=brown>正题</font>  
 $f(A)=a_nA^n+a_{n-1}A^{n-1}+\cdots+a_1A+a_0E_n$   
  
 $\Rightarrow f(A)\cdot\alpha=(a_nA^n+a_{n-1}A^{n-1}+\cdots+a_1A+a_0E_n)\cdot\alpha$   
 $=a_nA^n\cdot\alpha+a_{n-1}A^{n-1}\cdot\alpha+\cdots+a_1A\cdot\alpha+a_0E_n\cdot\alpha$   
 $=a_n\lambda^n\cdot\alpha+a_{n-1}\lambda^{n-1}\cdot\alpha+\cdots+a_1\lambda\cdot\alpha+a_0E_n\cdot\alpha$   
 $=a_n\lambda^n\cdot\alpha+a_{n-1}\lambda^{n-1}\cdot\alpha+\cdots+a_1\lambda\cdot\alpha+a_0\cdot\alpha$   
 $=(a_n\lambda^n+a_{n-1}\lambda^{n-1}+\cdots+a_1\lambda+a_0)\cdot\alpha$   
 $=f(\lambda)\cdot\alpha$   
  
 $\Rightarrow f(A)\cdot\alpha=f(\lambda)\cdot\alpha$   
  
又因为 $f(A)=$ 零矩阵  
  
 $\Rightarrow f(\lambda)=0$   
