**证明**  
Case1 $x\to+\infty$  
Step1 不等式放缩  
$x>0,\;[x]\leq x<[x]+1$  
  
$\Rightarrow \dfrac1{[x]+1}<\dfrac1x\leq\dfrac1{[x]}$  
  
$\Rightarrow1+\dfrac1{[x]+1}<1+\dfrac1x\leq1+\dfrac1{[x]}$  
  
$\Rightarrow\left(1+\dfrac1{[x]+1}\right)^x<\left(1+\dfrac1x\right)^x\leq\left(1+\dfrac1{[x]}\right)^x$  
  
$\Rightarrow\left(1+\dfrac1{[x]+1}\right)^{[x]}\leq\left(1+\dfrac1{[x]+1}\right)^x<\left(1+\dfrac1x\right)^x\leq\left(1+\dfrac1{[x]}\right)^x<\left(1+\dfrac1{[x]}\right)^{[x]+1}$  
  
$\Rightarrow\left(1+\dfrac1{[x]+1}\right)^{[x]}<\left(1+\dfrac1x\right)^x<\left(1+\dfrac1{[x]}\right)^{[x]+1}$  
  
Step2 夹逼  
左边:  
$\left(1+\dfrac1{[x]+1}\right)^{[x]}=\dfrac{\left(1+\dfrac1{[x]+1}\right)^{[x]}\cdot\left(1+\dfrac1{[x]+1}\right)}{\left(1+\dfrac1{[x]+1}\right)}=\dfrac{\left(1+\dfrac1{[x]+1}\right)^{[x]+1}}{\left(1+\dfrac1{[x]+1}\right)}$  
  
$\lim\limits_{x\to+\infty}\left(1+\dfrac1{[x]+1}\right)^{[x]}=\lim\limits_{x\to+\infty}\dfrac{\left(1+\dfrac1{[x]+1}\right)^{[x]+1}}{\left(1+\dfrac1{[x]+1}\right)}=\lim\limits_{n\to\infty}\dfrac{\left(1+\dfrac1{n+1}\right)^{n+1}}{\left(1+\dfrac1{n+1}\right)}$  
  
$=\lim\limits_{n\to\infty}{\left(1+\dfrac1{n+1}\right)^{n+1}}\div\lim\limits_{n\to\infty}{\left(1+\dfrac1{n+1}\right)}=e\div1=e$  
  
$\lim\limits_{x\to+\infty}\left(1+\dfrac1{[x]+1}\right)^{[x]}=e$  
  
右边:  
$\left(1+\dfrac1{[x]}\right)^{[x]+1}=\left(1+\dfrac1{[x]}\right)^{[x]}\cdot\left(1+\dfrac1{[x]}\right)$  
  
$\lim\limits_{x\to+\infty}\left(1+\dfrac1{[x]}\right)^{[x]+1}=\lim\limits_{x\to+\infty}\left(1+\dfrac1{[x]}\right)^{[x]}\cdot\lim\limits_{x\to+\infty}\left(1+\dfrac1{[x]}\right)$  
  
$=\lim\limits_{n\to\infty}\left(1+\dfrac1{n}\right)^{n}\cdot\lim\limits_{n\to\infty}\left(1+\dfrac1{n}\right)=e\cdot1$  
  
$\Rightarrow\lim\limits_{x\to+\infty}\left(1+\dfrac1{[x]}\right)^{[x]+1}=e$  
  
---  
  
Case2 $x\to-\infty$  
$\lim\limits_{x\to-\infty}\left(1+\dfrac1x\right)^x$  
  
$=\underline{\lim\limits_{t\to+\infty}\left(1+\dfrac1{-t}\right)^{-t}}=\lim\limits_{t\to+\infty}\left[\left(1+\dfrac1{-t}\right)^{t}\right]^{-1}=\left[\lim\limits_{t\to+\infty}\left(1+\dfrac1{-t}\right)^{t}\right]^{-1}=\dfrac1e$  
  
$=\lim\limits_{t\to+\infty}\left(\dfrac{t-1}t\right)^{-t}$  
  
$=\lim\limits_{t\to+\infty}\left(\dfrac{t}{t-1}\right)^{t}$  
  
$=\lim\limits_{t\to+\infty}\left(\dfrac{t-1+1}{t-1}\right)^{t}$  
  
$=\lim\limits_{t\to+\infty}\left(1+\dfrac{1}{t-1}\right)^{t}$  
  
$=\lim\limits_{t\to+\infty}\left(1+\dfrac{1}{t-1}\right)^{t-1+1}$  
  
$=\lim\limits_{t\to+\infty}\left(1+\dfrac{1}{t-1}\right)^{t-1}\cdot\left(1+\dfrac{1}{t-1}\right)^{1}$  
  
$=\lim\limits_{t\to+\infty}\left(1+\dfrac{1}{t-1}\right)^{t-1}\cdot\lim\limits_{t\to+\infty}\left(1+\dfrac{1}{t-1}\right)^{1}$  
  
$=e\cdot1=e$  
