**举例**  
 $A_{2\times3}，B_{3\times2}$   
  
 $|C_{2\times 2}|  
=|A_{2\times3}\cdot B_{3\times 2}|$   
  
 $=\begin{vmatrix}  
\sum\limits_{k=1}^na_{1k}b_{k1}&  
\sum\limits_{k=1}^na_{1k}b_{k2}\\\   
\sum\limits_{k=1}^na_{2k}b_{k1}&  
\sum\limits_{k=1}^na_{2k}b_{k2}  
\end{vmatrix}$   
  
 $=\left|\begin{bmatrix}  
a_{11}&a_{12}&a_{13}\\\   
a_{21}&a_{22}&a_{23}  
\end{bmatrix}\cdot  
\begin{bmatrix}  
b_{11}&b_{12}\\\   
b_{21}&b_{22}\\\   
b_{31}&b_{32}  
\end{bmatrix}\right|$   
  
 $=\underset{矩阵A的12列}{\begin{vmatrix}  
a_{11}&a_{12}\\\   
a_{21}&a_{22}  
\end{vmatrix}}\cdot  
\underset{矩阵B的12行}{\begin{vmatrix}  
b_{11}&b_{12}\\\   
b_{21}&b_{22}  
\end{vmatrix}}$   
  
 $+\underset{矩阵A的13列}{\begin{vmatrix}  
a_{11}&a_{13}\\\   
a_{21}&a_{23}  
\end{vmatrix}}\cdot  
\underset{矩阵B的12行}{\begin{vmatrix}  
b_{11}&b_{12}\\\   
b_{31}&b_{32}  
\end{vmatrix}}$   
  
 $+\underset{矩阵A的23列}{\begin{vmatrix}  
a_{12}&a_{13}\\\   
a_{22}&a_{23}  
\end{vmatrix}}\cdot  
\underset{矩阵B的23行}{\begin{vmatrix}  
b_{21}&b_{22}\\\   
b_{31}&b_{32}  
\end{vmatrix}}$   
