**举例**  
$f(x)=x^5+2x^4+3x^3+x^2+2x+1,\ b=3$  
$q(x)=x^4+5x^3+18x^2+55x+167,\ (x-3)$  
  
$x^5+2x^4+3x^3+x^2+2x+1-(x^5-3x^4)$  
$\to x^5+2x^4+3x^3+x^2+2x+1-(5x^4-15x^3)$  
$\to 18x^3+x^2+2x+1-(18x^3-54x^2)$  
$\to 55x^2+2x+1-(55x^2-165x)$  
$\to 167x+1-(167x-501)$  
$\to 502$  
$\Rightarrow x^5+2x^4+3x^3+x^2+2x+1$  
$=(x^4+5x^3+18x^2+55x+167)(x-3)+502$  
  
五次项:  $1$  
三次项:  $-15+18=3$  
四次项:  $-3+5=2$  
二次项:  $-3+18+55=1$  
一次项:  $167-55*3=2$  
常数项:  $-3*167+502=1$  
  
$c_{n+m}=a_n\cdot b_m$  
$c_k=\sum\limits_{i+j=a}a_i\cdot b_j$  
$c_0=a_0\cdot b_0$  
  
