**内容**  
设 $\alpha=(x_1,x_2,x_3)$ ， $\beta=(y_1,y_2,y_3)$ 是几何向量，则  
$\alpha$ 平行于 $\beta\Leftrightarrow\begin{vmatrix}x_1&x_2\\\ y_1&y_2\end{vmatrix}=\begin{vmatrix}x_1&x_3\\\ y_1&y_3\end{vmatrix}=\begin{vmatrix}x_2&x_3\\\ y_2&y_3\end{vmatrix}=0$  
  
**证明**  
必要性: $\alpha$ 平行于 $\beta$  
  
$\Rightarrow(x_1,x_2,x_3)=\lambda\cdot(y_1,y_2,y_3)$  
  
$\Rightarrow\begin{vmatrix}x_1&x_2\\\ y_1&y_2\end{vmatrix}=\begin{vmatrix}x_1&x_3\\\ y_1&y_3\end{vmatrix}=\begin{vmatrix}x_2&x_3\\\ y_2&y_3\end{vmatrix}=0$  
  
充分性:  
$\begin{vmatrix}x_1&x_2\\\ y_1&y_2\end{vmatrix}=\begin{vmatrix}x_1&x_3\\\ y_1&y_3\end{vmatrix}=\begin{vmatrix}x_2&x_3\\\ y_2&y_3\end{vmatrix}=0$  
  
$\Rightarrow x_1y_2=x_2y_1$ ， $x_1y_3=x_3y_1$ ， $x_2y_3=x_3y_2$  
  
$\Rightarrow\dfrac{x_1}{y_1}=\dfrac{x_2}{y_2}$ ， $\dfrac{x_1}{y_1}=\dfrac{x_3}{y_3}$ ， $\dfrac{x_2}{y_2}=\dfrac{x_3}{y_3}$  
  
$\Rightarrow\dfrac{x_1}{y_1}=\dfrac{x_2}{y_2}=\dfrac{x_3}{y_3}=\lambda$  
  
$\Rightarrow\alpha$ 平行于 $\beta$  
  
**说明**  
恒等变形  
$\begin{vmatrix}x_1&x_2\\\ y_1&y_2\end{vmatrix}=\begin{vmatrix}x_1&x_3\\\ y_1&y_3\end{vmatrix}=\begin{vmatrix}x_2&x_3\\\ y_2&y_3\end{vmatrix}=0$  
  
$\Rightarrow\begin{vmatrix}1&1&1\\\ x_1&x_2&x_3\\\ y_1&y_2&y_3\end{vmatrix}=0$  
