**形式1**  
 $A_{n\times n}\cdot X_{n\times m}  
=B_{n\times m}$  
  
**求解思路**  
 $A_{n\times n}\cdot X_{n\times m}  
=B_{n\times m}$  
  
 $\Rightarrow A_{n\times n}^{-1}\cdot  
A_{n\times n}\cdot X_{n\times m}  
=A_{n\times n}^{-1}\cdot B_{n\times m}$  
  
 $\Rightarrow E_n \cdot X_{n\times m}  
=A_{n\times n}^{-1}\cdot B_{n\times m}$  
  
 $\Rightarrow X_{n\times m}  
=A_{n\times n}^{-1}\cdot B_{n\times m}$  
  
 $\Rightarrow A_{n\times n}^{-1}\cdot B_{n\times m}$ 相当于对 $B$ 实施若干次初等行变换  
  
**复杂求解步骤**  
先求 $A^{-1}$ ，再右乘 $B_{n\times m}$  
  
**简单求解步骤**  
在计算中验证矩阵 $A$ 是否可逆  
  
 $\left[\begin{array}{c:c}  
A&B\end{array}\right]$  
  
 $\overset{初等行变换}\longrightarrow  
\left[\begin{array}{c:c}  
P_1\cdot A&P_1\cdot B\end{array}\right]$  
  
 $\overset{初等行变换}\longrightarrow  
\left[\begin{array}{c:c}  
P_2\cdot P_1\cdot A&  
P_2\cdot P_1\cdot B\end{array}\right]$  
  
 $\cdots$  
  
 $\overset{初等行变换}\longrightarrow  
\left[\begin{array}{c:c}  
P_r\cdots P_2\cdot P_1\cdot A&  
P_r\cdots P_2\cdot P_1\cdot B\end{array}\right]$  
  
 $=\left[\begin{array}{c:c}  
E_n&A^{-1}\cdot B\end{array}\right]$  
  
