**验证加法**  
  
 $\begin{bmatrix}\lambda+1&\lambda^2+2\\\ 3&\lambda\end{bmatrix}  
+\begin{bmatrix}\lambda+2&\lambda^2+3\\\ \lambda&1\end{bmatrix}  
=\begin{bmatrix}2\lambda+3&2\lambda^2+5\\\ \lambda+3&\lambda+1\end{bmatrix}  
=\begin{bmatrix}0&2\\\ 0&0\end{bmatrix}\lambda^2  
+\begin{bmatrix}2&0\\\ 1&1\end{bmatrix}\lambda  
+\begin{bmatrix}3&5\\\ 3&1\end{bmatrix}$  
  
 $\begin{bmatrix}\lambda+1&\lambda^2+2\\\ 3&\lambda\end{bmatrix}  
=\begin{bmatrix}0&1\\\ 0&0\end{bmatrix}\lambda^2  
+\begin{bmatrix}1&0\\\ 0&1\end{bmatrix}\lambda  
+\begin{bmatrix}1&2\\\ 3&0\end{bmatrix}$  
  
 $\begin{bmatrix}\lambda+2&\lambda^2+3\\\ \lambda&1\end{bmatrix}  
=\begin{bmatrix}0&1\\\ 0&0\end{bmatrix}\lambda^2  
+\begin{bmatrix}1&0\\\ 1&0\end{bmatrix}\lambda  
+\begin{bmatrix}2&3\\\ 0&1\end{bmatrix}$  
