**内容**  
$P_e(\alpha+\beta)=P_e(\alpha)+P_e(\beta)$  
  
$P_e(\lambda\cdot\alpha)=\lambda\cdot P_e(\alpha)$  
  
**证明**  
$\alpha+\beta$  
  
$=(\alpha_1+\alpha_2)+(\beta_1+\beta_2)$  
  
$=[P_e(\alpha)+\bar{P_e}(\alpha)]+[P_e(\beta)+\bar{P_e}(\beta)]$  
  
$=[P_e(\alpha)+P_e(\beta)]+[\bar{P_e}(\alpha)+\bar{P_e}(\beta)]$ (交换律+结合律)  
  
又因为  
  
$\alpha+\beta=P_e(\alpha+\beta)+\bar P_e(\alpha+\beta)$ ，  
  
其中 $P_e(\alpha+\beta)$ 平行于 $\vec e$ ， $\bar P_e(\alpha+\beta)\perp\vec e$  
  
再根据向量分解的唯一性得  
  
$\Rightarrow P_e(\alpha+\beta)=P_e(\alpha)+P_e(\beta)$  
  
$\Rightarrow\bar P_e(\alpha+\beta)=\bar{P_e}(\alpha)+\bar{P_e}(\beta)$  
  
---  
  
$\alpha=P_e(\alpha)+\bar P_e(\alpha)$  
  
$\lambda\cdot\alpha=P_e(\lambda\cdot\alpha)+\bar P_e(\lambda\cdot\alpha)$  
  
$\Rightarrow\lambda[P_e(\alpha)+\bar P_e(\alpha)]=P_e(\lambda\cdot\alpha)+\bar P_e(\lambda\cdot\alpha)$  
  
$\Rightarrow\lambda\cdot P_e(\alpha)+\lambda\cdot\bar P_e(\alpha)]=P_e(\lambda\cdot\alpha)+\bar P_e(\lambda\cdot\alpha)$  
  
$\Rightarrow\lambda\cdot P_e(\alpha)=P_e(\lambda\cdot\alpha)$ ， $\lambda\cdot\bar P_e(\alpha)=\bar P_e(\lambda\cdot\alpha)$  
