**证明-形式3-1**  
$P_1\cdots P_s\cdot A\cdot Q_1\cdots Q_t=\begin{bmatrix}  
E_r&O_{r\times(n-r)}\\\  
O_{(m-r)\times r}&O_{(m-r)\times(n-r)}  
\end{bmatrix}$  
  
$\Rightarrow  
(P_1\cdots P_s)\cdot A\cdot (Q_1\cdots Q_t)$  
$=\begin{bmatrix}  
E_r&O_{r\times(n-r)}\\\  
O_{(m-r)\times r}&O_{(m-r)\times(n-r)}  
\end{bmatrix}$  
  
$\Rightarrow  
P_m\cdot A\cdot Q_n=\begin{bmatrix}  
E_r&O_{r\times(n-r)}\\\  
O_{(m-r)\times r}&O_{(m-r)\times(n-r)}  
\end{bmatrix}$  
  
**证明-形式3-2**  
  
$P_1\cdots P_s\cdot A\cdot Q_1\cdots Q_t  
=\begin{bmatrix}  
E_r&0\\\ 0&0\end{bmatrix}_{m\times n}$  
  
**说明**  
1  $A\in M_{m\times n}(K)$ ： $A$ 是数域 $K$ 上的 $m\times n$ 阶矩阵  
  
2  $P_m\in M_m(K)$ ： $P$ 是数域 $K$ 上的 $n$ 阶方阵  
  
3  $Q_m\in M_m(K)$ ： $Q$ 是数域 $K$ 上的 $n$ 阶方阵  
