**证明**  
<font color=brown>定义映射乘法:</font>  
 $(\Phi\cdot\Psi)(\alpha)  
=(\Phi\circ\Psi)(\alpha)$   
  
<font color=brown>乘法单位元: </font>  
线性恒等变换(线性自同构)： $\mathbf1_V:a\mapsto a$   
 $(\mathbf1_V\cdot\Phi)(\alpha)  
=(\mathbf1_V\circ\Phi)(\alpha)  
=(\Phi)(\alpha)$   
  
<font color=brown>乘法结合律: </font>  
 $(\Phi\cdot\Psi)\cdot\Omega  
=\Phi\cdot(\Psi\cdot\Omega)$   
  
 $\Leftrightarrow(\Phi\circ\Psi)\circ\Omega  
=\Phi\circ(\Psi\circ\Omega)$  (复合映射的结合律)  
  
<font color=brown>数乘相融性：</font>  
 $(k\cdot(\Phi\cdot\Psi))(\alpha)$   
 $=(k\cdot(\Phi\circ\Psi))(\alpha)$   
 $=k\cdot(\Phi(\Psi(\alpha)))$   
  
<font color=brown>乘法分配律:</font>  
左分配律  
 $((\Phi+\Psi)\cdot\Omega)(\alpha)$   
 $=((\Phi+\Psi)\circ\Omega)(\alpha)$   
 $=(\Phi+\Psi)(\Omega(\alpha))$   
 $=\Phi(\Omega(\alpha))+\Psi(\Omega(\alpha))$   
 $=(\Phi\circ\Omega)(\alpha)  
+(\Psi\circ\Omega)(\alpha)$   
 $=(\Phi\cdot\Omega)(\alpha)  
+(\Psi\cdot\Omega)(\alpha)$   
  
 $\Rightarrow(\Phi+\Psi)\cdot\Omega  
=\Phi\cdot\Omega+\Psi\cdot\Omega$   
  
右分配律  
 $(\Omega\cdot(\Phi+\Psi))(\alpha)$   
 $=(\Omega\circ(\Phi+\Psi))(\alpha)$   
 $=\Omega((\Phi+\Psi)(\alpha))$   
 $=\Omega(\Phi(\alpha)+\Psi(\alpha))$   
 $=(\Omega\circ\Phi)(\alpha)  
+(\Omega\circ\Psi)(\alpha)$   
 $=(\Omega\cdot\Phi)(\alpha)  
+(\Omega\cdot\Psi)(\alpha)$   
