**内容**  
设 $V，U$ 是数域 $K$ 上的线性空间， $\Phi$ 是从 $V$ 到 $U$ 的线性映射，则 $\Phi(\mathbf0_V)=\mathbf0_U$ ，即线性映射 $\Phi$ 将 $V$ 中零向量 $\mathbf0_V$ 映射成 $U$ 中的零向量 $\mathbf0_U$  
  
**证明**  
令 $\alpha=\beta=\mathbf0_V\in V$  
  
$\Phi$ 是线性映射  
  
$\Rightarrow  
\Phi(\alpha+\beta)=\Phi(\alpha)+\Phi(\beta)$  
  
$\Rightarrow\Phi(\mathbf0_V)  
=\Phi(\mathbf0_V+\mathbf0_V)  
=\Phi(\mathbf0_V)+\Phi(\mathbf0_V)$  
  
$\Rightarrow\Phi(\mathbf0_V)  
-\Phi(\mathbf0_V)=\Phi(\mathbf0_V)$  (移项/消去律)  
  
$\Rightarrow\mathbf0_U=\Phi(\mathbf0_V)$  
  
**说明**  
反之不成立，即 $\Phi(\alpha)=\mathbf0_U  
\not\Rightarrow\alpha=\mathbf0_V$  
