**例**
$\begin{cases}
x_1+2x_2-x_3+3x_4+x_5=2\\\ 
2x_1+4x_2-2x_3+6x_4+3x_5=6\\\ 
-x_1-2x_2+x_3-x_4+3x_5=4
\end{cases}$

解：

$\Rightarrow\left[\begin{array}{ccccc:c}
1&2&-1&3&1&2\\\ 
2&4&-2&6&3&6\\\ 
-1&-2&1&-1&3&4
\end{array}\right]$

$\xrightarrow{初等行变换，行阶梯型矩阵}
\begin{bmatrix}
\underline{1}&2&-1&3&1&2\\\ 
0&0&0&\underline{2}&4&6\\\ 
0&0&0&0&\underline{1}&2
\end{bmatrix}$

$\xrightarrow{简化行阶梯型矩阵}
\begin{bmatrix}
\underline{1}&2&-1&0&0&3\\\ 
0&0&0&\underline{1}&0&-1\\\ 
0&0&0&0&\underline{1}&2
\end{bmatrix}$

$\xrightarrow{x_4\to x_2，
x_5\to x_3}
\begin{bmatrix}
1&0&0&2&-1&3\\\ 
0&1&0&0&0&-1\\\ 
0&0&1&0&0&2
\end{bmatrix}$

$\Rightarrow\delta_1=\begin{bmatrix}
-2\\\ 0\\\ 0\\\ 1\\\ 0\end{bmatrix}，
\delta_2=\begin{bmatrix}
1\\\ 0\\\ 0\\\ 0\\\ 1\end{bmatrix}，
\zeta=\begin{bmatrix}
3\\\ -1\\\ 2\\\ 0\\\ 0\end{bmatrix}$

$\xrightarrow{x_2\to x_4，
x_3\to x_5}
\eta_1=\begin{bmatrix}
-2\\\ 1\\\ 0\\\ 0\\\ 0\end{bmatrix}，
\eta_2=\begin{bmatrix}
1\\\ 0\\\ 1\\\ 0\\\ 0\end{bmatrix}，
\gamma=\begin{bmatrix}
3\\\ 0\\\ 0\\\ -1\\\ 2\end{bmatrix}$

$\Rightarrow$通解为$\gamma+c_1\cdot\eta_1
+c_2\cdot\eta_2，c_i\in K$