**内容**
$\lim u(x)=a>0,\;\lim v(x)=b$

$\Rightarrow\lim u(x)^{v(x)}=a^b$

**具体形式: $x\to x_0$**
$\lim\limits_{x\to x_0} u(x)=a>0,\;\lim\limits_{x\to x_0} v(x)=b$

$\Rightarrow\lim\limits_{x\to x_0} u(x)^{v(x)}=a^b$

**具体形式: $x\to x_0^{-}$**
$\lim\limits_{x\to x_0^-} u(x)=a>0,\;\lim\limits_{x\to x_0^-} v(x)=b$

$\Rightarrow\lim\limits_{x\to x_0^-} u(x)^{v(x)}=a^b$

**具体形式: $x\to x_0^{+}$**
$\lim\limits_{x\to x_0^+} u(x)=a>0,\;\lim\limits_{x\to x_0^+} v(x)=b$

$\Rightarrow\lim\limits_{x\to x_0^+} u(x)^{v(x)}=a^b$

**具体形式: $x\to+\infty$**
$\lim\limits_{x\to+\infty} u(x)=a>0,\;\lim\limits_{x\to+\infty} v(x)=b$

$\Rightarrow\lim\limits_{x\to+\infty} u(x)^{v(x)}=a^b$

**具体形式: $x\to-\infty$**
$\lim\limits_{x\to-\infty} u(x)=a>0,\;\lim\limits_{x\to-\infty} v(x)=b$

$\Rightarrow\lim\limits_{x\to-\infty} u(x)^{v(x)}=a^b$

**具体形式: $x\to\infty$**
$\lim\limits_{x\to\infty} u(x)=a>0,\;\lim\limits_{x\to\infty} v(x)=b$

$\Rightarrow\lim\limits_{x\to\infty} u(x)^{v(x)}=a^b$
