**内容**
$\limsup\limits_{n\to\infty}x_n=H$

$\iff\forall\;\epsilon>0$

$i\;)\;\exists\;N>0,\;n>N,\;x_n<H+\epsilon$

$ii\;)\;\{\cdots,x_n,\cdots\},\;x_n>H-\epsilon$

**证明: 必要性**
$\limsup\limits_{n\to\infty}x_n=H$

$i\;)$

$\Rightarrow H+\epsilon\leq x_k\leq M,\;1\leq k\leq n$

$\Rightarrow \exists\;N>0,\;n>N,\;x_n<H+\epsilon$

$ii\;)$

$\Rightarrow \forall\;\epsilon>0,\;\mathbf{U}(H,\epsilon)\cap\{x_n\}=\{\cdots,x_k,\cdots\}$

**证明: 充分性**
$\forall\;\epsilon>0,\;\exists\;N>0,\;n>N,\;x_n<H+\epsilon$

$\Rightarrow\forall\,\lim\limits_{k\to\infty}x_{n_k}=\xi_i\leq H+\epsilon$

$\Rightarrow\limsup\limits_{n\to\infty}x_n\leq H+\epsilon$

---

$\{\cdots,x_n,\cdots\},\;(M>)x_n>H-\epsilon$

$\Rightarrow\forall\,\lim\limits_{k\to\infty}x_{n_k}=\xi_i\geq H-\epsilon$

$\Rightarrow\limsup\limits_{n\to\infty}x_n\geq H-\epsilon$

---

$\Rightarrow H-\epsilon\leq\limsup\limits_{n\to\infty}x_n\leq H+\epsilon$

$\Rightarrow\lim\limits_{\epsilon\to0}(H-\epsilon)\leq\lim\limits_{\epsilon\to0}\left(\limsup_{n\to\infty}x_n\right)\leq \lim\limits_{\epsilon\to0}(H+\epsilon)$

$\Rightarrow\limsup\limits_{n\to\infty}x_n=H$
