$\begin{vmatrix}  
a&0&0&b\\\  
0&a&b&0\\\  
0&c&d&0\\\  
c&0&0&d  
\end{vmatrix}$  
  
$=-\underset{第4行与第3行交换}{\begin{vmatrix}  
a&0&0&b\\\  
0&a&b&0\\\  
c&0&0&d\\\  
0&c&d&0  
\end{vmatrix}}  
=\underset{第3行与第2行交换}{\begin{vmatrix}  
a&0&0&b\\\  
c&0&0&d\\\  
0&a&b&0\\\  
0&c&d&0  
\end{vmatrix}}$  
  
$=\underset{第4列与第3列交换}{\begin{vmatrix}  
a&0&b&0\\\  
c&0&d&0\\\  
0&a&0&b\\\  
0&c&0&d  
\end{vmatrix}}  
=\underset{第3列与第2列交换}{\begin{vmatrix}  
a&b&0&0\\\  
c&d&0&0\\\  
0&0&a&b\\\  
0&0&c&d  
\end{vmatrix}}$  
  
$=(ab-bc)^2$  
