**内容**  
设 $t(x)\in K[x],\  d(x)=(f(x),g(x))$  
则 $(f(x)\cdot t(x),\ g(x)\cdot t(x))=d(x)\cdot t(x)$  
$\enspace\enspace(f(x)\cdot t(x),\ g(x)\cdot t(x))=(f(x),\ g(x))\cdot t(x)$  
  
**证明**  
先证明是公因式  
$d(x)=(f(x),g(x))$  
$\Rightarrow\exists\ u(x),v(x)\in K[x],\  
d(x)=f(x)u(x)+g(x)v(x)$  
两边同时乘以 $t(x)$  
$\Rightarrow  
d(x)t(x)=f(x)u(x)t(x)+g(x)v(x)t(x)$  
$\Rightarrow  
d(x)t(x)=[f(x)t(x)]u(x)+[g(x)t(x)]v(x)$  
$\Rightarrow d(x)t(x)$ 是 $f(x)t(x),\ g(x)t(x)$ 的公因式  
  
再证明是最大公因式  
任取 $f(x)t(x),\ g(x)t(x)$ 的公因式 $h(x)$  
$\Rightarrow h(x)|f(x)t(x),\ h(x)|g(x)t(x)$  
又因为 $d(x)t(x)=[f(x)t(x)]u(x)+[g(x)t(x)]v(x)$  
$\Rightarrow h(x)|d(x)t(x)$  
$\Rightarrow d(x)t(x)$ 是最大公因式  
