**内容**  
设 $(e_1,e_2,\cdots,e_n)$ 是线性空间 $V_K$ 的一个基，矩阵 $A,B\in M_{n\times m}(K)$ ，若 $(e_1,e_2,\cdots,e_n)A=(e_1,e_2,\cdots,e_n)B$ ，则 $A=B$  
  
**证明**  
$(e_1,e_2,\cdots,e_n)\cdot A  
=\left(\sum\limits_{i=1}^na_{i1}\cdot e_i，\cdots，  
\sum\limits_{i=1}^na_{im}\cdot e_i\right)$  
  
$(e_1,e_2,\cdots,e_n)\cdot B  
=\left(\sum\limits_{i=1}^nb_{i1}\cdot e_i，\cdots，  
\sum\limits_{i=1}^nb_{im}\cdot e_i\right)$  
  
$\Rightarrow\sum\limits_{i=1}^na_{i1}\cdot e_i  
=\sum\limits_{i=1}^nb_{i1}\cdot e_i，\cdots，  
\sum\limits_{i=1}^na_{im}\cdot e_i  
=\sum\limits_{i=1}^nb_{im}\cdot e_i$  
  
$\Rightarrow\forall\ 1\le i\le n，a_{i1}=b_{i1}, a_{i2}=b_{i2}，  
\cdots，a_{im}=b_{im}$  
  
$\Rightarrow\forall\ 1\le i\le n，1\le j\le m，  
a_{ij}=b_{ij}$  
  
$\Rightarrow A=B$  
