**加法**  
 $\Phi+\Psi\iff A+B$   
  
加法交换律:  $\Phi+\Psi=\Psi+\Phi$   
 $\iff A+B=B+A$   
  
加法结合律:  $(\Phi+\Psi)+\Omega=\Phi+(\Psi+\Omega)$   
 $\iff (A+B)+C=A+(B+C)$   
  
---  
  
**乘法**  
 $\Psi\circ\Phi\iff AB$   
  
乘法结合律:  $\Omega\circ(\Psi\circ\Phi)=(\Omega\circ\Psi)\circ\Phi$   
 $\iff C(BA)=C(BA)$   
  
右分配律:  $\Phi\circ(\Psi+\Omega)=\Phi\circ\Psi+\Phi\circ\Omega$   
 $\iff A(B+C)=AB+AC$   
  
左分配律:  $(\Psi+\Omega)\circ\Phi=\Psi\circ\Phi+\Omega\circ\Phi$   
 $\iff (B+C)A=BA+CA$   
  
数乘:  $k\cdot\Phi\iff k\cdot A$   
  
数乘相融性:  $k(\Phi\circ\Psi)=(k\Phi)\circ\Psi=\Phi\circ(k\Psi)$   
 $\iff k(AB)=(kA)B=A(kB)$   
  
数乘结合律:  $(kl)\Phi=k(l\Phi)$   
 $\iff(kl)A=k(lA)$   
  
---  
  
**幂运算**  
 $\underbrace{\Phi\circ\Phi\circ\cdots\Phi}_{n个}=\Phi^n$   
  
 $\iff\underbrace{A\cdot A\cdot\cdots A}_{n个}=A^n$   
  
 $\Phi^n\circ\Phi^m=\Phi^{n+m}$   
 $\iff A^n\cdot A^m=A^{n+m}$   
  
 $(\Phi^n)^m=\Phi^{nm}\iff(A^n)^m=A^{nm}$   
  
 $\Phi^0=I_V\iff A^0=I_n$   
  
 $\underbrace{\Phi^{-1}\circ\Phi^{-1}\circ\cdots\Phi^{-1}}_{n个}=(\Phi^{-1})^n=\Phi^{-n}$   
  
 $\iff\underbrace{A^{-1}\cdot A^{-1}\cdot\cdots A^{-1}}_{n个}=(A^{-1})^n=A^{-n}$   
  
 $(A\cdot A\cdot\cdots A)^{-1}=A^{-1}\cdot A^{-1}\cdot\cdots A^{-1}$   
 $\Rightarrow (A^n)^{-1}=(A^{-1})^n$   
  
幂等变换  
 $\Phi^2=\Phi\iff A^2=A$   
  
幂零变换  
 $\Phi^n=$ 零线性变换 $\iff A^n=$ 零矩阵  
  
---  
  
**逆映射**  
 $\Phi\circ\Psi=\Psi\circ\Phi=I_V$   
 $\iff AB=BA=I_n$   
 $\Phi^{-1}\leftrightharpoons A^{-1}$   
  
 $(\Phi\circ\Psi)^{-1}=\Psi^{-1}\circ\Phi^{-1}$   
 $\iff(AB)^{-1}=B^{-1}A^{-1}$   
  
---  
  
零线性映射 $\leftrightharpoons$ 零矩阵  
单位阵 $\leftrightharpoons$ 恒等变换  
  
---  
  
运算性质:  
 $\Phi\leftrightharpoons A$ ， $\Phi^\star\leftrightharpoons A^T$   
  
 $(1)\ (\Phi+\Psi)^\star=\Phi^\star+\Psi^\star$ ，  
 $(A+B)^T=A^T+B^T$   
 $(\overline{A+B})^T=(\overline A)^T+(\overline B)^T$   
  
 $(2)\ (c\cdot\Phi)^\star=\overline{c}\cdot\Phi^\star$ ，  
 $(c\cdot A)^T=c\cdot A^T$   
 $(\overline{c\cdot A})^T=\bar c\cdot(\bar A)^T$   
  
 $(3)\ (\Phi\circ\Psi)^\star=\Psi^\star\circ\Phi^\star$ ，  
 $(AB)^T=B^T\cdot A^T$   
 $(\overline{AB})^T=(\bar B)^T\cdot (\bar A)^T$   
  
 $(4)\ (\Phi^\star)^\star=\Phi$ ，  
 $(A^T)^T=A$   
共轭转置，再共轭转置  
  
  
 $(5)\ $ 若 $\Phi$ 可逆，则 $\Phi^\star$ 也可逆，且 $(\Phi^\star)^{-1}=(\Phi^{-1})^\star$ ，  
 $(A^T)^{-1}=(A^{-1})^T$   
 $(A^T)^{-1}=(A^{-1})^T$   
