**证明思路**  
左边的第 $(i,j)$ 元素 $=$ 右边的第 $(i,j)$ 元素  
  
**证明：**  
 $(AB)^T$ 的第 $(i,j)$ 元  
 $=(AB)$ 的第 $(j,i)$ 元  
  
 $=A$ 的第 $j$ 行 $\cdot B$ 的第 $i$ 列  
  
 $=\sum\limits_{k=1}^na_{jk}\cdot b_{ki}$  
  
 $(B^T\cdot A^T)$ 的第 $(i,j)$ 元  
 $=B^T$ 的第 $i$ 行 $\cdot A^T$ 的第 $j$ 列  
 $=B$ 的第 $i$ 列 $\cdot A$ 的第 $j$ 行  
 $=\sum\limits_{k=1}^nb_{ki}\cdot a_{jk}$  
  
 $\Rightarrow(AB)^T=B^T\cdot A^T$  
  
**补充**  
 $(A_{2\times3}\cdot B_{3\times6})^T  
=B_{3\times6}^T\cdot A_{2\times3}^T$  
  
 $A_{2\times3}^T\to3\times2$  
  
 $B_{3\times6}^T\to6\times3$  
  
没法相乘  
