**证明**  
设 $A=(a_{ij})_{n\times n}$   
  
 $B=(b_{ij})_{n\times n}$   
  
构造一个 $2n$ 阶方阵  
 $C=\begin{bmatrix}  
A&O\\\ -E&B  
\end{bmatrix}$   
  
 $\Rightarrow|C|=$   
  
 $\left|\begin{array}{cccc:cccc}  
a_{11}&a_{12}&\cdots&a_{1n}&0&0&\cdots&0\\\   
a_{21}&a_{22}&\cdots&a_{2n}&0&0&\cdots&0\\\   
\vdots&\vdots&\ddots&\vdots&\vdots&\vdots&\ddots&\vdots\\\   
a_{n1}&a_{n2}&\cdots&a_{nn}&0&0&\cdots&0\\\   
-1&0&\cdots&0&b_{11}&b_{12}&\cdots&b_{1n}\\\   
0&-1&\cdots&0&b_{21}&b_{22}&\cdots&b_{2n}\\\   
0&0&\cdots&0&\vdots&\vdots&\ddots&\vdots\\\   
0&0&\cdots&-1&b_{n1}&b_{n2}&\cdots&b_{nn}  
\end{array}\right|$   
  
执行以下操作  
  
第 $n+1$ 行乘以 $a_{11}$ 加到第1行  
  
第 $n+1$ 行乘以 $a_{21}$ 加到第2行  
  
 $\cdots$   
  
第 $n+1$ 行乘以 $a_{n1}$ 加到第 $n$ 行  
  
 $\left|\begin{array}{cccc:cccc}  
0&a_{12}&\cdots&a_{1n}&a_{11}b_{11}&a_{11}b_{12}&\cdots&a_{11}b_{1n}\\\   
0&a_{22}&\cdots&a_{2n}&a_{21}b_{11}&a_{21}b_{12}&\cdots&a_{21}b_{1n}\\\   
\vdots&\vdots&\ddots&\vdots&\vdots&\vdots&\ddots&\vdots\\\   
0&a_{n2}&\cdots&a_{nn}&a_{n1}b_{11}&a_{n1}b_{12}&\cdots&a_{n1}b_{1n}\\\   
-1&0&\cdots&0&b_{11}&b_{12}&\cdots&b_{1n}\\\   
0&-1&\cdots&0&b_{21}&b_{22}&\cdots&b_{2n}\\\   
0&0&\cdots&0&\vdots&\vdots&\ddots&\vdots\\\   
0&0&\cdots&-1&b_{n1}&b_{n2}&\cdots&b_{nn}  
\end{array}\right|$   
  
依次类推：  
  
用 $a_{ij}$ 乘以行列式 $C$ 的第 $n+j$ 行，加到行列式 $C$ 的第 $i$ 行，  
  
一共执行 $n^2$ 次，得到以下行列式  
  
 $\left|\begin{array}{cccc:cccc}  
0&a_{12}&\cdots&a_{1n}&\sum\limits_{r=1}^na_{1r}b_{r1}&\sum\limits_{r=1}^na_{1r}b_{r2}&\cdots&\sum\limits_{r=1}^na_{1r}b_{rn}\\\   
0&a_{22}&\cdots&a_{2n}&\sum\limits_{r=1}^na_{2r}b_{r1}&\sum\limits_{r=1}^na_{2r}b_{r2}&\cdots&\sum\limits_{r=1}^na_{2r}b_{rn}\\\   
\vdots&\vdots&\ddots&\vdots&\vdots&\vdots&\ddots&\vdots\\\   
0&a_{n2}&\cdots&a_{nn}&\sum\limits_{r=1}^na_{nr}b_{r1}&\sum\limits_{r=1}^na_{nr}b_{r2}&\cdots&\sum\limits_{r=1}^na_{nr}b_{rn}\\\   
-1&0&\cdots&0&b_{11}&b_{12}&\cdots&b_{1n}\\\   
0&-1&\cdots&0&b_{21}&b_{22}&\cdots&b_{2n}\\\   
0&0&\cdots&0&\vdots&\vdots&\ddots&\vdots\\\   
0&0&\cdots&-1&b_{n1}&b_{n2}&\cdots&b_{nn}  
\end{array}\right|$   
  
  
  
 $\Rightarrow|C|  
=\begin{vmatrix}  
A&0\\\ -E&B  
\end{vmatrix}  
=\begin{vmatrix}  
0&AB\\\ -E&B  
\end{vmatrix}$   
  
