**内容**    
同余关系是等价关系    
    
**证明**    
反身性: 若 $f(x)\equiv f(x)\ (\bmod\ m(x))$ ，则 $f(x)\equiv f(x)\ (\bmod\ m(x))$     
 $f(x)\equiv f(x)\ (\bmod\ m(x))$     
 $\Leftrightarrow m(x)\mid[f(x)-f(x)]$     
 $\Leftrightarrow f(x)\equiv f(x)\ (\bmod\ m(x))$     
    
对称性: 若 $f(x)\equiv g(x)\ (\bmod\ m(x))$ ，则 $g(x)\equiv f(x)\ (\bmod\ m(x))$     
 $f(x)\equiv g(x)\ (\bmod\ m(x))$     
 $\Leftrightarrow m(x)\mid[f(x)-g(x)]$     
 $\Leftrightarrow m(x)\mid[-(f(x)-g(x))]$     
 $\Leftrightarrow m(x)\mid[g(x)-f(x)]$     
 $\Leftrightarrow g(x)\equiv f(x)\ (\bmod\ m(x))$     
    
传递性: 若 $f(x)\equiv g(x)\ (\bmod\ m(x))$ ，若 $g(x)\equiv h(x)\ (\bmod\ m(x))$ ，则 $f(x)\equiv h(x)\ (\bmod\ m(x))$     
 $f(x)\equiv g(x)\ (\bmod\ m(x))$     
 $\Rightarrow m(x)\mid[f(x)-g(x)]$     
 $\Rightarrow f(x)-g(x)=m(x)\cdot q_1(x)$     
    
 $g(x)\equiv h(x)\ (\bmod\ m(x))$     
 $\Rightarrow m(x)\mid[g(x)-h(x)]$     
 $\Rightarrow g(x)-h(x)=m(x)\cdot q_2(x)$     
    
 $\Rightarrow [f(x)-g(x)]+[g(x)-h(x)]=[m(x)\cdot q_1(x)]+[m(x)\cdot q_2(x)]$     
 $\Rightarrow f(x)-h(x)=m(x)\cdot[q_1(x)+q_2(x)]$     
 $\Rightarrow m(x)\mid[\ f(x)-h(x)\ ]$     
 $\Rightarrow f(x)\equiv h(x)\ (\bmod\ m(x))$     
