**性质1**
若$f(x)\equiv 0\ (\bmod\ m(x))$，则$m(x)|f(x)$

**证明**
$f(x)\equiv 0\ (\bmod(m(x)))$
$\Rightarrow m(x)\mid(f(x)-0)$
$\Rightarrow m(x)\mid f(x)$

---

**性质2**
若$f(x)\equiv 1\ (\bmod\ m(x))$，则$1=\rm{gcd}(f(x),m(x))$

**证明**
$f(x)\equiv 1\ (\bmod\ m(x))$
$\Rightarrow m(x)\mid[f(x)-1]$
$\Rightarrow f(x)-1=m(x)\cdot q(x)$
$\Rightarrow 1=f(x)-m(x)\cdot q(x)$
$\Rightarrow 1=f(x)\cdot 1-m(x)\cdot q(x)$
$\Rightarrow\exists q(x),1\in K[x], \rm{s.t.}\ 1=f(x)\cdot 1-m(x)\cdot q(x)$
$\Rightarrow1=\rm{gcd}(f(x),m(x))$
$\Rightarrow f(x)$与$m(x)$互素

**说明**
反之不成立
$f(x)$与$m(x)$互素
$\Rightarrow\exists u(x),v(x)\in K[x], \rm{s.t.}\ 1=f(x)\cdot u(x)+m(x)\cdot v(x)$
$\Rightarrow m(x)\mid[f(x)\cdot u(x)-1]$
$\Rightarrow f(x)\cdot u(x)\equiv1\ (\bmod\ m(x))$

---

**性质3**
若$a(x)\equiv b(x)\ (\bmod\ m(x))$，$c(x)\equiv d(x)\ (\bmod\ m(x))$
则$[a(x)\pm c(x)]\equiv[b(x)\pm d(x)]\ (\bmod\ m(x))$

**证明**
$a(x)\equiv b(x)\ (\bmod\ m(x))$
$\Rightarrow a(x)-b(x)=m(x)\cdot q_1(x)\cdots(1)$

$c(x)\equiv d(x)\ (\bmod\ m(x))$
$\Rightarrow c(x)-d(x)=m(x)\cdot q_2(x)\cdots(2)$

$(1)$式$(2)$式相加得
$\Rightarrow a(x)-b(x)+c(x)-d(x)=m(x)\cdot q_1(x)+m(x)\cdot q_2(x)$
$\Rightarrow [a(x)+c(x)]-[b(x)+d(x)]=m(x)\cdot[q_1(x)+q_2(x)]$
$\Rightarrow m(x)\mid[a(x)+c(x)]-[b(x)+d(x)]$
$\Rightarrow [a(x)+c(x)]\equiv[b(x)+d(x)]\ (\bmod\ m(x))$

$(1)$式$(2)$式相减得
$\Rightarrow a(x)-b(x)-c(x)+d(x)=m(x)\cdot q_1(x)-m(x)\cdot q_2(x)$
$\Rightarrow [a(x)-c(x)]-[b(x)-d(x)]=m(x)\cdot[q_1(x)+q_2(x)]$
$\Rightarrow m(x)\mid[a(x)-c(x)]-[b(x)-d(x)]$
$\Rightarrow [a(x)-c(x)]\equiv[b(x)-d(x)]\ (\bmod\ m(x))$

---

**性质4**
若$a(x)\equiv b(x)\ (\bmod\ m(x))$，$c(x)\equiv d(x)\ (\bmod\ m(x))$
则$[a(x)\cdot c(x)]\equiv[b(x)\cdot d(x)]\ (\bmod\ m(x))$

**证明**
$a(x)\equiv b(x)\ (\bmod\ m(x))$
$\Rightarrow a(x)-b(x)=m(x)\cdot q_1(x)$
$\Rightarrow a(x)=m(x)\cdot q_1(x)+b(x)\cdots(1)$

$c(x)\equiv d(x)\ (\bmod\ m(x))$
$\Rightarrow c(x)-d(x)=m(x)\cdot q_2(x)$
$\Rightarrow c(x)=m(x)\cdot q_2(x)+d(x)\cdots(2)$

$(1)$式$(2)$式相乘得
$a(x)\cdot c(x)=[m(x)\cdot q_1(x)+b(x)]\cdot[m(x)\cdot q_2(x)+d(x)]$
$=m(x)\cdot q_1(x)\cdot m(x)\cdot q_2(x)+[b(x)q_2(x)+d(x)q_1(x)]\cdot m(x)+b(x)\cdot d(x)$

移项得
$\Rightarrow a(x)\cdot c(x)-b(x)d(x)=m(x)\cdot q_1(x)\cdot m(x)\cdot q_2(x)+[b(x)q_2(x)+d(x)q_1(x)]\cdot m(x)$
$=m(x)\cdot[q_1(x)\cdot m(x)\cdot q_2(x)+[b(x)q_2(x)+d(x)q_1(x)]]$
$\Rightarrow m(x)\mid[a(x)\cdot c(x)-b(x)\cdot d(x)]$
$\Rightarrow [a(x)\cdot c(x)]\equiv[b(x)\cdot d(x)]\ (\bmod\ m(x))$

---

**性质5**
若$a(x)\equiv b(x)\ (\bmod\ p(x))$，$a(x)\equiv b(x)\ (\bmod\ q(x))$，$1=\rm{gcd}(p(x),q(x))$
则$a(x)\equiv b(x)\ (\bmod\ p(x)\cdot q(x))$

**证明**
$a(x)\equiv b(x)\ (\bmod\ p(x))$
$\Rightarrow p(x)\mid[a(x)-b(x)]$

$a(x)\equiv b(x)\ (\bmod\ q(x))$
$\Rightarrow q(x)\mid[a(x)-b(x)]$

又因为$1=\rm{gcd}(p(x),q(x))$
$\Rightarrow[p(x)\cdot q(x)]\mid[a(x)-b(x)]\ $（互素的性质1）
$\Rightarrow a(x)\equiv b(x)\ (\bmod\ p(x)\cdot q(x))$
