**证明**  
$y=f(u),\;\lim\limits_{u\to u_0}f(u)=f(u_0)$  
  
$\Rightarrow\forall\;\epsilon>0,\;\exists\;\delta>0,\;|u-u_0|<\delta,\;|\,f(u)-f(u_0)|<\epsilon$  
  
$\Rightarrow\forall\;\epsilon>0,\;\exists\;\delta>0,\;|\varphi(x)-\varphi(x_0)|<\delta,\;\left|\,f\,[\varphi(x)]-f\,[\varphi(x_0)]\right|<\epsilon$  
  
  
$\rm{let}\;\epsilon\prime=\delta,\;(\lim\limits_{x\to x_0}\varphi(x)=\varphi(x_0))$  
  
$\Rightarrow\exists\;\delta^\prime>0,\;|x-x_0|<\delta^\prime,\;|\varphi(x)-\varphi(x_0)|<\epsilon\prime=\delta$  
  
  
$\underline{(\forall\;\epsilon\to\exists\;\delta\to\forall\;\epsilon\prime(\leq\delta)\to\exists\;\delta\prime)}$  
  
$\Rightarrow\forall\;\epsilon>0,\;\exists\;\delta\prime>0,\;|x-x_0|<\delta^\prime,\;\left|\,f\,[\varphi(x)]-f\,[\varphi(x_0)]\right|<\epsilon$  
  
$\Rightarrow y=f\,[\varphi(x)],\;\lim\limits_{x\to x_0}f\,[\varphi(x)]=f\,[\varphi(x_0)]$  
