**例**    
 $\begin{vmatrix}    
1&-1&1&x-1\\\     
1&-1&x+1&-1\\\      
1&x-1&1&-1\\\     
x+1&-1&1&-1    
\end{vmatrix}$     
    
**解**    
 $\begin{vmatrix}    
1&-1&1&x-1\\\     
1&-1&x+1&-1\\\      
1&x-1&1&-1\\\     
x+1&-1&1&-1    
\end{vmatrix}$     
    
 $\overset{转置}{=}    
\begin{vmatrix}    
1&1&1&x+1\\\     
-1&-1&x-1&-1\\\      
1&x+1&1&1\\\     
x-1&-1&-1&-1    
\end{vmatrix}$     
    
 $\overset{每行乘1或-1加到第1行}{=}    
\begin{vmatrix}    
x&x&x&x\\\     
-1&-1&x-1&-1\\\      
1&x+1&1&1\\\     
x-1&-1&-1&-1    
\end{vmatrix}$     
    
 $\overset{提取公因子}{=}    
x\cdot\begin{vmatrix}    
1&1&1&1\\\     
-1&-1&x-1&-1\\\      
1&x+1&1&1\\\     
x-1&-1&-1&-1    
\end{vmatrix}$     
    
 $\overset{倍加}{=}    
x\cdot\begin{vmatrix}    
1&1&1&1\\\     
0&0&x&0\\\      
0&x&0&0\\\     
x&0&0&0    
\end{vmatrix}    
=x\cdot(-1)^{\frac{4\times3}2}(1\cdot x^3)=x^4$     
    
或者    
 $\overset{交换第1列与第4列，第2列与第3列}{=}    
x\cdot\begin{vmatrix}    
1&1&1&1\\\     
0&x&0&0\\\      
0&0&x&0\\\     
0&0&0&x    
\end{vmatrix}=x^4$     
